Cleanup. Updated bad_pos invariant. Resolved several admits.

theories/examples/authentikit_susp_security.v
@@ -6,51 +6,12 @@ From auth.examples Require Export authentikit_susp authentikit_base_susp_securit
 From iris.base_logic.lib Require Export na_invariants.
 From iris.algebra Require Import auth agree numbers csum excl.
 
-(* Class tableG (Σ: gFunctors) := {
-  tableG_na_invG :: na_invG Σ;
-  tableG_name: gname;
-}.
-
-Definition table_inv `{!invGS_gen hlc Σ} `{!tableG Σ} (N : namespace) (P : iProp Σ) :=
-  na_inv tableG_name N P.
-Definition table_tok `{!invGS_gen hlc Σ} `{!tableG Σ} (E : coPset) :=
-  na_own tableG_name E. *)
-
-(* Definition idcntrUR := authUR nat.
-Class idcntrG Σ := IdcntrG { idcntr_inG :> inG Σ idcntrUR; idcntrG_name : gname }. *)
-
-(* Definition msizeUR := authUR natUR.
-Class msizeG Σ := MsizeG { msize_inG :> inG Σ msizeUR; msizeG_name : gname }.
-
-Lemma msize_alloc `{inG Σ msizeUR} :
-  ⊢ |==> ∃ _ : msizeG Σ,
-      (own msizeG_name (●{DfracOwn (1/2)} 0) ∗
-         own msizeG_name (●{DfracOwn (1/2)} 0) ∗ own msizeG_name (◯ 0))%I.
-Proof.
-  iMod (own_alloc (● 0 ⋅ ◯ 0)) as (γ) "[Hauth Hfrag]"; [admit|].
-  set (H1 := MsizeG _ _ γ).
-  iExists _. iDestruct "Hauth" as "[$ $]".
-  by iFrame.
-Admitted. *)
-
-(* Lemma idcntr_alloc `{inG Σ idcntrUR} :
-  ⊢ |==> ∃ _ : idcntrG Σ, (own idcntrG_name (●{DfracOwn (1/2)} 0) ∗ own idcntrG_name (●{DfracOwn (1/2)} 0))%I.
-Proof.
-  iMod (own_alloc (● 0 ⋅ ◯ 0)) as (γ) "[Hauth _]"; [admit|].
-  set (H1 := IdcntrG _ _ γ).
-  iExists _.
-  by iDestruct "Hauth" as "[$ $]".
-Admitted. *)
-
-(* Lemma state_alloc `{inG Σ stateUR} :
-  ⊢ |==> ∃ _ : stateG Σ, (own stateG_name (● (∅, ∅)))%I.
-Proof.
-  iMod (own_alloc ((● (∅, ∅)) : stateUR)) as (γ) "Hst"; [admit|].
-  by iExists (StateG _ _ γ).
-Admitted. *)
 
 Definition poisonOSR := authUR (optionUR (optionUR (agree unitUR))).
 Class poisonOSG Σ := PoisonOSG { poisonOS_inG :> inG Σ poisonOSR; poisonOSG_name : gname }.
+
+Definition idcntrUR := authUR nat.
+Class idcntrG Σ := IdcntrG { idcntr_inG :> inG Σ idcntrUR; idcntrG_name : gname }.
 
 Lemma pos_alloc `{inG Σ poisonOSR} :
   ⊢ |==> ∃ _ : poisonOSG Σ, 
@@ -61,23 +22,33 @@ Proof.
   set (H1 := PoisonOSG _ _ γ).
   iExists _. by iFrame.
 Admitted.
+
+Lemma idcntr_alloc `{inG Σ idcntrUR} :
+  ⊢ |==> ∃ _ : idcntrG Σ, 
+      (own idcntrG_name (●{DfracOwn (1/2)} 0) ∗ 
+      own idcntrG_name (●{DfracOwn (1/2)} 0))%I.
+Proof.
+  iMod (own_alloc (● 0 ⋅ ◯ 0)) as (γ) "[Hauth _]"; [admit|].
+  set (H1 := IdcntrG _ _ γ).
+  iExists _.
+  by iDestruct "Hauth" as "[$ $]".
+Admitted.
   
 Section proof.
-  Context `{!authG Σ, !seqG Σ, !poisonOSG Σ}.
+  Context `{!authG Σ, !seqG Σ, !poisonOSG Σ, !idcntrG Σ}.
 
-  Definition authBaseN : namespace := nroot .@ "susp_ver".
-  Definition gmapN : namespace := authBaseN .@ "gmap".
+  Definition authBaseN : namespace := nroot .@ "susp_sec".
   Definition tableN : namespace := authBaseN .@ "table".
-  Definition tableLocSet : namespace := authBaseN .@ "tableloc".
-  Definition tableLocN (susp : val) : namespace := tableLocSet .@ susp.
 
-  (* Definition msize_auth (n : nat) : iProp Σ :=
-    own msizeG_name (●{DfracOwn (1/2)} n) ∗ own msizeG_name (◯ n).
-  Definition msize_frag (n : nat) : iProp Σ :=
-    own msizeG_name (●{DfracOwn (1/2)} n). *)
+  Local Notation s_is_ser_proph := (s_is_ser_proph authBaseN).
+  Local Notation ser_spec_un := (ser_spec_un authBaseN).
+  Local Notation ser_spec_3 := (ser_spec_3 authBaseN).
+  Local Notation count_spec := (count_spec authBaseN).
+  Local Notation val_eq_rel := (val_eq_rel authBaseN).
 
-  (* Definition idcntr_frag (n : nat) := own idcntrG_name (●{DfracOwn (1/2)} n). *)
-
+  Local Notation lrel_evidence := (lrel_evidence authBaseN).
+  Local Notation lrel_auth := (lrel_auth authBaseN).
+  
   Definition pos_car := optionUR (optionUR (agree unitUR)).
 
   Definition pos (o : pos_car) := own poisonOSG_name (●{DfracOwn (1/2)} o).
@@ -91,18 +62,8 @@ Section proof.
   Definition bad_pos_frag := pos_frag (Some None).
   Definition done_pos_frag := pos_frag (Some (Some (to_agree ()))).
 
-  Local Notation s_is_ser_proph := (s_is_ser_proph authBaseN).
-  Local Notation ser_spec_un := (ser_spec_un authBaseN).
-  Local Notation ser_spec_3 := (ser_spec_3 authBaseN).
-  Local Notation count_spec := (count_spec authBaseN).
-  Local Notation val_eq_rel := (val_eq_rel authBaseN).
+  Definition id_frag (id : nat) := own idcntrG_name (●{DfracOwn (1/2)} id).
 
-  Local Notation lrel_evidence := (lrel_evidence authBaseN).
-  Local Notation lrel_auth := (lrel_auth authBaseN).
-
-  (* Lemma get_frag (o : pos_car) :
-    pos o -∗ pos o ∗ pos_frag o.
-  Proof. Admitted. *)
 
   Lemma pos_agree (o o' : pos_car) :
     pos o -∗ pos o' -∗ ⌜o' = o⌝ ∗ pos o ∗ pos o'.
@@ -120,174 +81,57 @@ Section proof.
     bad_pos -∗ bad_pos ==∗ done_pos ∗ done_pos ∗ done_pos_frag.
   Proof. Admitted.
 
-
-  (* Definition proph_type : Type := nat * option unit.
-
-  Definition proph_cond (v : proph_type) (pid : nat) : iProp Σ :=
-    (∀ (m : parentUR), ∃ (x av : val) (t : evi_type),
-        ⌜v = (pid, Some tt)⌝ ∗ val_eq t x av ∗
-          ⌜m !! pid = Some (to_agree (t, x))⌝) ∨
-      (⌜v = (pid, None)⌝).
-
-  Fixpoint take_until {A B : Type} (f : A → option B) (xs : list A) : list B :=
-    match xs with
-    | []      => []
-    | x :: xs =>
-      match f x with
-      | Some y => y :: (take_until f xs)
-      | None   => []
-      end
-    end.
-
-  Definition longest_valid_prefix (us : list val) : list proph_type :=
-    take_until (λ u,
-        match u with
-          (#(LitInt v), SOMEV #())%V => if Z.geb v 0 then Some (Z.to_nat v, Some ()) else None
-        | (#(LitInt v), NONEV)%V => if Z.geb v 0 then Some (Z.to_nat v, None) else None
-        | _ => None
-        end
-      ) us.
-
-  Definition proph_list (p : proph_id) (vs : list (nat * option unit)) : iProp Σ :=
-    ∃ (us : list (val * val)),
-      proph p us ∗ ⌜vs = longest_valid_prefix (map snd us)⌝
-        ∗ [∗ list] k↦v ∈ vs, (∃ (pid : nat), proph_cond v pid).
-
-  Definition option_unit_val (v : option unit) : val :=
-    match v with Some _ => SOMEV #() | None => NONEV end.
   
-  Lemma wp_resolve_proph_val_some p vs (pid : nat) :
-    ∀ x av t (m : parentUR),
-      {{{ proph_list p vs ∗ val_eq t x av ∗ ⌜m !! pid = Some (to_agree (t, x))⌝ }}}
-        resolve_proph: #p to: (#pid, SOMEV #())%V
-      {{{ vs', RET #(); ⌜vs = (pid, Some tt) :: vs'⌝ ∗ proph_list p vs' }}}.
-  Proof.
-    iIntros (???? Φ) "((%us & Hp & % & Hcon) & Heq & %Hmap) HΦ".
-    wp_apply (wp_resolve_proph with "Hp").
-    iIntros (us') "[% Hp]". simplify_eq.
-    iApply "HΦ". iFrame "Hp". iSplit; [|iSplit; [done|]].
-    - iPureIntro. simpl.
-      rewrite /longest_valid_prefix. simpl.
-      assert ((pid >=? 0)%Z = true).
-      { rewrite Z.geb_le. lia. }
-      rewrite H. do 2 f_equal. lia.
-    - iSimpl in "Hcon".
-      rewrite /longest_valid_prefix.
-      assert ((pid >=? 0)%Z = true).
-      { rewrite Z.geb_le. lia. }
-      simpl. rewrite H. simpl.
-      iDestruct "Hcon" as "[H1 Hcon]". iFrame.
-  Qed.
-  
-  Lemma wp_resolve_proph_val_none p vs (pid : nat) :
-    {{{ proph_list p vs }}}
-      resolve_proph: #p to: (#pid, NONEV)%V;;
-      resolve_proph: #p to: NONEV
-    {{{ RET #(); ⌜vs = [(pid, None)]⌝ }}}.
-  Proof.
-    iIntros (Φ) "(%us & Hp & %) HΦ".
-    wp_apply (wp_resolve_proph with "Hp").
-    iIntros (?) "[% Hp]". wp_pures.
-    wp_apply (wp_resolve_proph with "Hp").
-    iIntros (?) "[% Hp]". iApply "HΦ".
-    simplify_eq. iPureIntro.
-    rewrite /longest_valid_prefix /option_unit_val.
-    simpl; f_equal.
-    assert ((pid >=? 0)%Z = true).
-    { rewrite Z.geb_le. lia. }
-    rewrite H. do 2 f_equal. lia.
-  Qed.
+  Lemma id_agree id id' :
+    id_frag id -∗ id_frag id' -∗ ⌜id = id'⌝ ∗ id_frag id ∗ id_frag id'.
+  Proof. Admitted.
 
-  Lemma wp_resolve_proph_final p vs (v : option unit) :
-    {{{ proph_list p vs }}}
-      resolve_proph: #p to: (#0, option_unit_val v)%V;;
-      resolve_proph: #p to: NONEV
-    {{{ RET #(); ⌜vs = [(0, v)]⌝ }}}.
-  Proof.
-    iIntros (Φ) "(%us & Hp & %) HΦ".
-    wp_apply (wp_resolve_proph with "Hp").
-    iIntros (?) "[% Hp]". wp_pures.
-    wp_apply (wp_resolve_proph with "Hp").
-    iIntros (?) "[% Hp]". iApply "HΦ".
-    simplify_eq. iPureIntro.
-    rewrite /longest_valid_prefix /option_unit_val.
-    destruct v; simpl; [destruct u|]; f_equal.
-  Qed. *)
+  Lemma id_update id id':
+    id_frag id -∗ id_frag id ==∗ id_frag id' ∗ id_frag id'.
+  Proof. Admitted.
 
-  (* map size is always > 1, if poison value then finish returns none *)
 
   Definition finish_spec1 (finish : val) (x a ser : val) : iProp Σ :=
-    ∀ (s s' : string) (E: coPset) (t : evi_type),
+    ∀ (E: coPset) (s s' : string) (t : evi_type),
       ⌜↑authSet authBaseN ⊆ E⌝ -∗
       {{{ seq_tok E ∗ s_is_ser_proph t x s' ∗ ser_spec_3 ser t ∗
           ⌜a = InjLV #s⌝ }}}
-            (* ser_spec_3 ser t  ∗
-            val_eq_rel authBaseN (lrel_bi_bin A) ∗ val_eq_rel_un authBaseN (lrel_bi_un A) ∗ *)
-            (* s_is_ser'' t' aᵥ s ∗ ⌜a = InjLV #(hash s)⌝ }}} *)
         finish #()
-        {{{ (o : option val), RET $o;
-        (* We might prophesy that the filled-in value is the correct one,
-           But it is still possible that the value isn't actually filled. *)
-            seq_tok E (* ∗ if o is None then True else A x aᵢ *) }}}.
-
-  (* Definition finish_spec1_dc (finish : val) (x a ser : val) (A : lrel_un Σ) : iProp Σ :=
-    ∀ (s s' : string) (E: coPset) (t : evi_type),
-      ⌜↑authSet authBaseN ⊆ E⌝ -∗
-      {{{ seq_tok E ∗ s_is_ser_proph t x s' ∗ ser_spec_3 ser t ∗
-          ⌜a = InjLV #s⌝ }}}
-            (* ser_spec_3 ser t  ∗
-            val_eq_rel authBaseN (lrel_bi_bin A) ∗ val_eq_rel_un authBaseN (lrel_bi_un A) ∗ *)
-            (* s_is_ser'' t' aᵥ s ∗ ⌜a = InjLV #(hash s)⌝ }}} *)
-        finish #()
-        {{{ (o : option val), RET $o;
-        (* We might prophesy that the filled-in value is the correct one,
-           But it is still possible that the value isn't actually filled. *)
-            seq_tok E ∗ if o is None then True else A x aᵢ }}}. *)
+        {{{ (o : option val), RET $o; seq_tok E }}}.
 
   Definition finish_spec1_bad (finish : val) (x a ser : val) : iProp Σ :=
-    ∀ (s s' : string) (E: coPset) (t : evi_type),
+    ∀ (E: coPset) (s s' : string) (t : evi_type),
       ⌜↑authSet authBaseN ⊆ E⌝ -∗
       {{{ seq_tok E ∗ s_is_ser_proph t x s' ∗ ser_spec_3 ser t ∗
           hashed s ∗ ⌜a = InjLV #(hash s)⌝ ∗ ⌜s ≠ s'⌝ }}}
-            (* ser_spec_3 ser t  ∗
-            val_eq_rel authBaseN (lrel_bi_bin A) ∗ val_eq_rel_un authBaseN (lrel_bi_un A) ∗ *)
-            (* s_is_ser'' t' aᵥ s ∗ ⌜a = InjLV #(hash s)⌝ }}} *)
         finish #()
         {{{ (o : option val), RET $o; seq_tok E ∗ ⌜o = None⌝ }}}.
 
   Definition finish_spec2 (finish : val) (x a ser : val) : iProp Σ :=
-    ∀ (s' s'' : string) (E: coPset) (t : evi_type) (susp : loc) (o' : pos_car),
+    ∀ (E: coPset) (s' s'' : string) (t : evi_type) (susp : loc) (o' : pos_car),
       ⌜↑authSet authBaseN ⊆ E ∧ ↑tableN ⊆ E⌝ -∗
       {{{ seq_tok E ∗ s_is_ser_proph t x s' ∗ ser_spec_3 ser t ∗ valid_pos o' ∗ 
           ⌜a = InjRV #susp⌝ ∗ seq_inv (authN authBaseN susp) (auth_inv s'' susp) }}}
-            (* ser_spec_3 ser t  ∗
-            val_eq_rel authBaseN (lrel_bi_bin A) ∗ val_eq_rel_un authBaseN (lrel_bi_un A) ∗ *)
-            (* s_is_ser'' t' aᵥ s ∗ ⌜a = InjLV #(hash s)⌝ }}} *)
         finish #()
         {{{ (o : option val), RET $o;
-        (* We might prophesy that the filled-in value is the correct one,
-           But it is still possible that the value isn't actually filled. *)
             seq_tok E ∗ (if o is Some _ then pos o' else True) }}}.
 
   Definition finish_spec2_bad (finish : val) (x a ser : val) : iProp Σ :=
-    ∀ (s s' s'' : string) (E: coPset) (t : evi_type) (susp : loc),
+    ∀ (E: coPset) (s s' s'' : string) (t : evi_type) (susp : loc),
       ⌜↑authSet authBaseN ⊆ E⌝ -∗
       {{{ seq_tok E ∗ s_is_ser_proph t x s' ∗ ser_spec_3 ser t ∗
           ⌜a = InjRV #susp⌝ ∗ ⌜s'' = some_ser_str (string_ser_str (hash s))⌝ ∗ 
           hashed s ∗ seq_inv (authN authBaseN susp) (auth_inv s'' susp) ∗ ⌜s ≠ s'⌝ }}}
-            (* ser_spec_3 ser t  ∗
-            val_eq_rel authBaseN (lrel_bi_bin A) ∗ val_eq_rel_un authBaseN (lrel_bi_un A) ∗ *)
-            (* s_is_ser'' t' aᵥ s ∗ ⌜a = InjLV #(hash s)⌝ }}} *)
         finish #()
         {{{ (o : option val), RET $o; seq_tok E ∗ ⌜o = None⌝ }}}.
 
-  Definition good_finish_specs (m : gmap val val) finish x a ser : iProp Σ :=
+  Definition good_finish_specs finish x a ser : iProp Σ :=
     ((∃ (s : string), ⌜a = InjLV #s⌝ ∗ finish_spec1 finish x a ser) ∨ 
       (∃ s'' (susp : loc), ⌜a = InjRV #susp⌝ ∗
         seq_inv (authN authBaseN susp) (auth_inv s'' susp) ∗
         finish_spec2 finish x a ser)).
 
-  Definition bad_finish_specs (m : gmap val val) finish x a ser s s' : iProp Σ :=
+  Definition bad_finish_specs finish x a ser s s' : iProp Σ :=
     ((⌜a = InjLV #(hash s)⌝ ∗ hashed s ∗ 
         (finish_spec1_bad finish x a ser ∧ ⌜s ≠ s'⌝)) ∨ 
       (∃ s'' (susp : loc), ⌜a = InjRV #susp⌝ ∗ hashed s ∗
@@ -295,196 +139,31 @@ Section proof.
         seq_inv (authN authBaseN susp) (auth_inv s'' susp) ∗
           (finish_spec2_bad finish x a ser ∧ ⌜s ≠ s'⌝))).
 
+
   Definition susp_big_sep (m : gmap val val) : iProp Σ :=
     [∗ map] k ↦ v ∈ m,
       ∃ (ctr : nat) (finish x a ser : val) (t : evi_type) (s' : string),
         (⌜ctr > 0 ∧ v = (#ctr, finish)%V⌝ ∗ 
             s_is_ser_proph t x s' ∗ ser_spec_3 ser t ∗
-            (good_finish_specs m finish x a ser ∨
-              (∃ s, bad_pos_frag ∗ bad_finish_specs m finish x a ser s s'))).
+            (good_finish_specs finish x a ser ∨
+              (∃ s, bad_pos_frag ∗ bad_finish_specs finish x a ser s s'))).
 
   Definition susp_bad_ge1 (m : gmap val val) : iProp Σ :=
     good_pos ∨ done_pos ∨
-      (bad_pos ∗ ⌜map.map_length m > 0⌝).
-        (* (∃ (k v : val) (ctr : nat) finish x a ser t s s', 
-          ⌜map_Exists (λ k' v', v = v' ∧ k = k') m⌝ ∗
-          ⌜ctr > 0 ∧ v = (#ctr, finish)%V⌝ ∗ 
-            s_is_ser_proph t x s' ∗ ser_spec_3 ser t ∗
-            bad_finish_specs m finish x a ser s s')). *)
+      (bad_pos ∗ 
+        ∃ (pid ctr : nat) (v finish x a ser : val) (t : evi_type) (s s' : string),
+        ⌜m !! #pid = Some v ∧ ctr > 0 ∧ v = (#ctr, finish)%V⌝ ∗
+          s_is_ser_proph t x s' ∗ ser_spec_3 ser t ∗
+          bad_finish_specs finish x a ser s s').
       
   Definition is_susp_table (l : loc) : iProp Σ :=
-    ∃ (d : val) (m : gmap val val),
-      l ↦ d ∗ ⌜is_map d m⌝ ∗ susp_big_sep m ∗ susp_bad_ge1 m.
-
-  (* Definition in_susp_table (l : loc) (id : nat) : iProp Σ :=
-    ∃ (d v : val) (m : gmap val val) (s : nat),
-      is_susp_table l -∗ l ↦ d ∗ ⌜is_map d m⌝
-      -∗ is_susp_table l ∗ ⌜m !! #id = Some v⌝.
-
-  Definition not_in_susp_table (l : loc) (id : nat) : iProp Σ :=
-    ∃ (d : val) (m : gmap val val) (s : nat),
-      is_susp_table l -∗ l ↦ d ∗ ⌜is_map d m s⌝
-      -∗ is_susp_table l ∗ ⌜m !! #id = None⌝. *)
+    ∃ (d : val) (m : gmap val val) (ctr : nat),
+      l ↦ d ∗ ⌜is_map d m⌝ ∗ susp_big_sep m ∗ susp_bad_ge1 m ∗
+      id_frag ctr ∗ ⌜∀ ctr', ctr' ≥ ctr → m !! #ctr' = None⌝.
 
   Definition inv_susp_table (l: loc) := seq_inv tableN (is_susp_table l).
 
-  (* Lemma idcntr_update (cnt : nat) :
-    idcntr_frag cnt ∗ idcntr_frag cnt ==∗ idcntr_frag (cnt + 1) ∗ idcntr_frag (cnt + 1).
-  Proof. Admitted.
-
-  Lemma idcntr_agree (cnt cnt' : nat) :
-    idcntr_frag cnt ∗ idcntr_frag cnt' -∗ ⌜cnt = cnt'⌝ ∗ idcntr_frag cnt ∗ idcntr_frag cnt'.
-  Proof. Admitted. *)
-
-  (* Definition count_inv (cnt : nat) (m : mapUR) (lm : locPidMapUR) :=
-    ∀ (id : nat),
-      id ≥ cnt →
-      (m !! id = None ∧
-         (∀ (l : loc), lm !! l = None ∨
-                         (∀ id', lm !! l = Some id' → id ≠ id'))).
   
-  Definition global_state (cnt : nat) (m : mapUR) (lm : locPidMapUR) : iProp Σ :=
-    own stateG_name (● (m, lm)) ∗ idcntr_frag cnt ∗
-      ⌜count_inv cnt m lm⌝ ∗
-      (∀ (id : nat) (x vᵥ : val) (l : loc) (t : evi_type),
-          ⌜m !! id = Some (to_agree (t, x, vᵥ, (None : option loc), true))⌝ -∗
-            (in_susp_table l id ∨ (not_in_susp_table l id ∗ val_eq t x vᵥ))).
-  
-  Definition empty_state : prodUR mapUR locPidMapUR := (∅, ∅).
-
-  Lemma init_global_state :
-    idcntr_frag 0 ==∗ global_state 0 ∅ ∅.
-  Proof.
-    iIntros "Hfrag".
-    iFrame.
-    iMod state_alloc as (γs) "Hst".
-
-    iModIntro. iSplitL; [admit|].
-    iSplit.
-    { iPureIntro. intros ??. split; first done.
-      intros ?. by left. }
-    iIntros (??????). done.
-  Admitted.
-  
-  Lemma global_state_update_empty (cnt : nat) (m : mapUR) (lm : locPidMapUR) :
-    global_state cnt m lm ∗ idcntr_frag cnt ==∗ global_state (cnt+1) m lm ∗ idcntr_frag (cnt+1).
-  Proof.
-    iIntros "((Hst & Hcntfrag & %Hcntinv & Hseminv) & Hcntauth)".
-    
-    iCombine "Hcntauth Hcntfrag" as "Hfull".
-    iMod (own_update with "Hfull") as "[Hfull _]".
-    { apply (auth_update _ 0 (cnt+1) 1).
-      apply (nat_local_update _ _ (cnt+1)).
-      lia. }
-
-  Admitted.
-
-  Definition singleton_map (id : nat) (t : evi_type) (x vᵥ : val) (so : option loc) (b : bool) : mapUR :=
-    {[ id := to_agree (t, x, vᵥ, so, b) ]}.
-
-  Definition single_instance_frag (id : nat) (t : evi_type) (x vᵥ : val) (so : option loc) (b : bool) : stateUR :=
-    ◯ (singleton_map id t x vᵥ so b, if so is Some s then {[ s := id ]} else ∅).
-
-  Definition updated_map (m : mapUR) (id : nat) (t : evi_type) (x vᵥ : val) (so : option loc) (b : bool) : mapUR :=
-    <[ id := to_agree (t, x, vᵥ, so, b) ]> m.
-
-  Definition updated_loc_map (m : locPidMapUR) (so : option loc) (id : nat) : locPidMapUR :=
-    if so is Some s then <[ s := id ]> m else m.
-
-  Lemma global_state_update_singleton (cnt : nat) (m : mapUR) (lm : locPidMapUR) (t : evi_type) (x vᵥ : val) (so : option loc) (b : bool) :
-    global_state cnt m lm ∗ idcntr_frag cnt
-    ==∗ global_state (cnt + 1) (updated_map m cnt t x vᵥ so b) (updated_loc_map lm so cnt) ∗ single_instance cnt t x vᵥ so b ∗ idcntr_frag (cnt + 1).
-  Proof.
-    iIntros "((Hst & Hcntfrag & %Hcntinv & Hseminv) & Hcntauth)".
-    iMod ((own_update
-             stateG_name
-             (● (m, lm))
-             (● (updated_map m cnt t x vᵥ so b, updated_loc_map lm so cnt) ⋅ single_instance_frag cnt t x vᵥ so b))
-           with "Hst") as "Hst".
-    { apply (auth_update _ empty_state _ _).
-      apply prod_local_update; simpl.
-      { apply gmap.alloc_local_update; last done.
-        apply Hcntinv. lia. }
-      destruct so; last done.
-      admit. }
-    iPoseProof (own_op with "Hst") as "[Hst Hfrag]".
-
-    iCombine "Hcntauth Hcntfrag" as "Hfull".
-    iMod (own_update with "Hfull") as "[Hfull _]".
-    { apply (auth_update _ 0 (cnt+1) 1).
-      apply (nat_local_update _ _ (cnt+1)).
-      lia. }
-
-    iAssert (idcntr_frag (cnt + 1) ∗ idcntr_frag (cnt + 1))%I with "[Hfull]" as "[H1 H2]".
-    { admit. }
-
-    iModIntro.
-    iSplitR "H2 Hfrag"; [|iFrame].
-
-    rewrite /global_state.
-    iFrame. iSplitR "Hseminv".
-    iPureIntro.
-    { intros id H. rewrite /updated_map.
-      rewrite lookup_insert_None.
-      split; last admit.
-      split; last lia.
-      apply Hcntinv. lia. }
-    iIntros (?????).
-    iSpecialize ("Hseminv" $! id x0 vᵥ0 l t0) as #.
-    iIntros (?). iApply "Hseminv".
-  Admitted.
-
-  Lemma msize_agree (s s' : nat) :
-    msize_auth s ∗ msize_frag s' -∗ ⌜s = s'⌝ ∗ msize_auth s ∗ msize_frag s'.
-  Proof.
-    iIntros "[[Hauth1 Hfrag] Hauth2]".
-    iCombine "Hauth1 Hauth2" as "Hauth".
-    iDestruct (own_valid with "Hauth") as "%H".
-    move: H => /auth_auth_dfrac_op_inv ->.
-
-    iDestruct "Hauth" as "[Hauth1 Hauth2]". by iFrame.
-  Qed.
-
-  Lemma msize_update (s s': nat) :
-    msize_auth s ∗ msize_frag s ==∗ msize_auth s' ∗ msize_frag s'.
-  Proof.
-    iIntros "[[Hauth1 Hfrag] Hauth2]".
-    iCombine "Hauth1 Hauth2" as "Hauth".
-    iMod (own_update_2 with "Hauth Hfrag") as "[Hauth Hfrag]".
-    { apply (auth_update s s s' s').
-      apply nat_local_update. lia. }
-
-    iDestruct "Hauth" as "[Hauth1 Hauth2]".
-    by iFrame.
-  Qed.
-    
-  Lemma idcntr_agree (cnt cnt' : nat) :
-    ∀ m lm, global_state cnt m lm ∗ idcntr_frag cnt'
-            -∗ ⌜cnt = cnt'⌝ ∗ global_state cnt m lm ∗ idcntr_frag cnt.
-  Proof.
-    iIntros (??) "[(? & Hcntfrag & ?) Hidauth]".
-    iCombine "Hcntfrag Hidauth" as "Hfull".
-    iDestruct (own_valid with "Hfull") as "%H".
-    move: H => /auth_auth_dfrac_op_inv H.
-    rewrite H.
-
-    iDestruct "Hfull" as "[Hcntfrag Hidauth]".
-    by iFrame.
-  Qed. *)
-    
-(*  Definition proph_list (vs : val) : iProp Σ :=
-    ∃ (m: gmap int proph_id),
-      ([∗ map] id ↦ p ∈ m, ∃ ( 
-
-  Definition resolves (i : nat) : iProp Σ := True.
-
-  Fixpoint is_fine (A : lrel Σ) (anc_exist : bool) (v1 v2 anc1 anc2 : val) (pid : int) : iProp Σ :=
-    ∃ (anc_exist : bool) (anc1 anc2 : val) (pid : int)
-    if anc then
-      resolves pid -∗ is_fine A 
-    else
-      .*)
-
   Lemma v_finish_spec1 :
     ∀ (a x ser : val) (st : loc),
       {{{ True }}}
@@ -508,14 +187,6 @@ Section proof.
     case_bool_decide; simplify_eq; wp_pures.
     - iApply ("HΦ" $! (Some _)); by iFrame "∗ #".
     - iApply ("HΦ" $! None); by iFrame "∗ #".
-
-    (* iPoseProof "HA" as "[HA_bin HA_un]".
-    iMod ("Hrel_bin" with "[//] Htok [Hsers] Hser HA_bin") as "[Htok HA'_bin]".
-    { by iLeft. }
-    iMod ("Hrel_un" with "[//] Htok [Hsers] Hser HA_un") as "[Htok HA'_un]".
-    { by iLeft. }
-
-    iApply ("HΦ" $! (Some _)). by iFrame "∗ #". *)
   Qed.
 
   Lemma v_finish_spec1_bad :
@@ -538,20 +209,9 @@ Section proof.
     iIntros "(Htok & #[[% Hsers]|%])"; simplify_eq; wp_pures;
     wp_apply (wp_hash); try done;
     iIntros "#hashs'"; wp_pures;
-    case_bool_decide; simplify_eq; wp_pures;
-
-    destruct (decide (collision s s')) as [|Hnc%not_collision];
-      try (iExFalso; by iApply (hashes_auth.hashed_inj_or_coll with "hashs hashs'") );
-    destruct Hnc as [<-|?]; simplify_eq.
+    case_bool_decide; simplify_eq; wp_pures.
+    { iPoseProof (hashes_auth.hashed_s_equal s s' with "[//] hashs hashs'") as "->". done. }
     iApply ("HΦ" $! None); by iFrame "∗ #".
-
-    (* iPoseProof "HA" as "[HA_bin HA_un]".
-    iMod ("Hrel_bin" with "[//] Htok [Hsers] Hser HA_bin") as "[Htok HA'_bin]".
-    { by iLeft. }
-    iMod ("Hrel_un" with "[//] Htok [Hsers] Hser HA_un") as "[Htok HA'_un]".
-    { by iLeft. }
-
-    iApply ("HΦ" $! (Some _)). by iFrame "∗ #". *)
   Qed.
 
   Lemma v_finish_spec2 :
@@ -592,7 +252,7 @@ Section proof.
       wp_apply (typed_proph_wp_resolve1 StringTypedProph with "Hproph"); try done.
       wp_pures. iModIntro. iIntros (?). wp_pures.
 
-      iDestruct "Htabo" as (??) "(Hl & %Hm & Hbigsep & Hge)".
+      iDestruct "Htabo" as (???) "(Hl & %Hm & Hbigsep & Hge & Hid)".
       wp_apply wp_hash; try done; iIntros "_"; wp_pures; wp_store.
       iMod (pointsto_persist with "Hsusp") as "#Hsusp".
 
@@ -603,98 +263,158 @@ Section proof.
       { iMod ("Hclose" with "[$Htok]") as "Htok".
         { iNext. iLeft. iFrame "#". iSplit; eauto.
           iRight. repeat iExists _. iSplit; eauto. }
-        iMod ("Hclose_tab" with "[$Hl $Hbigsep $Htok $Hge //]") as "Htok".
+        iMod ("Hclose_tab" with "[$Hl $Hbigsep $Htok $Hge $Hid //]") as "Htok".
         iApply ("HΦ" $! None). by iFrame. }
 
-      iDestruct (big_sepM_lookup_acc with "Hbigsep") as "[[% Hs] Hbigsep]"; [done|subst].
-      iDestruct "Hs" as (?????? Hv) 
-        "(#Hser' & #Hserspec' & [#Hfinish|(%&Hfrag&#Hfinish)])"; last first;
-        destruct! Hv; simplify_eq; wp_pures.
-      + destruct Ho' as [-> | ->];
-        iPoseProof (pos_auth_frag_valid with "Hpos Hfrag") as (?) "[Hpos #Hfrag]";
-        simplify_eq; first admit; clear H2.
-        iDestruct "Hge" as "[Hpos'|[Hpos'|[Hpos' %Hge]]]";
-          iPoseProof (pos_agree with "Hpos Hpos'") as (?) "[Hpos Hpos']"; 
-          simplify_eq.
+      iDestruct (big_sepM_lookup_acc with "Hbigsep") as "[[% #Hs] Hbigsep]"; [done|subst].
+      iDestruct "Hs" as (?????? Hv) "Hs"; destruct! Hv; simplify_eq; wp_pures.
+      case_bool_decide; simplify_eq; wp_pures; wp_load;
+        wp_bind (map_remove _ _); wp_apply (gwp_map_remove with "[//]");
+        try done; iIntros (??); wp_store; wp_pures;
+        iPoseProof ("Hbigsep" with "[$Hs]") as "Hbigsep";
+          try (iFrame; iExists ctr0; iSplit; try done; iRight; iFrame "#");
+        iDestruct (big_sepM_delete _ m #pid ((#ctr0, finish)%V) with "Hbigsep")
+          as "[_ Hbigsep']"; try done;
+        destruct Ho' as [-> | ->];
+          iDestruct "Hge" as "[Hpos'|[Hpos'|[Hpos' Hge]]]";
+          iPoseProof (pos_agree with "Hpos Hpos'") as (?) "[Hpos Hpos']";
+        iDestruct "Hs" as 
+          "(#Hser' & #Hserspec' & [#Hfinish|(%& Hfrag &#Hfinish)])";
+          simplify_eq;
+        iMod ("Hclose" with "[$Htok]") as "Htok";
+          try (iNext; iLeft; iFrame "hashs' #"; iSplit; eauto;
+              iRight; repeat iExists _; iSplit; eauto).
 
-        case_bool_decide; simplify_eq; wp_pures; wp_load;
-          wp_bind (map_remove _ _); wp_apply (gwp_map_remove with "[//]");
-          try done; iIntros (??); wp_store; wp_pures;
-          iPoseProof ("Hbigsep" with "[$Hser' $Hserspec' $Hfinish]") as "Hbigsep";
-            try (iFrame; iExists ctr; iSplit; try done; iRight; iFrame "#");
-          iDestruct (big_sepM_delete _ m #pid ((#ctr, finish)%V) with "Hbigsep")
-            as "[_ Hbigsep']"; try done.
-        * iMod (pos_update2 with "Hpos Hpos'") as "(Hpos & Hpos' & _)".
-          iMod ("Hclose" with "[$Htok]") as "Htok";
-          try (iNext; iLeft; iFrame "hashs' #"; iSplit; eauto;
-                iRight; repeat iExists _; iSplit; eauto);
-          iMod ("Hclose_tab" with "[$Hl $Hbigsep' $Htok Hpos']") as "Htok";
-          try (iNext; iSplit; try done; iRight; by iLeft).
-          iDestruct "Hfinish" as 
-            "[(%&#hashs&[Hfinish %])|(%&%&%&#hashs&%&#Hinv'&[Hfinish %])]";
-          wp_apply ("Hfinish" with "[] [$Htok]");
-          try solve_ndisj; iFrame "# ∗"; eauto;
-          iIntros (?) "[Htok ->]"; iApply ("HΦ" $! None); by iFrame.
-        * wp_load; wp_pures; wp_bind (map.map_insert _ _ _);
+      2,6:
+        iPoseProof (pos_auth_frag_valid with "Hpos Hfrag") as (Hincl) "[Hpos #Hfrag']";
+        simplify_eq; apply option_included in Hincl; destruct! Hincl; simplify_eq.
+
+      4,5,6:
+        wp_load; wp_pures; wp_bind (map.map_insert _ _ _);
           wp_apply (gwp_map_insert with "[//]"); try done;
-          iIntros (??); wp_store;
-          iDestruct (big_sepM_insert _ (delete #pid m) #pid ((#(ctr-1), finish)%V) with "[$Hbigsep']")
-            as "Hbigsep''"; try apply lookup_delete; iFrame "#".
-          { iExists (ctr-1). iPureIntro. split; repeat f_equal; try lia. admit. }
-          iMod ("Hclose" with "[$Htok]") as "Htok";
-            try (iNext; iLeft; iFrame "hashs' #"; iSplit; eauto;
-                  iRight; repeat iExists _; iSplit; eauto).
-          iMod ("Hclose_tab" with "[$Hl $Hbigsep'' $Htok Hpos']") as "Htok"; iFrame "%".
-          { iNext. do 2 iRight. iFrame. admit. }
-          iModIntro; iApply ("HΦ" $! (Some _)); by iFrame.
-      + case_bool_decide; simplify_eq; wp_pures; wp_load;
-          wp_bind (map_remove _ _); wp_apply (gwp_map_remove with "[//]");
-          try done; iIntros (??); wp_store; wp_pures;
-          iPoseProof ("Hbigsep" with "[$Hser' $Hserspec']") as "Hbigsep";
-            repeat (iExists _); try (iSplit). 1,4: admit.
-          1,3: by iLeft.
-        all:
-          iDestruct "Hfinish" as 
-            "[(%&%&Hfinish)|(%&%&%&#Hinv'&Hfinish)]";
-          iDestruct (big_sepM_delete _ m #pid ((#ctr, finish)%V) with "Hbigsep")
-            as "[_ Hbigsep]"; try done.
-        1,2: (* First branch of the if *)
-          iMod ("Hclose" with "[$Htok]") as "Htok";
-          try (iNext; iLeft; iFrame "hashs' #"; iSplit; eauto;
-                iRight; repeat iExists _; iSplit; eauto);
-          destruct Ho' as [-> | ->];
-            iDestruct "Hge" as "[Hpos'|[Hpos'|[Hpos' %Hge]]]";
-            iPoseProof (pos_agree with "Hpos Hpos'") as (?) "[Hpos Hpos']"; 
-            simplify_eq;
-          iMod ("Hclose_tab" with "[$Hl $Hbigsep $Htok Hpos']") as "Htok";
-            try (iFrame "%"; iNext; iFrame; eauto; admit).
-          1,2: 
-            wp_apply ("Hfinish" with "[//] [$Htok $Hser' $Hserspec' //]");
-            iIntros (?) "Htok"; iApply "HΦ"; iFrame; destruct o; eauto;
-              try (by iLeft); by iRight.
-          1,2: 
-            wp_apply ("Hfinish" with "[//] [$Htok $Hser' $Hserspec' $Hinv' $Hpos]");
-              eauto.
-        all: (* else branch *)
-          wp_load; wp_pures; wp_bind (map.map_insert _ _ _);
-          wp_apply (gwp_map_insert with "[//]"); try done;
-          iIntros (??); wp_store;
-          iDestruct (big_sepM_insert _ (delete #pid m) #pid ((#(ctr-1), finish)%V) with "[$Hbigsep]")
-            as "Hbigsep"; try apply lookup_delete;
-          try (iFrame "Hser' Hserspec'"); repeat iExists _; try (iSplit). 1,4: admit.
-        1,3 : iLeft; iFrame "#"; eauto.
-        all:
-          iMod ("Hclose" with "[$Htok]") as "Htok";
-          try (iNext; iLeft; iFrame "hashs' #"; iSplit; eauto;
-                iRight; repeat iExists _; iSplit; eauto);
-          destruct Ho' as [-> | ->];
-            iDestruct "Hge" as "[Hpos'|[Hpos'|[Hpos' %Hge]]]";
-            iPoseProof (pos_agree with "Hpos Hpos'") as (?) "[Hpos Hpos']"; 
-            simplify_eq;
-          iMod ("Hclose_tab" with "[$Hl $Hbigsep $Htok Hpos']") as "Htok";
-            try (iFrame "%"; iNext; iFrame; eauto; admit);
-          iModIntro; iApply ("HΦ" $! (Some _)); by iFrame.
-  Admitted.
+          iIntros (??); wp_store.
+
+      + iMod ("Hclose_tab" with "[$Hl $Hbigsep' $Htok Hpos' Hid]") as "Htok".
+        { iNext. iExists ctr. iSplit; iFrame; try done.
+          iDestruct "Hid" as "[$ %]". iPureIntro.
+          intros ??. rewrite lookup_delete_None. eauto. }
+        iDestruct "Hfinish" as "[(%&%&Hfinish)|(%&%&%&#Hinv'&Hfinish)]".
+        { wp_apply ("Hfinish" with "[//] [$Htok $Hser' $Hserspec' //]").
+          iIntros (?) "Htok"; iApply "HΦ". iFrame. destruct o; eauto. }
+        { wp_apply ("Hfinish" with "[//] [$Htok $Hser' $Hserspec' Hpos]");
+          iFrame "# ∗"; eauto. }
+
+      + iDestruct "Hge" as (?????????? ?) "Hge". destruct! H4.
+
+        destruct (decide (#pid = #pid0)); simplify_eq.
+        { iMod (pos_update2 with "Hpos Hpos'") as "(Hpos & Hpos' & _)".
+          iMod ("Hclose_tab" with "[$Hl $Hbigsep' $Htok Hpos' Hid]") as "Htok".
+          { iNext. iExists ctr. iSplit; iFrame; try done.
+            iDestruct "Hid" as "[$ %]". iPureIntro.
+            intros ??. rewrite lookup_delete_None. eauto. }
+          iClear "#".
+          iDestruct "Hge" as  "(Hser1 & Hser1' & Hfinish1)".
+          iDestruct "Hfinish1" as "[(%&#hashs&[Hfinish %])|(%&%&%&#hashs&%&#Hinv'&[Hfinish %])]";
+            wp_apply ("Hfinish" with "[//] [$Htok $Hser1 $Hser1' $hashs]"); eauto;
+            iIntros (?) "[Htok ->]"; iApply ("HΦ" $! None); by iFrame. }
+
+        destruct (size (delete #pid m)) as [|size] eqn:Hsize.
+        { rewrite map_size_empty_iff in Hsize.
+          eassert (delete #pid m !! #pid0 = Some _).
+          { rewrite lookup_delete_Some /=. eauto. }
+          rewrite Hsize in H6. done. }
+
+        iMod ("Hclose_tab" with "[$Hl $Hbigsep' Hge $Htok Hpos' Hid]") as "Htok"; iFrame "%".
+        { iNext. iExists ctr. iSplitL "Hpos' Hge".
+          { do 2 iRight. iFrame "∗ # %". iExists pid0, ctr1, _. iPureIntro.
+            by rewrite (lookup_delete_ne _ _ _ n). }
+          iDestruct "Hid" as "[$ %]". iPureIntro.
+          intros ??. rewrite lookup_delete_None. eauto. }
+        iDestruct "Hfinish" as "[(%&%&Hfinish)|(%&%&%&#Hinv'&Hfinish)]".
+        { wp_apply ("Hfinish" with "[//] [$Htok $Hser' $Hserspec' //]").
+          iIntros (?) "Htok"; iApply "HΦ". iFrame. destruct o; eauto. }
+        { wp_apply ("Hfinish" with "[//] [$Htok $Hser' $Hserspec' Hpos]");
+          iFrame "# ∗"; eauto. }
+
+      + iMod (pos_update2 with "Hpos Hpos'") as "(Hpos & Hpos' & _)".
+        iMod ("Hclose_tab" with "[$Hl $Hbigsep' $Htok Hpos' Hid]") as "Htok".
+        { iNext. iExists ctr. iSplit; iFrame; try done.
+          iDestruct "Hid" as "[$ %]". iPureIntro.
+          intros ??. rewrite lookup_delete_None. eauto. }
+        iDestruct "Hfinish" as 
+          "[(%&#hashs&[Hfinish %])|(%&%&%&#hashs&%&#Hinv'&[Hfinish %])]";
+        wp_apply ("Hfinish" with "[] [$Htok]");
+        try solve_ndisj; iFrame "# ∗"; eauto;
+        iIntros (?) "[Htok ->]"; iApply ("HΦ" $! None); by iFrame.
+
+      + iDestruct (big_sepM_insert _ (delete #pid m) #pid ((#(ctr0-1), finish)%V) with "[$Hbigsep']")
+          as "Hbigsep'"; try apply lookup_delete;
+          try (iFrame "Hser' Hserspec'"); try (iExists (ctr0-1)); repeat iExists _;
+          try iSplit; 
+            try (iPureIntro; split; repeat f_equal; try lia;
+              inversion H1; try lia; by simplify_eq);
+            try (by iLeft).
+        iMod ("Hclose_tab" with "[$Hl $Hbigsep' $Htok Hpos' Hid]") as "Htok".
+        { iNext. iExists ctr. iSplit; iFrame; try done.
+          iDestruct "Hid" as "[$ %]". iPureIntro.
+          intros ??. rewrite lookup_insert_None.
+          destruct (decide (#pid = #ctr')); simplify_eq.
+          { specialize (H5 ctr' H6) as H5'. simplify_eq. }
+          rewrite lookup_delete_ne; eauto. }
+        iApply ("HΦ" $! (Some _)); iModIntro. iFrame.
+
+      + iDestruct (big_sepM_insert _ (delete #pid m) #pid ((#(ctr0-1), finish)%V) with "[$Hbigsep']")
+          as "Hbigsep'"; try apply lookup_delete;
+          try (iFrame "Hser' Hserspec'"); try (iExists (ctr0-1)); repeat iExists _;
+          try iSplit; 
+            try (iPureIntro; split; repeat f_equal; try lia;
+              inversion H1; try lia; by simplify_eq);
+            try (by iLeft).
+        iMod ("Hclose_tab" with "[$Hl $Hbigsep' $Htok Hge Hpos' Hid]") as "Htok".
+        { iNext. iExists ctr. iSplit; try done. 
+          iSplitL "Hge Hpos'".
+          { do 2 iRight; iFrame.
+            iDestruct "Hge" as (?????????? ?) "$". 
+            destruct! H5. simplify_eq.
+            destruct (decide (#pid = #pid0)); simplify_eq.
+            { iExists pid0, (ctr0-1), _. iPureIntro.
+              rewrite lookup_insert_Some. split; eauto.
+              split; repeat f_equal; try lia.
+              inversion H1; try lia. by simplify_eq. }
+            { iExists pid0, ctr1, _. iPureIntro.
+              rewrite (lookup_insert_ne _ _ _ _ n).
+              rewrite lookup_delete_Some /=. split; eauto. } }
+          iDestruct "Hid" as "[$ %]". iPureIntro.
+          intros ??. rewrite lookup_insert_None.
+          destruct (decide (#pid = #ctr')); simplify_eq.
+          { specialize (H5 ctr' H6) as H5'. simplify_eq. }
+          rewrite lookup_delete_ne; eauto. }
+
+        iApply ("HΦ" $! (Some _)); iModIntro. iFrame.
+
+      + iDestruct (big_sepM_insert _ (delete #pid m) #pid ((#(ctr0-1), finish)%V) with "[$Hbigsep']")
+          as "Hbigsep'"; try apply lookup_delete;
+          try (iFrame "Hser' Hserspec'"); try (iExists (ctr0-1)); repeat iExists _;
+          try iSplit;
+            try (iPureIntro; split; repeat f_equal; try lia;
+              inversion H1; try lia; by simplify_eq);
+            try (iRight; iFrame "#").
+        iMod ("Hclose_tab" with "[$Hl $Hbigsep' $Htok Hpos' Hid]") as "Htok".
+        { iNext; iExists ctr; iSplit; try done. 
+          iSplitL "Hpos'".
+          { do 2 iRight; iFrame "# ∗".
+            iExists pid, (ctr0-1), _. iPureIntro.
+            rewrite lookup_insert_Some. split; eauto.
+            split; repeat f_equal; try lia.
+            inversion H1; try lia. by simplify_eq. }
+          iDestruct "Hid" as "[$ %]". iPureIntro.
+          intros ??. rewrite lookup_insert_None.
+          destruct (decide (#pid = #ctr')); simplify_eq.
+          { specialize (H5 ctr' H6) as H5'. simplify_eq. }
+          rewrite lookup_delete_ne; eauto. }
+
+        iApply ("HΦ" $! (Some _)); iModIntro. iFrame.
+  Qed.
 
   Lemma v_finish_spec2_bad :
     ∀ (a x ser : val) (st : loc),
@@ -707,7 +427,7 @@ Section proof.
     rewrite /v_finish.
     wp_pures. iModIntro. iApply "HΦ".
     rewrite /finish_spec1.
-    iIntros (s s' s'' ????).
+    iIntros (? s s' s'' ???).
     iIntros (?) "!# (Htok & #Hser & #Hserspec & % & % & #hashs & #Hinv & %) HΦ".
     wp_pures. wp_apply ("Hserspec" with "[//] [$Hser $Htok]").
     iIntros ([]); last first.
@@ -717,27 +437,22 @@ Section proof.
     iMod (na_inv_acc with "Hinv Htok") as "(Hinv1 & Htok & Hclose)"; [solve_ndisj|solve_ndisj|].
     iDestruct "Hinv1" as ">[(%s1&%& #hashs1 & %& #Hsusp & %Hser)|(%&%&%& Hsusp & Hproph & %Hser)]";
       wp_load; wp_pures; destruct! Hser; simplify_eq.
-    - assert (s = s1) as ->; first admit.
+    - iPoseProof (hashes_auth.hashed_s_equal s s1 with "[//] hashs hashs1") as "->".
       iMod ("Hclose" with "[$Htok]") as "Htok".
       { iNext. iLeft. iFrame "#". iSplit; eauto. 
         iRight. repeat iExists _. iSplit; eauto. }
       wp_apply wp_hash; try done;
       iIntros "#hashs'"; wp_pures;
-      case_bool_decide; simplify_eq; wp_pures;
-
-      destruct (decide (collision s' s1)) as [|Hnc%not_collision];
-        try (iExFalso; by iApply (hashes_auth.hashed_inj_or_coll with "hashs' hashs1") );
-      destruct Hnc as [<-|?]; simplify_eq.
+      case_bool_decide; simplify_eq; wp_pures.
+      { by iPoseProof (hashes_auth.hashed_s_equal s' s1 with "[//] hashs' hashs1") as "->".  }
       iApply ("HΦ" $! None); by iFrame "∗ #".
     
     - wp_apply wp_hash; try done; iIntros "#hashs'"; wp_pures.
       wp_apply (typed_proph_wp_resolve1 StringTypedProph with "Hproph"); try done.
       wp_pures. iModIntro. iIntros (?). wp_pures.
+      by iPoseProof (hashes_auth.hashed_s_equal s' s with "[//] hashs' hashs") as "->".
+  Qed.
 
-      destruct (decide (collision s s')) as [|Hnc%not_collision];
-        try (iExFalso; by iApply (hashes_auth.hashed_inj_or_coll with "hashs hashs'") );
-      destruct Hnc as [<-|?]; simplify_eq.
-  Admitted.
 
   Definition is_proof (v : val) : iProp Σ :=
     ∃ (l : list string), ⌜is_list l v⌝.
@@ -756,12 +471,12 @@ Section proof.
   Definition lrel_bin_auth_comp' (A : lrel_bi Σ) : lrel Σ := LRel (λ v1 v2,
     ∀ t K (w w' : val) (cntr : nat),
       {{{ spec_ideal t (fill K (v2 w')) ∗ seq_tok ⊤ ∗ 
-          is_proof_state w cntr ∗ good_pos }}}
+          is_proof_state w cntr ∗ good_pos ∗ id_frag cntr }}}
         v1 w
       {{{ (o1 : option val), RET $o1;
           seq_tok ⊤ ∗
             if o1 is Some w1 then
-              ∃ (a prfst prf : val) (cntr' : nat),
+              ∃ (a prfst prf : val) (cntr' : nat), id_frag cntr' ∗
                  ⌜w1 = (prfst, a)%V ∧ prfst = (prf, #cntr')%V⌝ ∗
                   ((∃ (w2 : val), spec_ideal t (fill K w2) ∗ 
                     lrel_auth_comp_post A w1 w2 ∗ good_pos) ∨ 
@@ -770,24 +485,15 @@ Section proof.
 
   Definition lrel_un_auth_comp' (A_un : lrel_un Σ) : lrel_un Σ := LRelUn (λ v1,
     ∀ (w : val) (cntr : nat),
-      {{{ seq_tok ⊤ ∗ is_proof_state w cntr ∗ bad_pos }}}
+      {{{ seq_tok ⊤ ∗ is_proof_state w cntr ∗ bad_pos ∗ id_frag cntr }}}
         v1 w
       {{{ (o1 : option val), RET $o1;
           seq_tok ⊤ ∗
             if o1 is Some w1 then
-              ∃ (a prfst prf : val) (cntr' : nat),
+              ∃ (a prfst prf : val) (cntr' : nat), id_frag cntr' ∗
                 ⌜w1 = (prfst, a)%V ∧ prfst = (prf, #cntr')%V⌝ ∗
                   lrel_auth_comp_post_bad A_un w1 ∗ bad_pos
             else True }}})%I.
-
-  (* Definition lrel_auth_comp_bad : lrel Σ := LRel (λ v1 v2,
-    ∀ w,
-      {{{ seq_tok ⊤ ∗ is_proof_state w }}}
-        v1 w
-      {{{ (o1 : option val), RET $o1;
-          seq_tok ⊤ ∗
-            if o1 is Some w1 then lrel_auth_comp_post_bad w1 v2
-            else True }}})%I. *)
 
   Definition lrel_auth_comp' (A : lrel_bi Σ) : lrel_bi Σ :=
     LRelBi (lrel_un_auth_comp' (lrel_bi_un A)) (lrel_bin_auth_comp' A).
@@ -795,19 +501,10 @@ Section proof.
   Program Definition lrel_auth_comp : kindO Σ (⋆ ⇒ ⋆)%kind := λne A, lrel_auth_comp' A.
   Next Obligation.
     intros ????. split; [intros ?|intros ??];
-      rewrite /lrel_car/= /lrel_un_car/= /lrel_un_auth_comp' /lrel_bin_auth_comp';
-      do 25 f_equiv; first solve_proper.
-    do 10 f_equiv; solve_proper.
+      rewrite /lrel_car/= /lrel_un_car/= /lrel_un_auth_comp' /lrel_bin_auth_comp'.
+    do 27 f_equiv; first solve_proper.
+    do 37 f_equiv; solve_proper.
   Qed.
-
-  (* Definition lrel_hash_fail_option' (A : lrel Σ) : lrel Σ := LRel (λ v1 v2,
-    (A v1 v2 ∨ (∃ x, A x v2)))%I.
-
-  Program Definition lrel_hash_fail_option : kindO Σ (⋆ ⇒ ⋆)%kind := λne A, lrel_hash_fail_option' A.
-  Next Obligation.
-    intros ??????. rewrite /lrel_car /=.
-    solve_proper.
-  Qed.    *)
   
   Definition auth_ctx {Θ} (Δ : ctxO Σ Θ) := ext (ext Δ lrel_auth) lrel_auth_comp.
 
@@ -817,10 +514,10 @@ Section proof.
   Proof.
     iIntros "#HA".
     rewrite interp_var1_ext2.
-    iIntros (?? Ψ) "!# (Htok & %H & ?) HΨ".
+    iIntros (?? Ψ) "!# (Htok & %H & Hpos & Hid) HΨ".
     simpl in H. destruct H as (? & -> & Hp).
     wp_pures. iModIntro. iApply ("HΨ" $! (Some _)).
-    iFrame "Htok". iExists _, _, _, _.
+    iFrame. do 3 iExists _.
     iSplit; first done. iFrame.
     iExists _, _. iFrame "HA".
     iExists _. iSplit; [done|]. rewrite /is_proof_state.
@@ -843,12 +540,11 @@ Section proof.
         iModIntro. iFrame. clear.
         iSplit; interp_unfold!.
         { rewrite interp_var1_ext2.
-          iIntros (????? Ψ) "!# (Hi & Htok & %H & ?) HΨ".
+          iIntros (????? Ψ) "!# (Hi & Htok & %H & Hpos & Hid) HΨ".
           simpl in H. destruct H as (? & -> & Hp).
           i_pures; wp_pures.
           iModIntro. iApply ("HΨ" $! (Some _)).
-          iFrame "Htok".
-          iExists _, _, _, _.
+          iFrame. iExists _, _, _.
           iSplit; first done. iFrame.
           iLeft. iFrame. iExists _, _.
           iFrame "HA".
@@ -882,14 +578,14 @@ Section proof.
   Proof.
     iIntros "#HmA #HmB".
     rewrite interp_var2_ext3. 
-    iIntros (???Ψ) "!# (Htok & #Hprf & Hpos) HΨ". wp_pures.
+    iIntros (?? Ψ) "!# (Htok & #Hprf & Hpos & Hid) HΨ". wp_pures.
     wp_pures. wp_bind (v _)%I.
-    wp_apply ("HmA" with "[$Htok $Hprf $Hpos]").
+    wp_apply ("HmA" with "[$Htok $Hprf $Hpos $Hid]").
     iIntros (o) "[Htok Ho]".
     destruct o; last first.
     { wp_pures. iApply ("HΨ" $! None). by iFrame. }
     iPoseProof "Hprf" as (??) "Hprf'". 
-    iDestruct "Ho" as (????[??]) "[(%&%&%&%& #Hprf1 & HA) Hpos]".
+    iDestruct "Ho" as (????) "(Hid & [%%] & [(%&%&%&%& #Hprf1 & HA) Hpos])".
     iPoseProof "Hprf1" as (??) "Hprf1'". 
     simplify_eq. wp_pures.
     rewrite interp_un_arr_unfold.
@@ -899,8 +595,8 @@ Section proof.
     iIntros (?) "(H & Htok) /=".
     interp_unfold in "H".
     rewrite interp_var2_ext3.
-    wp_apply ("H" with "[$Htok $Hprf1 $Hpos]").
-    iIntros (?) "(Htok & Ho) /=".
+    wp_apply ("H" with "[$Htok $Hprf1 $Hpos $Hid]").
+    iIntros (o) "[Htok Ho] /=".
     iApply "HΨ". iFrame.
   Qed.
 
@@ -932,15 +628,15 @@ Section proof.
             interp_unfold in "HmA".
             iSplit; interp_unfold!.
             { rewrite interp_var2_ext3.
-              iIntros (u1 u2 ??? Ψ) "!# (Hi & Htok & Hprf & Hpos) HΨ".
+              iIntros (u1 u2 ??? Ψ) "!# (Hi & Htok & Hprf & Hpos & Hid) HΨ".
               i_pures; wp_pures.
               i_bind (v2 _)%I; wp_bind (v1 _)%I.
               iDestruct "HmA" as "[HmA _]".
-              wp_apply ("HmA" with "[$Hi $Htok $Hprf $Hpos]").
+              wp_apply ("HmA" with "[$Hi $Htok $Hprf $Hpos $Hid]").
               iIntros (o) "[Htok Ho]".
               destruct o; last first.
               { wp_pures. iApply ("HΨ" $! None). by iFrame. }
-              iDestruct "Ho" as (????) "(%H & [H|H])".
+              iDestruct "Ho" as (????) "(Hid & %H & [H|H])".
               + iDestruct "H" as (?) "(Hi & H & Hpos)".
                 iDestruct "H" as (? a1' a2 ->) "[#Hprf #HA]".
                 wp_pures.
@@ -954,7 +650,7 @@ Section proof.
                 iPoseProof "Hprf" as (??) "Hprf'". simplify_eq.
                 interp_unfold in "H". rewrite interp_var2_ext3.
                 iDestruct "H" as "[H _]".
-                wp_apply ("H" with "[$Hi $Htok $Hprf $Hpos]").
+                wp_apply ("H" with "[$Hi $Htok $Hprf $Hpos $Hid]").
                 iIntros (?) "(Htok & Ho) /=".
                 iApply "HΨ". iFrame.
               + iDestruct "H" as "[H Hpos]".
@@ -971,13 +667,12 @@ Section proof.
                 destruct! H. simplify_eq.
                 iPoseProof "Hprf" as (??) "Hprf'". simplify_eq.
                 rewrite interp_var2_ext3.
-                wp_apply ("H" with "[$Htok $Hprf $Hpos]").
+                wp_apply ("H" with "[$Htok $Hprf $Hpos $Hid]").
                 iIntros (?) "(Htok & Ho) /=".
                 iApply "HΨ". iFrame.
                 destruct o1; last done. iFrame.
-                iDestruct "Ho" as (????[??]) "Hbad".
-                iExists _, _, _, _. iSplit; first done.
-                iFrame. }
+                iDestruct "Ho" as (????) "($ & % & $)".
+                eauto. }
             { iDestruct "HmA" as "[_ HmA]".
               iDestruct "HmB" as "[_ HmB]".
               iApply (refines_un_auth_bind with "HmA HmB"). } }
@@ -1065,7 +760,7 @@ Section proof.
         end)%V.
   Proof.
     iIntros (??????) "#Htab #Hser' #Hser3 #Hcount #Hdeser #Hauth_un".
-    iIntros (???) "!# (Htok & Hproof & Hpos) HΦ".
+    iIntros (???) "!# (Htok & Hproof & Hpos & Hid) HΦ".
     wp_pures.
     iDestruct "Hproof" as (? -> ) "Hproof".
     wp_pures. iDestruct "Hproof" as "(% & %)".
@@ -1092,68 +787,67 @@ Section proof.
       + wp_bind (finish #()).
         assert (c0 = 0); [lia|]. simplify_eq.
 
-        iApply ("Hfinish" $! _ _ ⊤ with "[//] [$Htok $Hserproph $Hser3 //]").
+        iMod (na_inv_acc with "Htab Htok") as "(Htabo & Htok & Hclose_tab)"; [solve_ndisj|solve_ndisj|].
+        iDestruct "Htabo" as (???) "(Hl & >%Hm & Hbigsep & Hge & >Hid' & >%Hidinv)".
+
+        iPoseProof (id_agree with "Hid Hid'") as (->) "[Hid Hid']".
+        iMod (id_update _ (ctr+1) with "Hid Hid'") as "[Hid Hid']".
+
+        iMod ("Hclose_tab" with "[$Htok $Hl $Hbigsep $Hge $Hid']") as "Htok".
+        { iNext. iFrame "%". iPureIntro. intros ??. apply Hidinv. lia. }
+
+        iApply ("Hfinish" $! ⊤ with "[//] [$Htok $Hserproph $Hser3 //]").
         iNext. iIntros ([]) "Htok"; wp_pures; last first.
         { iApply ("HΦ" $! (None)). by iFrame. }
 
         wp_apply gwp_list_tail; [done|].
-        iIntros (vl Hl).
-
-        (* iMod (na_inv_acc with "Htab Htok") as "(Htabo & Htok & Hclose_tab)"; [solve_ndisj|solve_ndisj|]. *)
-        (* iDestruct "Htabo" as (??) "(Hl & >%Hm & Hbigsep)". *)
-        wp_pures.
-
-        (* iPoseProof (idcntr_agree with "[$Hid $Hfrag]") as (->) "[Hid Hfrag]".
-        iMod (idcntr_update with "[$Hid $Hfrag]") as "[Hid Hfrag]". *)
-
-        (* iPoseProof (idcntr_agree with "[$Hst $Hfrag]") as (->) "[Hst Hfrag]".
-        iMod (global_state_update_empty with "[$Hst $Hfrag]") as "[Hst Hfrag]". *)
-        
-        (* iMod ("Hclose_tab" with "[$Hl $Hbigsep $Htok]") as "Htok"; try done. *)
-        (* { iFrame "%". iPureIntro. intros ?. apply Hci. lia. } *)
+        iIntros (vl Hl). wp_pures.
         
         iApply ("HΦ" $! (Some _)).
-
         iFrame "# ∗"; iModIntro; repeat (iExists _);
-          iSplit; try (iSplit; try done; iPureIntro; repeat f_equal; 
-            instantiate (1 := cntr + 1); lia);
-          iFrame "# ∗ %"; iExists _, (cntr+1);
+          iSplit; try (iSplit; try done; iPureIntro; repeat f_equal; lia); 
+          iFrame "# ∗ %"; iExists _, (ctr+1);
           iSplit; iPureIntro; repeat f_equal; lia.
 
       + iMod (na_inv_acc with "Htab Htok") as "(Htabo & Htok & Hclose_tab)"; [solve_ndisj|solve_ndisj|].
-        iDestruct "Htabo" as (??) "(Hl & >%Hm & Hbigsep & Hge)". wp_load.
+        iDestruct "Htabo" as (???) "(Hl & >%Hm & Hbigsep & Hge & Hid' & >%Hidinv)". wp_load.
 
-        (* iPoseProof (idcntr_agree with "[$Hst $Hfrag]") as (->) "[Hst Hfrag]".
-        iPoseProof (msize_agree with "[$Hms $Hs]") as (<-) "[Hms Hs]".
-        iMod (global_state_update_singleton with "[$Hst $Hfrag]") as "(Hst & Hins & Hfrag)". *)
-        (* iPoseProof (idcntr_agree with "[$Hid $Hfrag]") as (->) "[Hid Hfrag]".
-        iMod (idcntr_update with "[$Hid $Hfrag]") as "[Hid Hfrag]". *)
+        iPoseProof (id_agree with "Hid Hid'") as (->) "[Hid Hid']".
+        iMod (id_update _ (ctr+1) with "Hid Hid'") as "[Hid Hid']".
 
-        (* assert (m0 !! #c1 = None). { apply Hci. lia. } *)
-        wp_bind (map.map_insert _ _ _). wp_pures.
-        iApply (gwp_map_insert #cntr (#c0, finish)%V d m _ _); [done|done|].
+        wp_pures. wp_bind (map.map_insert _ _ _).
+        wp_apply (gwp_map_insert #ctr); try done.
         
-        iModIntro. iIntros (d') "%Hmap'". wp_store.
-        (* iMod (msize_update _ (s+1) with "[$Hms $Hs]") as "[Hms Hs]". *)
+        iIntros (d') "%Hmap'". wp_store.
         wp_pures. wp_apply (gwp_list_tail with "[//]").
         iIntros "/=" (tl Htl). wp_pures.
-        iDestruct "Hge" as "[Hpos'|[Hpos'|[Hpos' %Hge]]]";
+        iDestruct "Hge" as "[Hpos'|[Hpos'|[Hpos' Hge]]]";
           iPoseProof (pos_agree with "Hpos Hpos'") as (?) "[Hpos Hpos']"; 
           simplify_eq.
 
-        iMod ("Hclose_tab" with "[$Hl Hbigsep Hpos' $Htok Hfinish]") as "Htok".
-        { iNext. iExists _. iSplit; try done. iSplit; last admit.
-          iApply (big_sepM_insert_2 with "[Hfinish]"); last done.
-          assert (c0 > 0).
-          { apply Nat.neq_0_lt_0. intros ->. by apply H0. }
-          repeat iExists _. repeat (try (iSplit; eauto)).
-          do 2 iLeft. iFrame. eauto. }
+        iMod ("Hclose_tab" with "[$Hl Hbigsep Hpos' $Htok Hfinish Hge $Hid']") as "Htok".
+        { iNext. iExists _. iSplit; try done. 
+          iSplit; [|iSplitL "Hpos' Hfinish Hge"].
+          { iApply (big_sepM_insert_2 with "[Hfinish]"); last done.
+            assert (c0 > 0).
+            { apply Nat.neq_0_lt_0. intros ->. by apply H0. }
+            repeat iExists _. repeat (try (iSplit; eauto)).
+            do 2 iLeft. iFrame. eauto. }
+          { iDestruct "Hge" as (?????????? Hv) "Hge".
+            destruct! Hv. simplify_eq.
+            do 2 iRight. iFrame. iExists pid, ctr0, _.
+            destruct (decide (#ctr = #pid)); simplify_eq.
+            { specialize (Hidinv pid ltac:(lia)). simplify_eq. }
+            iPureIntro. rewrite lookup_insert_ne; eauto. }
+          iPureIntro. intros ??.
+          specialize (Hidinv ctr' ltac:(lia)).
+          rewrite lookup_insert_None. split; eauto.
+          intros ?. simplify_eq. lia. }
 
         iApply ("HΦ" $! (Some _)).
         iFrame "# ∗"; iModIntro; repeat (iExists _);
-          iSplit; try (iSplit; try done; iPureIntro; repeat f_equal; 
-            instantiate (1 := cntr + 1); lia);
-          iFrame "# ∗ %"; iExists _, (cntr+1);
+          iSplit; try (iSplit; try done; iPureIntro; repeat f_equal; lia); 
+          iFrame "# ∗ %"; iExists _, (ctr+1);
           iSplit; iPureIntro; repeat f_equal; lia.
     
     - wp_apply (v_finish_spec2 with "Htab").
@@ -1162,72 +856,70 @@ Section proof.
       case_bool_decide; wp_pures; simplify_eq.
       * wp_bind (finish #()).
         assert (c0 = 0); [lia|]. simplify_eq.
+
+        iMod (na_inv_acc with "Htab Htok") as "(Htabo & Htok & Hclose_tab)"; [solve_ndisj|solve_ndisj|].
+        iDestruct "Htabo" as (???) "(Hl & >%Hm & Hbigsep & Hge & >Hid' & >%Hidinv)".
+
+        iPoseProof (id_agree with "Hid Hid'") as (->) "[Hid Hid']".
+        iMod (id_update _ (ctr+1) with "Hid Hid'") as "[Hid Hid']".
+
+        iMod ("Hclose_tab" with "[$Htok $Hl $Hbigsep $Hge $Hid']") as "Htok".
+        { iNext. iFrame "%". iPureIntro. intros ??. apply Hidinv. lia. }
         
-        iApply ("Hfinish" $! _ _ ⊤ tA' with "[//] [$Htok $Hserproph $Hser3 $Hinv $Hpos]"); eauto.
+        iApply ("Hfinish" $! ⊤ with "[//] [$Htok $Hserproph $Hser3 $Hinv $Hpos]"); eauto.
         iNext. iIntros ([]) "[Htok Hpos]"; wp_pures; last first.
         { iApply ("HΦ" $! (None)). eauto. }
 
         wp_apply gwp_list_tail; [done|].
-        iIntros (vl Hl).
-
-        (* iMod (na_inv_acc with "Htab Htok") as "(Htabo & Htok & Hclose_tab)"; [solve_ndisj|solve_ndisj|]. *)
-        (* iDestruct "Htabo" as (??) "(Hl & >%Hm & Hbigsep)". *)
-        wp_pures.
-
-        (* iPoseProof (idcntr_agree with "[$Hid $Hfrag]") as (->) "[Hid Hfrag]".
-        iMod (idcntr_update with "[$Hid $Hfrag]") as "[Hid Hfrag]". *)
-
-        (* iPoseProof (idcntr_agree with "[$Hst $Hfrag]") as (->) "[Hst Hfrag]".
-        iMod (global_state_update_empty with "[$Hst $Hfrag]") as "[Hst Hfrag]". *)
-        
-        (* iMod ("Hclose_tab" with "[$Hl $Hbigsep $Htok]") as "Htok"; try done. *)
-        (* { iFrame "%". iIntros (id). iPureIntro. intros ?. apply Hci. lia. } *)
+        iIntros (vl Hl). wp_pures.
         
         iApply ("HΦ" $! (Some _)).
-
         iFrame "# ∗"; iModIntro; repeat (iExists _);
-          iSplit; try (iSplit; try done; iPureIntro; repeat f_equal; 
-            instantiate (1 := cntr + 1); lia);
-          iFrame "# ∗ %". iExists _, (cntr+1);
+          iSplit; try (iSplit; try done; iPureIntro; repeat f_equal; lia); 
+          iFrame "# ∗ %"; iExists _, (ctr+1);
           iSplit; iPureIntro; repeat f_equal; lia.
       
       * iMod (na_inv_acc with "Htab Htok") as "(Htabo & Htok & Hclose_tab)"; [solve_ndisj|solve_ndisj|].
-        iDestruct "Htabo" as (??) "(Hl & >%Hm & Hbigsep & Hge)". wp_load.
+        iDestruct "Htabo" as (???) "(Hl & >%Hm & Hbigsep & Hge & Hid' & >%Hidinv)". wp_load.
 
-        (* iPoseProof (idcntr_agree with "[$Hst $Hfrag]") as (->) "[Hst Hfrag]".
-        iPoseProof (msize_agree with "[$Hms $Hs]") as (<-) "[Hms Hs]".
-        iMod (global_state_update_singleton with "[$Hst $Hfrag]") as "(Hst & Hins & Hfrag)". *)
-        (* iPoseProof (idcntr_agree with "[$Hid $Hfrag]") as (->) "[Hid Hfrag]".
-        iMod (idcntr_update with "[$Hid $Hfrag]") as "[Hid Hfrag]". *)
+        iPoseProof (id_agree with "Hid Hid'") as (->) "[Hid Hid']".
+        iMod (id_update _ (ctr+1) with "Hid Hid'") as "[Hid Hid']".
 
-        (* assert (m0 !! #c1 = None). { apply Hci. lia. } *)
         wp_bind (map.map_insert _ _ _). wp_pures.
-        iApply (gwp_map_insert #cntr (#c0, finish)%V d m _ _); [done|done|].
+        iApply (gwp_map_insert #ctr (#c0, finish)%V d m _ _); [done|done|].
         
         iModIntro. iIntros (d') "%Hmap'". wp_store.
-        (* iMod (msize_update _ (s+1) with "[$Hms $Hs]") as "[Hms Hs]". *)
         wp_pures. wp_apply (gwp_list_tail with "[//]").
         iIntros "/=" (tl Htl). wp_pures.
-        iDestruct "Hge" as "[Hpos'|[Hpos'|[Hpos' %Hge]]]";
+        iDestruct "Hge" as "[Hpos'|[Hpos'|[Hpos' Hge]]]";
           iPoseProof (pos_agree with "Hpos Hpos'") as (?) "[Hpos Hpos']"; 
           simplify_eq.
 
-        iMod ("Hclose_tab" with "[$Hl Hbigsep Hpos' $Htok Hfinish]") as "Htok".
-        { iNext. iExists _. iSplit; try done. iSplit; last admit.
-          iApply (big_sepM_insert_2 with "[Hfinish]"); last done.
-          assert (c0 > 0).
-          { apply Nat.neq_0_lt_0. intros ->. by apply H0. }
-          repeat iExists _. repeat (try (iSplit; [done|])).
-          iLeft. iRight. by iFrame "# ∗". }
+        iMod ("Hclose_tab" with "[$Hl Hbigsep Hpos' $Htok Hfinish Hge $Hid']") as "Htok".
+        { iNext. iExists _. iSplit; try done. 
+          iSplit; [|iSplitL "Hpos' Hfinish Hge"].
+          { iApply (big_sepM_insert_2 with "[Hfinish]"); last done.
+            assert (c0 > 0).
+            { apply Nat.neq_0_lt_0. intros ->. by apply H0. }
+            repeat iExists _. repeat (try (iSplit; eauto)).
+            iLeft. iRight. iFrame. eauto. }
+          { iDestruct "Hge" as (?????????? Hv) "Hge".
+            destruct! Hv. simplify_eq.
+            do 2 iRight. iFrame. iExists pid, ctr0, _.
+            destruct (decide (#ctr = #pid)); simplify_eq.
+            { specialize (Hidinv pid ltac:(lia)). simplify_eq. }
+            iPureIntro. rewrite lookup_insert_ne; eauto. }
+          iPureIntro. intros ??.
+          specialize (Hidinv ctr' ltac:(lia)).
+          rewrite lookup_insert_None. split; eauto.
+          intros ?. simplify_eq. lia. }
 
         iApply ("HΦ" $! (Some _)).
-
         iFrame "# ∗"; iModIntro; repeat (iExists _);
-          iSplit; try (iSplit; try done; iPureIntro; repeat f_equal; 
-            instantiate (1 := cntr + 1); lia);
-          iFrame "# ∗ %"; iExists _, (cntr+1);
+          iSplit; try (iSplit; try done; iPureIntro; repeat f_equal; lia); 
+          iFrame "# ∗ %"; iExists _, (ctr+1);
           iSplit; iPureIntro; repeat f_equal; lia.
-  Admitted.
+  Qed.
 
   Lemma refines_auth_unauth Θ (Δ : ctxO Σ Θ) c :
     inv_susp_table c
@@ -1258,14 +950,14 @@ Section proof.
           iDestruct "Hauth_bi" as "[(% & -> & Hauth_bi)|->]"; wp_pures; last first.
           { iFrame. iModIntro.
             interp_unfold!. rewrite interp_var2_ext3. iSplit.
-            { iIntros (??????) "!# (Hi & Htok & Hproof & Hpos) HΦ".
+            { iIntros (??????) "!# (Hi & Htok & Hproof & Hpos & Hid) HΦ".
               wp_pures. iApply ("HΦ" $! None). by iFrame. }
             iIntros (???) "!# (Htok & Hproof & Hpos) HΦ".
             wp_pures. iApply ("HΦ" $! None). by iFrame. }
           iDestruct "Hauth_un" as "[(% & % & Hauth_un)|->]"; last first.
           { iFrame. iModIntro.
             interp_unfold!. rewrite interp_var2_ext3. iSplit.
-            { iIntros (??????) "!# (Hi & Htok & Hproof & Hpos) HΦ".
+            { iIntros (??????) "!# (Hi & Htok & Hproof & Hpos & Hid) HΦ".
               wp_pures. iApply ("HΦ" $! None). by iFrame. }
             iIntros (???) "!# (Htok & Hproof & Hpos) HΦ".
             wp_pures. iApply ("HΦ" $! None). by iFrame. }
@@ -1275,7 +967,7 @@ Section proof.
           simplify_eq.
           iFrame. iModIntro.
           iSplit; interp_unfold!; rewrite interp_var2_ext3.
-          { iIntros (??????) "!# (Hi & Htok & Hproof & Hpos) HΦ".
+          { iIntros (??????) "!# (Hi & Htok & Hproof & Hpos & Hid) HΦ".
             wp_pures. i_pures. iDestruct "Hproof" as (? -> ) "Hproof".
             wp_pures. iDestruct "Hproof" as "(% & %)".
             wp_apply gwp_list_head; [done| ].
@@ -1292,10 +984,10 @@ Section proof.
             iPoseProof "Hauth_bi" as "(%&%&%&#hashs1&#Hser1&#HA&[%|(%&%&%&%&#Hinv)])";
               simplify_eq; iIntros "[Hserser Hserproph]";
               iPoseProof ("Hserproph" with "Hserser") as ">[#HA_un [%s2 #Hserproph]]";
-              wp_pures; wp_apply ("Hcount" $! _ _ ⊤ with "[//] [$Hserproph $Htok]");
+            wp_pures; wp_apply ("Hcount" $! _ _ ⊤ with "[//] [$Hserproph $Htok]");
               iIntros (?) "[_ Htok]"; wp_pures.
-            - (* iPoseProof (deser_ser_proph authBaseN with "[$Htok $Hserser]") as ">[Htok [% Hserproph]]". *)
-              destruct (decide (s2 = s1)); simplify_eq; last first.
+
+            - destruct (decide (s2 = s1)); simplify_eq; last first.
 
               + wp_apply v_finish_spec1_bad; try done.
                 iIntros (finish) "Hfinish". wp_pures.
@@ -1304,40 +996,49 @@ Section proof.
                 * wp_bind (finish #()).
                   assert (c0 = 0); [lia|]. simplify_eq.
 
-                  iApply ("Hfinish" $! _ _ ⊤ with "[//] [$Htok $Hserproph $Hser3 $hashs1 //]").
+                  iApply ("Hfinish" $! ⊤ with "[//] [$Htok $Hserproph $Hser3 $hashs1 //]").
                   iNext. iIntros ([]) "[Htok %]"; simplify_eq; wp_pures.
                   iApply ("HΦ" $! (None)). by iFrame.
 
                 * iMod (na_inv_acc with "Htab Htok") as "(Htabo & Htok & Hclose_tab)"; [solve_ndisj|solve_ndisj|].
-                  iDestruct "Htabo" as (??) "(Hl & >%Hm & Hbigsep & Hge)". wp_load.
+                  iDestruct "Htabo" as (???) "(Hl & >%Hm & Hbigsep & Hge & Hid' & >%Hidinv)". wp_load.
 
-                  iDestruct "Hge" as "[Hpos'|[Hpos'|[Hpos' %Hge]]]";
+                  iPoseProof (id_agree with "Hid Hid'") as (->) "[Hid Hid']".
+                  iMod (id_update _ (ctr+1) with "Hid Hid'") as "[Hid Hid']".
+
+                  iDestruct "Hge" as "[Hpos'|[Hpos'|[Hpos' Hge]]]";
                     iPoseProof (pos_agree with "Hpos Hpos'") as (?) "[Hpos Hpos']"; 
                     simplify_eq.
 
                   iMod (pos_update1 with "Hpos Hpos'") as "(Hpos & Hpos' & Hfrag)".
 
                   wp_bind (map.map_insert _ _ _). wp_pures.
-                  iApply (gwp_map_insert #cntr (#c0, finish)%V d m _ _); [done|done|].
+                  iApply (gwp_map_insert #ctr (#c0, finish)%V d m _ _); [done|done|].
                   
                   iModIntro. iIntros (d') "%Hmap'". wp_store.
-
-                  (* iMod (msize_update _ (s+1) with "[$Hms $Hs]") as "[Hms Hs]". *)
                   wp_pures. wp_apply (gwp_list_tail with "[//]").
                   iIntros "/=" (tl Htl). wp_pures.
-                  iMod ("Hclose_tab" with "[$Hl Hbigsep $Htok Hfinish Hpos' Hfrag]") as "Htok".
-                  { iNext. iFrame "%". iSplitR "Hpos'"; last first.
-                    { do 2 iRight. iFrame "∗". admit. }
-                    iApply (big_sepM_insert_2 with "[Hfinish Hfrag]"); last done.
-                    assert (c0 > 0).
-                    { apply Nat.neq_0_lt_0. intros ->. by apply H0. }
-                    repeat iExists _. repeat (try (iSplit; eauto)).
-                    iRight. iFrame. iExists _. iLeft. by iFrame "# ∗". }
+                  iMod ("Hclose_tab" with "[$Hl Hbigsep $Htok Hfinish Hpos' Hfrag $Hid']") as "Htok".
+                  { iNext. iFrame "# %". iSplit; [|iSplitL].
+                    { iApply (big_sepM_insert_2 with "[Hfinish Hfrag]"); last done.
+                      assert (c0 > 0).
+                      { apply Nat.neq_0_lt_0. intros ->. by apply H0. }
+                      repeat iExists _. repeat (try (iSplit; eauto)).
+                      iRight. iFrame. iExists _. iLeft. by iFrame "# ∗". }
+                    { do 2 iRight. iFrame "∗ #". iExists ctr, c0. repeat iExists _.
+                      iSplit; [|iLeft; by iFrame]. iPureIntro.
+                      rewrite lookup_insert. repeat (split; eauto).
+                      assert (c0 ≠ 0); try lia.
+                      intros ?. simplify_eq. } 
+                    iPureIntro. intros ??.
+                    specialize (Hidinv ctr' ltac:(lia)).
+                    rewrite lookup_insert_None. split; eauto.
+                    intros ?. simplify_eq. lia. }
 
                   iModIntro. iApply ("HΦ" $! (Some _)). iFrame "∗ % #". 
                   repeat (iExists _). iSplit.
-                  { iPureIntro. split; repeat f_equal. instantiate (1 := cntr + 1). lia. }
-                  iRight; iFrame "# ∗ %"; iExists _, (cntr+1);
+                  { iPureIntro. split; repeat f_equal. lia. }
+                  iRight; iFrame "# ∗ %"; iExists _, (ctr+1);
                     iSplit; iPureIntro; repeat f_equal; lia.
                   
               + wp_apply v_finish_spec1; try done.
@@ -1347,7 +1048,16 @@ Section proof.
                 * wp_bind (finish #()).
                   assert (c0 = 0); [lia|]. simplify_eq.
 
-                  iApply ("Hfinish" $! _ _ ⊤ with "[//] [$Htok $Hserproph $Hser3 //]").
+                  iMod (na_inv_acc with "Htab Htok") as "(Htabo & Htok & Hclose_tab)"; [solve_ndisj|solve_ndisj|].
+                  iDestruct "Htabo" as (???) "(Hl & >%Hm & Hbigsep & Hge & >Hid' & >%Hidinv)".
+
+                  iPoseProof (id_agree with "Hid Hid'") as (->) "[Hid Hid']".
+                  iMod (id_update _ (ctr+1) with "Hid Hid'") as "[Hid Hid']".
+
+                  iMod ("Hclose_tab" with "[$Htok $Hl $Hbigsep $Hge $Hid']") as "Htok".
+                  { iNext. iFrame "%". iPureIntro. intros ??. apply Hidinv. lia. }
+
+                  iApply ("Hfinish" $! ⊤ with "[//] [$Htok $Hserproph $Hser3 //]").
                   iNext. iIntros ([]) "Htok"; simplify_eq; wp_pures; last first.
                   { iApply ("HΦ" $! (None)). by iFrame. }
 
@@ -1358,43 +1068,48 @@ Section proof.
                   iMod ("Hrel" $! ⊤ with "[//] Htok [Hserproph] Hser1 HA") as "[Htok #HA']";
                     try by iRight.
                   iFrame "# ∗". iModIntro; repeat (iExists _);
-                  iSplit; try (iSplit; try done; iPureIntro; repeat f_equal; 
-                    instantiate (1 := cntr + 1); lia).
-                  iLeft. iFrame "# ∗ %"; iExists _, (cntr+1);
+                  iSplit; try (iSplit; try done; iPureIntro; repeat f_equal; lia);
+                  iLeft; iFrame "# ∗ %"; iExists _, (ctr+1);
                     iSplit; iPureIntro; repeat f_equal; lia.
                     
                 * iMod (na_inv_acc with "Htab Htok") as "(Htabo & Htok & Hclose_tab)"; [solve_ndisj|solve_ndisj|].
-                  iDestruct "Htabo" as (??) "(Hl & >%Hm & Hbigsep & >Hge)". wp_load.
+                  iDestruct "Htabo" as (???) "(Hl & >%Hm & Hbigsep & Hge & Hid' & >%Hidinv)". wp_load.
 
-                  iDestruct "Hge" as "[Hpos'|[Hpos'|[Hpos' %Hge]]]";
+                  iPoseProof (id_agree with "Hid Hid'") as (->) "[Hid Hid']".
+                  iMod (id_update _ (ctr+1) with "Hid Hid'") as "[Hid Hid']".
+
+                  iDestruct "Hge" as "[Hpos'|[Hpos'|[Hpos' Hge]]]";
                     iPoseProof (pos_agree with "Hpos Hpos'") as (?) "[Hpos Hpos']"; 
                     simplify_eq.
 
                   wp_bind (map.map_insert _ _ _). wp_pures.
-                  iApply (gwp_map_insert #cntr (#c0, finish)%V d m _ _); [done|done|].
+                  iApply (gwp_map_insert #ctr (#c0, finish)%V d m _ _); [done|done|].
                   
                   iModIntro. iIntros (d') "%Hmap'". wp_store.
 
                   wp_pures. wp_apply (gwp_list_tail with "[//]").
                   iIntros "/=" (tl Htl). wp_pures.
-                  iMod ("Hclose_tab" with "[$Hl Hbigsep $Htok Hfinish Hpos]") as "Htok".
-                  { iNext. iFrame "%". iSplitR "Hpos"; last first; try by iLeft.
-                    iApply (big_sepM_insert_2 with "[Hfinish]"); last done.
-                    assert (c0 > 0).
-                    { apply Nat.neq_0_lt_0. intros ->. by apply H0. }
-                    repeat iExists _. repeat (try (iSplit; eauto)).
-                    do 2 iLeft. iFrame. eauto. }
+                  iMod ("Hclose_tab" with "[$Hl Hbigsep $Htok Hfinish Hpos Hid']") as "Htok".
+                  { iNext. iFrame "% ∗". iSplitL.
+                    { iApply (big_sepM_insert_2 with "[Hfinish]"); last done.
+                      assert (c0 > 0).
+                      { apply Nat.neq_0_lt_0. intros ->. by apply H0. }
+                      repeat iExists _. repeat (try (iSplit; eauto)).
+                      do 2 iLeft. iFrame. eauto. }
+                    iPureIntro. intros ??.
+                    specialize (Hidinv ctr' ltac:(lia)).
+                    rewrite lookup_insert_None. split; eauto.
+                    intros ?. simplify_eq. lia. }
 
                   iApply ("HΦ" $! (Some _)).
                   iMod ("Hrel" $! ⊤ with "[//] Htok [Hserproph] Hser1 HA") as "[Htok #HA']";
                     try by iRight.
                   iFrame "# ∗"; iModIntro; repeat (iExists _).
-                  iSplit; try (iSplit; try done; iPureIntro; repeat f_equal; 
-                    instantiate (1 := cntr + 1); lia).
-                  iLeft. iFrame "# ∗ %"; iExists _, (cntr+1);
+                  iSplit; try (iSplit; try done; iPureIntro; repeat f_equal; lia).
+                  iLeft. iFrame "# ∗ %"; iExists _, (ctr+1);
                     iSplit; iPureIntro; repeat f_equal; lia.
 
-            - destruct (decide (s2 = s1)); simplify_eq; last first.
+            - destruct (decide (s1 = s2)); simplify_eq; last first.
 
               + wp_apply v_finish_spec2_bad; try done.
                 iIntros (finish) "Hfinish". wp_pures.
@@ -1403,40 +1118,51 @@ Section proof.
                 * wp_bind (finish #()).
                   assert (c0 = 0); [lia|]. simplify_eq.
 
-                  iApply ("Hfinish" $! _ _ _ ⊤ with "[//] [$Htok $Hserproph $Hser3 $hashs1 $Hinv //]").
+                  iApply ("Hfinish" $! ⊤ with "[//] [$Htok $Hserproph $Hser3 $hashs1 $Hinv //]").
                   iNext. iIntros ([]) "[Htok %]"; simplify_eq; wp_pures.
                   iApply ("HΦ" $! (None)). by iFrame.
                 
                 * iMod (na_inv_acc with "Htab Htok") as "(Htabo & Htok & Hclose_tab)"; [solve_ndisj|solve_ndisj|].
-                  iDestruct "Htabo" as (??) "(Hl & >%Hm & Hbigsep & Hge)". wp_load.
+                  iDestruct "Htabo" as (???) "(Hl & >%Hm & Hbigsep & Hge & Hid' & >%Hidinv)". wp_load.
 
-                  iDestruct "Hge" as "[Hpos'|[Hpos'|[Hpos' %Hge]]]";
+                  iPoseProof (id_agree with "Hid Hid'") as (->) "[Hid Hid']".
+                  iMod (id_update _ (ctr+1) with "Hid Hid'") as "[Hid Hid']".
+
+                  iDestruct "Hge" as "[Hpos'|[Hpos'|[Hpos' Hge]]]";
                     iPoseProof (pos_agree with "Hpos Hpos'") as (?) "[Hpos Hpos']"; 
                     simplify_eq.
 
                   iMod (pos_update1 with "Hpos Hpos'") as "(Hpos & Hpos' & Hfrag)".
 
                   wp_bind (map.map_insert _ _ _). wp_pures.
-                  iApply (gwp_map_insert #cntr (#c0, finish)%V d m _ _); [done|done|].
+                  iApply (gwp_map_insert #ctr (#c0, finish)%V d m _ _); [done|done|].
                   
                   iModIntro. iIntros (d') "%Hmap'". wp_store.
 
                   (* iMod (msize_update _ (s+1) with "[$Hms $Hs]") as "[Hms Hs]". *)
                   wp_pures. wp_apply (gwp_list_tail with "[//]").
                   iIntros "/=" (tl Htl). wp_pures.
-                  iMod ("Hclose_tab" with "[$Hl Hbigsep $Htok Hfinish Hpos' Hfrag]") as "Htok".
-                  { iNext. iFrame "%". iSplitR "Hpos'"; last first.
-                    { do 2 iRight. iFrame "∗". admit. }
-                    iApply (big_sepM_insert_2 with "[Hfinish Hfrag]"); last done.
-                    assert (c0 > 0).
-                    { apply Nat.neq_0_lt_0. intros ->. by apply H0. }
-                    repeat iExists _. repeat (try (iSplit; eauto)).
-                    iRight. iFrame. iExists _. iRight. by iFrame "# ∗". }
-
+                  iMod ("Hclose_tab" with "[$Hl Hbigsep $Htok Hfinish Hpos' Hfrag Hid']") as "Htok".
+                  { iNext. iFrame "% ∗". iSplit; [|iSplitL].
+                    { iApply (big_sepM_insert_2 with "[Hfinish Hfrag]"); last done.
+                      assert (c0 > 0).
+                      { apply Nat.neq_0_lt_0. intros ->. by apply H0. }
+                      repeat iExists _. repeat (try (iSplit; eauto)).
+                      iRight. iFrame. iExists _. iRight. by iFrame "# ∗". }
+                    { do 2 iRight. iFrame "∗ #". iExists ctr, c0. repeat iExists _.
+                      iSplit; [|iRight; by iFrame]. iPureIntro.
+                      rewrite lookup_insert. repeat (split; eauto).
+                      assert (c0 ≠ 0); try lia.
+                      intros ?. simplify_eq. } 
+                    iPureIntro. intros ??.
+                    specialize (Hidinv ctr' ltac:(lia)).
+                    rewrite lookup_insert_None. split; eauto.
+                    intros ?. simplify_eq. lia. }
+                  
                   iModIntro. iApply ("HΦ" $! (Some _)). iFrame "∗ % #". 
                   repeat (iExists _). iSplit.
-                  { iPureIntro. split; repeat f_equal. instantiate (1 := cntr + 1). lia. }
-                  iRight; iFrame "# ∗ %"; iExists _, (cntr+1);
+                  { iPureIntro. split; repeat f_equal. lia. }
+                  iRight; iFrame "# ∗ %"; iExists _, (ctr+1);
                     iSplit; iPureIntro; repeat f_equal; lia.
 
               + wp_apply (v_finish_spec2 with "Htab").
@@ -1446,53 +1172,65 @@ Section proof.
                 * wp_bind (finish #()).
                   assert (c0 = 0); [lia|]. simplify_eq.
 
-                  iApply ("Hfinish" $! _ _ ⊤ with "[//] [$Htok $Hserproph $Hser3 $Hinv $Hpos]"); eauto.
+                  iMod (na_inv_acc with "Htab Htok") as "(Htabo & Htok & Hclose_tab)"; [solve_ndisj|solve_ndisj|].
+                  iDestruct "Htabo" as (???) "(Hl & >%Hm & Hbigsep & Hge & >Hid' & >%Hidinv)".
+
+                  iPoseProof (id_agree with "Hid Hid'") as (->) "[Hid Hid']".
+                  iMod (id_update _ (ctr+1) with "Hid Hid'") as "[Hid Hid']".
+
+                  iMod ("Hclose_tab" with "[$Htok $Hl $Hbigsep $Hge $Hid']") as "Htok".
+                  { iNext. iFrame "%". iPureIntro. intros ??. apply Hidinv. lia. }
+
+                  iApply ("Hfinish" $! ⊤ with "[//] [$Htok $Hserproph $Hser3 $Hinv $Hpos]"); eauto.
                   iNext. iIntros ([]) "[Htok Hpos]"; wp_pures; last first.
                   { iApply ("HΦ" $! (None)). eauto. }
 
                   wp_apply gwp_list_tail; [done|].
                   iIntros (vl Hl). wp_pures.
-                  
-                  iApply ("HΦ" $! (Some _)).
 
+                  iApply ("HΦ" $! (Some _)).
                   iMod ("Hrel" $! ⊤ with "[//] Htok [Hserproph] Hser1 HA") as "[Htok #HA']";
                     try by iRight.
                   iFrame "# ∗"; iModIntro; repeat (iExists _).
-                  iSplit; try (iSplit; try done; iPureIntro; repeat f_equal; 
-                    instantiate (1 := cntr + 1); lia).
-                  iLeft. iFrame "# ∗ %". iExists _, (cntr+1);
+                  iSplit; try (iSplit; try done; iPureIntro; repeat f_equal; lia).
+                  iLeft. iFrame "# ∗ %"; iExists _, (ctr+1);
                     iSplit; iPureIntro; repeat f_equal; lia.
                 
                 * iMod (na_inv_acc with "Htab Htok") as "(Htabo & Htok & Hclose_tab)"; [solve_ndisj|solve_ndisj|].
-                  iDestruct "Htabo" as (??) "(Hl & >%Hm & Hbigsep & >Hge)". wp_load.
+                  iDestruct "Htabo" as (???) "(Hl & >%Hm & Hbigsep & Hge & Hid' & >%Hidinv)". wp_load.
 
-                  iDestruct "Hge" as "[Hpos'|[Hpos'|[Hpos' %Hge]]]";
+                  iPoseProof (id_agree with "Hid Hid'") as (->) "[Hid Hid']".
+                  iMod (id_update _ (ctr+1) with "Hid Hid'") as "[Hid Hid']".
+
+                  iDestruct "Hge" as "[Hpos'|[Hpos'|[Hpos' Hge]]]";
                     iPoseProof (pos_agree with "Hpos Hpos'") as (?) "[Hpos Hpos']"; 
                     simplify_eq.
 
                   wp_bind (map.map_insert _ _ _). wp_pures.
-                  iApply (gwp_map_insert #cntr (#c0, finish)%V d m _ _); [done|done|].
+                  iApply (gwp_map_insert #ctr (#c0, finish)%V d m _ _); [done|done|].
                   
                   iModIntro. iIntros (d') "%Hmap'". wp_store.
 
                   wp_pures. wp_apply (gwp_list_tail with "[//]").
                   iIntros "/=" (tl Htl). wp_pures.
-                  iMod ("Hclose_tab" with "[$Hl Hbigsep $Htok Hfinish Hpos]") as "Htok".
-                  { iNext. iFrame "%". iSplitR "Hpos"; last first; try by iLeft.
-                    iApply (big_sepM_insert_2 with "[Hfinish]"); last done.
-                    assert (c0 > 0).
-                    { apply Nat.neq_0_lt_0. intros ->. by apply H0. }
-                    repeat iExists _. repeat (try (iSplit; [done|])).
-                    iLeft. iRight. by iFrame "# ∗". }
-
+                  iMod ("Hclose_tab" with "[$Hl Hbigsep $Htok Hfinish Hpos Hid']") as "Htok".
+                  { iNext. iFrame "% ∗". iSplitL.
+                    { iApply (big_sepM_insert_2 with "[Hfinish]"); last done.
+                      assert (c0 > 0).
+                      { apply Nat.neq_0_lt_0. intros ->. by apply H0. }
+                      repeat iExists _. repeat (try (iSplit; [done|])).
+                      iLeft. iRight. by iFrame "# ∗". }
+                    iPureIntro. intros ??.
+                    specialize (Hidinv ctr' ltac:(lia)).
+                    rewrite lookup_insert_None. split; eauto.
+                    intros ?. simplify_eq. lia. }
+                  
                   iApply ("HΦ" $! (Some _)).
-
                   iMod ("Hrel" $! ⊤ with "[//] Htok [Hserproph] Hser1 HA") as "[Htok #HA']";
                     try by iRight.
                   iFrame "# ∗"; iModIntro; repeat (iExists _).
-                  iSplit; try (iSplit; try done; iPureIntro; repeat f_equal; 
-                      instantiate (1 := cntr + 1); lia);
-                  iLeft; iFrame "# ∗ %"; iExists _, (cntr+1);
+                  iSplit; try (iSplit; try done; iPureIntro; repeat f_equal; lia).
+                  iLeft. iFrame "# ∗ %"; iExists _, (ctr+1);
                     iSplit; iPureIntro; repeat f_equal; lia. }
               
           { iApply (refines_un_auth_unauth with "Htab Hser' Hser3 Hcount Hdeser Hauth_un"). } }
@@ -1552,7 +1290,7 @@ Section proof.
       iFrame. iModIntro. interp_unfold!.
       rewrite interp_var2_ext3.
       iApply (refines_un_auth_unauth with "Htab Hser' Hser3 Hcount Hdeser Hauth_un"). }
-  Admitted.
+  Qed.
   
   Lemma refines_Authenticatable Θ (Δ : ctxO Σ Θ) :
     ⊢ REL v_Authenticable << i_Authenticable : ⟦ Authenticatable ⟧ (auth_ctx Δ).
