theories/examples/authentikit_base_susp_security.v
@@ -13,373 +13,11 @@ Inductive evi_type : Type :=
 | tint
 | tauth.
 
-(* Definition mapUR := gmapUR nat (agreeR (prodO
-                                          (prodO
-                                             (prodO
-                                                (prodO (leibnizO evi_type) valO)
-                                                valO)
-                                             (optionO locO))
-                                          (leibnizO bool))).
-
-Definition locPidMapUR := gmapUR locO nat.
-
-Definition stateUR := authUR (prodUR mapUR locPidMapUR).
-Class stateG Σ := StateG { state_inG :> inG Σ stateUR; stateG_name : gname }. *)
-
-(* Definition counterUR := gmapUR nat (authR natUR).
-Class counterG Σ := CounterG { counter_inG :> inG Σ counterUR; counterG_name : gname }. *)
-
 Definition authSet (N : namespace) : namespace := N .@ "auth".
 Definition authN (N : namespace) (l : loc) : namespace := (authSet N) .@ l.
 
 Section authenticatable.
   Context `{!heapGS_gen hlc Σ, !seqG Σ} (N : namespace).
-
-  (* Definition authSerSet : namespace := N .@ "auth_ser".
-  Definition authSerN (v: val) : namespace := authSerSet .@ v.
-  Definition authValidSet : namespace := N .@ "auth_valid".
-  Definition authValidN (v: val) : namespace := authValidSet .@ v.
-  Definition authCountSet : namespace := N .@ "auth_count".
-  Definition authCountN (l: loc) : namespace := authCountSet .@ l.
-  Definition authInSet : namespace := N .@ "auth_in".
-  Definition authInN (l : loc) : namespace := authInSet .@ l. *)
-
-  (* Definition single_instance (id : nat) (t : evi_type) (x vᵥ : val) (susp_option : option loc) (b : bool)  : iProp Σ :=
-    own stateG_name (◯ ({[ id := to_agree (t, x, vᵥ, susp_option, b) ]} : mapUR,
-                         (if susp_option is Some susp then {[ susp := id ]} else ∅) : locPidMapUR)). *)
-
-  (* Definition count (pid c : nat) : iProp Σ :=
-    own counterG_name ({[ pid := ● c ]}).
-
-  Definition token (pid : nat) : iProp Σ :=
-    own counterG_name ({[ pid := ◯ 1 ]}).
-
-  Definition used_token (pid : nat) : iProp Σ :=
-    □ (own counterG_name ({[ pid := ◯ 1 ]})). *)
-
-  (* Definition suspended_loc (susp : loc) : iProp Σ :=
-    ∀ (h: string), susp ↦□ InjRV #h -∗ False.
-
-  (* Definition count_auth_inv (susp : loc) (c : nat) : iProp Σ :=
-    ((∃ (h : string), susp ↦□ (InjRV #h) ∗ ⌜c = 0⌝) ∨
-       (suspended_loc susp ∗ ⌜c = 1⌝)). *)
-  
-  Fixpoint count_is_correct (t : evi_type) (v : val) (c : nat) : iProp Σ :=
-    match t with
-    | tprod t1 t2 =>
-        ∃ (c1 c2 : nat) (v1 v2 : val),
-          ⌜v = (v1, v2)%V ∧ (c1 + c2)%nat = c⌝ ∗ count_is_correct t1 v1 c1 ∗ count_is_correct t2 v2 c2
-    | tsum t1 t2 =>
-        (∃ (v1 : val), ⌜v = InjLV v1⌝ ∗ count_is_correct t1 v1 c) ∨
-          (∃ (v2 : val), ⌜v = InjRV v2⌝ ∗ count_is_correct t2 v2 c)
-    | tstring => string_valid_val v ∧ ⌜c = 0⌝
-    | tint => int_valid_val v ∧ ⌜c = 0⌝
-    | tauth =>
-        (∃ v1, ⌜v = SOMEV v1⌝ ∧
-                 ((∃ (h : string), ⌜v1 = InjLV #h ∧ c = 0⌝) ∨ 
-                    (∃ (susp : loc),
-                        ⌜v1 = InjRV #susp⌝ ∗
-                          ((∃ (h : string), susp ↦□ (InjRV #h) ∗ ⌜c = 0⌝) ∨
-                             (∃ (pid : nat), susp ↦{#1/4} InjLV #pid ∗ ⌜c = 1⌝)))))
-  end.
-
-  #[global] Instance count_is_correct_timeless t v c: Timeless (count_is_correct t v c).
-  Proof. revert v c; induction t => v c; simpl; apply _. Qed.
-
-  Fixpoint susp_in_v (t : evi_type) (v : val) (susp : loc) : iProp Σ :=
-    match t with
-    | tprod t1 t2 =>
-        ∃ (v1 v2 : val), ⌜v = (v1, v2)%V⌝ ∧ (susp_in_v t1 v1 susp ∨ susp_in_v t2 v2 susp)
-    | tsum t1 t2 =>
-        ∃ (v' : val), (⌜v = InjLV v'⌝ ∧ susp_in_v t1 v' susp) ∨ (⌜v = InjRV v'⌝ ∧ susp_in_v t2 v' susp)
-    | tstring | tint => False
-    | tauth => ∃ v1, ⌜v = SOMEV v1 ∧ v1 = InjRV #susp⌝ ∗
-                       ((∃ (pid : nat), susp ↦{#1/4} InjLV #pid) ∨ False)
-  end.
-
-  Fixpoint sub_obj (v sv: val) (t : evi_type) :=
-    match t with
-    | tprod t1 t2 =>
-        ∃ v1 v2, v = (v1, v2)%V ∧ (sv = v1 ∨ sv = v2 ∨ sub_obj v1 sv t1 ∨ sub_obj v2 sv t2)
-    | tsum t1 t2 =>
-        ∃ v', ((v = InjLV v' ∧ sub_obj v' sv t1 ∧ v = v') ∨
-                 (v = InjRV v' ∧ sub_obj v' sv t2 ∧ v = v'))
-    | tstring => False
-    | tint => False
-    | tauth =>
-        ∃ v', (v = SOMEV (InjLV v') ∨ (v = SOMEV (InjRV v'))) ∧ v' = sv
-  end.
-
-  Definition subeq_obj (v sv: val) :=
-    (∃ t, sub_obj v sv t) ∨ v = sv.
-
-  Lemma subeq_obj_trans (v sv ssv : val) :
-    subeq_obj v sv → subeq_obj sv ssv → subeq_obj v ssv.
-  Proof. Admitted.
-
-  Fixpoint sub_obj_bin (v1 v2 sv1 sv2 : val) (t : evi_type) :=
-    match t with
-    | tprod t1 t2 =>
-        ∃ v11 v12 v21 v22, v1 = (v11, v12)%V ∧ v2 = (v21, v22)%V ∧
-                             ((sv1 = v11 ∧ sv2 = v21) ∨ (sv1 = v12 ∧ sv2 = v22) ∨
-                                (sub_obj_bin v11 v21 sv1 sv2 t1) ∨
-                                (sub_obj_bin v12 v22 sv1 sv2 t2))
-    | tsum t1 t2 =>
-        ∃ v1' v2', ((v1 = InjLV v1' ∧ v2 = InjLV v2' ∧
-                       sub_obj_bin v1' v2' sv1 sv2 t1) ∨
-                      (v1 = InjRV v1' ∧ v2 = InjRV v2' ∧
-                         sub_obj_bin v1' v2' sv1 sv2 t2))
-    | tstring => False
-    | tint => False
-    | tauth => False
-  end.
-
-  Definition subeq_obj_bin (v1 v2 sv1 sv2 : val) :=
-    (∃ t, sub_obj_bin v1 v2 sv1 sv2 t) ∨ (v1 = sv1 ∧ v2 = sv2).
-
-  Lemma subeq_obj_bin_trans (v1 v2 sv1 sv2 ssv1 ssv2 : val) :
-    subeq_obj_bin v1 v2 sv1 sv2 → subeq_obj_bin sv1 sv2 ssv1 ssv2 → subeq_obj_bin v1 v2 ssv1 ssv2.
-  Proof. Admitted.
-    
-  Lemma subeq_obj_bin_to_unary (v1 v2 sv1 sv2 : val) :
-    subeq_obj_bin v1 v2 sv1 sv2 → subeq_obj v1 sv1 ∧ subeq_obj v2 sv2.
-  Proof. Admitted. *)
-                                                        
-  (* Fixpoint val_eq (t : evi_type) (v1 v2 : val) : iProp Σ :=
-    match t with
-    | tprod t1 t2 =>
-        ∃ v11 v12 v21 v22,
-          ⌜v1 = (v11, v12)%V ∧ v2 = (v21, v22)%V⌝ ∗ val_eq t1 v11 v21 ∗ val_eq t2 v12 v22
-    | tsum t1 t2 => 
-        ∃ v1' v2',
-          (⌜v1 = InjLV v1' ∧ v2 = InjLV v2'⌝ ∗ val_eq t1 v1' v2') ∨
-            (⌜v1 = InjRV v1' ∧ v2 = InjRV v2'⌝ ∗ val_eq t2 v1' v2')
-    | tstring => ∃ (s: string), ⌜v1 = #s ∧ v2 = #s⌝
-    | tint => ∃ (i: nat), ⌜v1 = #i ∧ v2 = #i⌝
-    | tauth =>
-        ⌜v1 = NONEV ∧ v2 = NONEV⌝ ∨
-          (∃ (h: string), (⌜v1 = SOMEV (InjLV #h)⌝ ∨
-                   (∃ (susp : loc), ⌜v1 = SOMEV (InjRV #susp)⌝ ∗ susp ↦□ InjRV #h)) ∧
-                  (⌜v2 = SOMEV (InjLV #h)⌝ ∨
-                     (∃ (susp : loc), ⌜v2 = SOMEV (InjRV #susp)⌝ ∗ susp ↦□ InjRV #h)))
-  end.
-
-  #[global] Instance val_eq_persistent t v1 v2 : Persistent (val_eq t v1 v2).
-  Proof. revert v1 v2. induction t => v1 v2; simpl; apply _. Qed.
-
-  Lemma val_eq_sym t v1 v2 :
-    val_eq t v1 v2 ⊣⊢ val_eq t v2 v1.
-  Proof.
-    iInduction t as [t1 IH1 t2 IH2 | t1 IH1 t2 IH2 | | | ] "IH" forall (v1 v2); simpl.
-    all: iSplit.
-    all: try (iIntros "(%x & [-> ->])"; iExists x; done).
-    all: try (iIntros "[[-> ->] | (%h & H1 & H2)]";
-      [iLeft; iPureIntro; naive_solver |
-       iRight; iExists h; iSplit; [done | done]]).
-    - iIntros "(%v11 & %v12 & %v21 & %v22 & [-> ->] & H1 & H2)".
-      iExists v21, v22, v11, v12. iSplitR. iPureIntro; done.
-      iSplitL "H1". iApply "IH". iExact "H1". iApply "IH1". iExact "H2".
-    - iIntros "(%v11 & %v12 & %v21 & %v22 & [-> ->] & H1 & H2)".
-      iExists v21, v22, v11, v12. iSplitR. iPureIntro; done.
-      iSplitL "H1". iApply "IH". iExact "H1". iApply "IH1". iExact "H2".
-    - iIntros "(%v1' & %v2' & [HL | HR])".
-      + iDestruct "HL" as "[%Heq Ha]". destruct Heq as [-> ->].
-        iExists v2', v1'. iLeft. iSplitR. iPureIntro; done. iApply "IH". iExact "Ha".
-      + iDestruct "HR" as "[%Heq Hb]". destruct Heq as [-> ->].
-        iExists v2', v1'. iRight. iSplitR. iPureIntro; done. iApply "IH1". iExact "Hb".
-    - iIntros "(%v1' & %v2' & [HL | HR])".
-      + iDestruct "HL" as "[%Heq Ha]". destruct Heq as [-> ->].
-        iExists v2', v1'. iLeft. iSplitR. iPureIntro; done. iApply "IH". iExact "Ha".
-      + iDestruct "HR" as "[%Heq Hb]". destruct Heq as [-> ->].
-        iExists v2', v1'. iRight. iSplitR. iPureIntro; done. iApply "IH1". iExact "Hb".
-  Qed.
-
-  Lemma val_eq_trans t v1 v2 v3 :
-    val_eq t v1 v2 ∗ val_eq t v2 v3 -∗ val_eq t v1 v3.
-  Proof.
-    iInduction t as [t1 IH1 t2 IH2 | t1 IH1 t2 IH2 | | | ] "IH" forall (v1 v2 v3); simpl; iIntros "[H1 H2]".
-    { iDestruct "H1" as "(%v11 & %v12 & %v21 & %v22 & [-> ->] & Ha & Hb)".
-      iDestruct "H2" as "(%w11 & %w12 & %w21 & %w22 & [[%Heq1 ->] [Hc Hd]])".
-      injection Heq1; intros; subst.
-      iExists v11, v12, w21, w22.
-      iSplitR. iPureIntro; done.
-      iSplitL "Ha Hc". iApply "IH". iFrame.
-      iApply "IH1". iFrame. }
-    { iDestruct "H1" as "(%a & %b & [HL1 | HR1])";
-      iDestruct "H2" as "(%c & %d & [HL2 | HR2])".
-      - iDestruct "HL1" as "[%Heq1 Ha]". destruct Heq1 as [-> ->].
-        iDestruct "HL2" as "[%Heq2 Hb]". destruct Heq2 as [Heq2a ->].
-        injection Heq2a; intros; subst.
-        iExists a, d. iLeft. iSplitR. iPureIntro; done. iApply "IH". iFrame.
-      - iDestruct "HL1" as "[%Heq1 _]". destruct Heq1 as [_ ->].
-        iDestruct "HR2" as "[%Heq2 _]". destruct Heq2 as [Heq2a _]. discriminate.
-      - iDestruct "HR1" as "[%Heq1 _]". destruct Heq1 as [_ ->].
-        iDestruct "HL2" as "[%Heq2 _]". destruct Heq2 as [Heq2a _]. discriminate.
-      - iDestruct "HR1" as "[%Heq1 Ha]". destruct Heq1 as [-> ->].
-        iDestruct "HR2" as "[%Heq2 Hb]". destruct Heq2 as [Heq2a ->].
-        injection Heq2a; intros; subst.
-        iExists a, d. iRight. iSplitR. iPureIntro; done. iApply "IH1". iFrame. }
-    { iDestruct "H1" as "(%s & [%Heq1 %Heq2])".
-      iDestruct "H2" as "(%s' & [%Heq3 %Heq4])".
-      iPureIntro. simplify_eq. eauto. }
-    { iDestruct "H1" as "(%i & [%Heq1 %Heq2])".
-      iDestruct "H2" as "(%i' & [%Heq3 %Heq4])".
-      iPureIntro. simplify_eq. eauto. }
-    iDestruct "H1" as "[%Hn1 | (%h & Hv1 & Hw1)]".
-    { destruct Hn1 as [-> ->].
-      iDestruct "H2" as "[%Hn2 | (%h & Hv2 & _)]".
-      - iLeft. iPureIntro. done.
-      - iDestruct "Hv2" as "[%Habs | (%susp & %Habs & _)]"; discriminate. }
-    iDestruct "H2" as "[%Hn2 | (%h' & Hv2 & Hw2)]";
-      [destruct Hn2 as [-> _];
-       iDestruct "Hw1" as "[%Habs | (%susp & %Habs & _)]"; discriminate|].
-    iDestruct "Hw1" as "[%Hv2eq | (%susp1 & %Hv2eq & #Hf1)]".
-    all: iDestruct "Hv2" as "[%Hv2eq' | (%susp2 & %Hv2eq' & #Hf2)]".
-    all: try (simplify_eq; discriminate).
-    all: simplify_eq.
-    2: iDestruct (pointsto_agree with "Hf1 Hf2") as "%Hagree"; simplify_eq.
-    all: iRight; iExists h'; iSplit; [iExact "Hv1" | iExact "Hw2"].
-  Qed.
-
-  Lemma val_eq_inj_t t1 t2 v1 v2 :
-    val_eq t1 v1 v2 ∗ val_eq t2 v1 v2 -∗ ⌜t1 = t2⌝.
-  Proof. Admitted. *)
-
-  (* Lemma sub_obj_bin_val_eq_agree_t (v1 v2 sv1 sv2 : val) (t1 t2 : evi_type) :
-    ⌜sub_obj_bin v1 v2 sv1 sv2 t1⌝ ∗ val_eq t2 v1 v2 -∗ ⌜t1 = t2⌝.
-  Proof.
-    iIntros "[%Hbinsub #Heq]".
-    destruct t1, t2; simpl in Hbinsub; iSimpl in "Heq".
-  Admitted.
-
-  Lemma val_eq_sub_eq (v1 v2 sv1 sv2 : val) (t : evi_type) :
-    ⌜subeq_obj_bin v1 v2 sv1 sv2⌝ ∗ val_eq t v1 v2 -∗ ∃ st, val_eq st sv1 sv2.
-  Proof.
-    iInduction t as [| | | |]
-                      forall (v1 v2 sv1 sv2);
-                             iIntros "[%Hbinsubeq #Heq]";
-                             simpl in Hbinsubeq.
-      - destruct Hbinsubeq as [[t Hbinsub]|Hbineq];
-          iPoseProof "Heq" as (?????) "(#Heq1 & #Heq2)"; last first.
-        { destruct! H. destruct! Hbineq. simplify_eq.
-          iExists (tprod t1 t2). by iFrame "#". }
-        destruct! H. simplify_eq.
-        iPoseProof (sub_obj_bin_val_eq_agree_t with "[$Heq //]") as "->".
-        destruct Hbinsub as (?&?&?&? & ?&? & [[-> ->]|[[-> ->]|[Hbinsub1|Hbinsub2]]]).
-        + simplify_eq. iFrame "#".
-        + simplify_eq. iFrame "#".
-        + simplify_eq. iApply "IHt1". iFrame "#".
-          iPureIntro. left. eauto.
-        + simplify_eq. iApply "IHt2". iFrame "#".
-          iPureIntro. left. eauto.
-      - destruct Hbinsubeq as [[t Hbinsub]|Hbineq]; last first;
-          iPoseProof "Heq" as (??) "[(% & Heq1)|(% & Heq2)]".
-        { destruct! Hbineq. destruct! H. simplify_eq.
-          iExists (tsum t1 t2). iExists _, _.
-          iLeft. iFrame "#". eauto. }
-        { destruct! Hbineq. destruct! H. simplify_eq.
-          iExists (tsum t1 t2). iExists _, _.
-          iRight. iFrame "#". eauto. }
-        + iPoseProof (sub_obj_bin_val_eq_agree_t with "[$Heq //]") as "->".
-          destruct Hbinsub as (?&? & [(-> & -> & Hbinsub1)|(-> & -> & Hbinsub2)]);
-            destruct! H; simplify_eq.
-          iApply "IHt1". iFrame "#".
-          iPureIntro. left. eauto.
-        + iPoseProof (sub_obj_bin_val_eq_agree_t with "[$Heq //]") as "->".
-          destruct Hbinsub as (?&? & [(-> & -> & Hbinsub1)|(-> & -> & Hbinsub2)]);
-            destruct! H; simplify_eq.
-          iApply "IHt2". iFrame "#".
-          iPureIntro. left. eauto.
-      - destruct Hbinsubeq as [[t Hbinsub]|Hbineq]; last first.
-        { destruct! Hbineq. simplify_eq. iFrame "#". }
-        by iPoseProof (sub_obj_bin_val_eq_agree_t with "[$Heq //]") as "->".
-      - destruct Hbinsubeq as [[t Hbinsub]|Hbineq]; last first.
-        { destruct! Hbineq. simplify_eq. iFrame "#". }
-        by iPoseProof (sub_obj_bin_val_eq_agree_t with "[$Heq //]") as "->".
-      - destruct Hbinsubeq as [[t Hbinsub]|Hbineq]; last first.
-        { destruct! Hbineq. simplify_eq. iFrame "#". }
-        by iPoseProof (sub_obj_bin_val_eq_agree_t with "[$Heq //]") as "->".
-  Qed.
-
-  Lemma sub_obj_susp_in (v : val) (susp : loc) (pid : nat) (t : evi_type) :
-    ⌜sub_obj v (InjRV (InjRV #susp)) t⌝ ∗ susp ↦{#1/4} (InjLV #pid) -∗ susp_in_v t v susp.
-  Proof. Admitted.
-
-  #[global] Instance susp_in_v_timeless t v l: Timeless (susp_in_v t v l).
-  Proof. revert v l; induction t => v l; simpl; apply _. Qed.
-
-  Lemma count_gt0 (t : evi_type) (v : val) (susp : loc) (c : nat) :
-    susp_in_v t v susp ∗ count_is_correct t v c -∗ ⌜c > 0⌝ ∗ susp_in_v t v susp ∗ count_is_correct t v c.
-  Proof.
-    iIntros "[Hin Hcount]".
-    iInduction t as [| | | |] forall (v c).
-    - iDestruct "Hin" as (???) "[Hin|Hin]";
-        iDestruct "Hcount" as (????[??]) "(Hcount1 & Hcount2)";
-        simplify_eq.
-      + iPoseProof ("IHt1" with "Hin Hcount1") as "(%&Hin1&Hcount1)".
-        iFrame. iSplit; [|eauto]. iPureIntro. lia.
-      + iPoseProof ("IHt2" with "Hin Hcount2") as "(%&Hin2&Hcount2)".
-        iFrame. iSplit; [|eauto]. iPureIntro. lia.
-    - iDestruct "Hin" as (?) "[(%&Hin)|(%&Hin)]";
-        iDestruct "Hcount" as "[(%&%&Hcount)|(%&%&Hcount)]";
-        simplify_eq.
-      + iPoseProof ("IHt1" with "Hin Hcount") as "(%&Hin&Hcount)".
-        iSplit; [done|]. iSplitL "Hin".
-        { iExists _. iLeft. eauto. }
-        { iLeft. eauto. }
-      + iPoseProof ("IHt2" with "Hin Hcount") as "(%&Hin&Hcount)".
-        iSplit; [done|]. iSplitL "Hin".
-        { iExists _. iRight. eauto. }
-        { iRight. eauto. }
-    - done.
-    - done.
-    - iDestruct "Hin" as (?[??]) "Hin";
-        iDestruct "Hcount" as (??) "[(%&%&%)|(%&%&Hcount)]";
-        simplify_eq.
-      iDestruct "Hin" as "[(% & Hin)|Hin]";
-        iDestruct "Hcount"  as "[(%&Hcount&%)|(%&Hcount&%)]";
-        eauto; simplify_eq.
-      + by iPoseProof (pointsto_agree with "Hin Hcount") as "%Hf".
-      + iSplit; [iPureIntro; lia|].
-        iSplitL "Hin".
-        { iExists _. eauto. }
-        { iExists _. iSplit; [done|].
-          iRight. iExists _. iSplit; [done|]. iRight. eauto. }
-  Qed. *)
-    
-  (* Lemma count_update (v : val) (t : evi_type) (susp : loc) (c : nat) (h : string):
-    susp ↦□ InjRV #h -∗ susp_in_v t v susp -∗ count_is_correct t v c -∗ count_is_correct t v (c-1).
-  Proof.
-    iIntros "#Hsusp Hin Hcount".
-    iPoseProof (count_gt0 with "[$Hin $Hcount]") as "(%Hc&Hin&Hcount)".
-    iInduction t as [| | | |] forall (v c Hc).
-    - iDestruct "Hcount" as (????[??]) "(Hcount1 & Hcount2)".
-      iDestruct "Hin" as (v1' v2' ?)  "[Hin|Hin]"; simplify_eq.
-      + iPoseProof (count_gt0 with "[$Hin $Hcount1]") as (?) "[Hin Hcount1]".
-        iPoseProof ("IHt1" with "[//] Hin Hcount1") as "Hcount1'".
-        iFrame "∗ #". iPureIntro. split; [done|lia].
-      + iPoseProof (count_gt0 with "[$Hin $Hcount2]") as (?) "[Hin Hcount2]".
-        iPoseProof ("IHt2" with "[//] Hin Hcount2") as "Hcount2'".
-        iFrame "∗ #". iPureIntro. split; [done|lia].
-    - iDestruct "Hin" as (?) "[(%&Hin)|(%&Hin)]";
-        iDestruct "Hcount" as "[(%&%&Hcount)|(%&%&Hcount)]";
-        simplify_eq.
-      + iPoseProof ("IHt1" with "[//] Hin Hcount") as "Hcount'".
-        iFrame. iLeft. eauto.
-      + iPoseProof ("IHt2" with "[//] Hin Hcount") as "Hcount'".
-        iFrame. iRight. eauto.
-    - done.
-    - done.
-    - iDestruct "Hin" as (?[??]) "Hin";
-        iDestruct "Hcount" as (??) "[(%&%&%)|(%&%&Hcount)]";
-        simplify_eq.
-      iDestruct "Hin" as "[Hin|Hin]";
-        iDestruct "Hcount" as "[(%&Hinvc'&%)|(Hinvc'&%)]";
-        simplify_eq; try lia.
-      + iExists _. iSplit; [done|].
-        iRight. iExists _. iSplit; [done|]. eauto.
-      + iExFalso. by iApply "Hin".
-  Qed. *)
 
   Definition proph_susp (p : proph_id) (h : string) : iProp Σ :=
     (typed_proph1_prop StringTypedProph) p h.
@@ -407,54 +45,7 @@ Section authenticatable.
       hashed s1 ∗ auth_is_ser_2 s susp) ∨ 
       auth_is_ser_3_proph s susp.
   
-  (* Definition auth_is_ser (v : val) (s : string) : iProp Σ :=
-    auth_is_ser_1 v s ∨ auth_is_ser_2 v s. *)
-
-  (* Definition auth_valid_val_2 (susp : loc) : iProp Σ :=
-    ∃ (h : string) (t : evi_type) (ax avᵥ : val),
-      susp ↦□ InjRV #h ∗
-        ((∃ aid, single_instance aid t ax avᵥ None true ∗ val_eq t ax avᵥ)  (* Most recent pre-filled ancestor *)
-         -∗ (∃ vᵥ, (∃ px pvᵥ, ⌜subeq_obj_bin px pvᵥ (SOMEV (InjRV #susp)) vᵥ⌝) -∗ val_eq tauth (SOMEV (InjRV #susp)) vᵥ)).                         
-  Definition auth_valid_val_3 (susp : loc) (dq : dfrac) : iProp Σ :=
-    (∃ (pid : nat) (p : proph_id) (pt t : evi_type) (px pvᵥ ax avᵥ : val),
-        susp ↦{dq} (InjLV #pid) ∗
-          ((∃ b so, single_instance pid pt px pvᵥ so b) -∗ susp_in_v pt px susp) ∗ (* Parent's instance *)
-          ((∃ aid, single_instance aid t ax avᵥ None true ∗ val_eq t ax avᵥ )  (* Most recent pre-filled ancestor *)
-           -∗ (∃ vᵥ, ⌜subeq_obj_bin px pvᵥ (SOMEV (InjRV #susp)) vᵥ⌝ -∗ val_eq tauth (SOMEV (InjRV #susp)) vᵥ))).
-
-  Definition valid_auth_inv (susp : loc) : iProp Σ :=
-    (auth_valid_val_2 susp ∨ auth_valid_val_3 susp (DfracOwn (1/2))).
-
-  Definition auth_valid_val (v1 : val) : iProp Σ :=
-    ∃ v, ⌜v1 = SOMEV v⌝ ∧
-           ((∃ (h : string), ⌜v = InjLV #h⌝) ∨
-              (∃ (susp : loc),
-                  ⌜v = InjRV #susp⌝ ∗ seq_inv (authValidN #susp) (valid_auth_inv susp))).
-
-  Definition auth_deser_valid_val (dq : dfrac) (v1 : val) : iProp Σ :=
-    ∃ v, ⌜v1 = SOMEV v⌝ ∧
-           ((∃ (h : string), ⌜v = InjLV #h⌝) ∨
-              (∃ (susp : loc),
-                  ⌜v = InjRV #susp⌝ ∗ auth_valid_val_3 susp dq)). *)
-
-  (* Definition auth_deser_valid_val_tok (v1 : val) : iProp Σ :=
-    ∃ v, ⌜v1 = SOMEV v⌝ ∧
-           ((∃ (h : string), ⌜v = InjLV #h⌝) ∨
-              (∃ (susp : loc),
-                  ⌜v = InjRV #susp⌝ ∗
-                    (∃ (pid : nat), susp ↦ (InjLV #pid) ∗ token pid))). *)
-             
   
-  (* Fixpoint s_is_ser_ser (t : evi_type) (v : val) (s : string) : iProp Σ :=
-    match t with
-    | tprod t1 t2 => prod_is_ser' v s (s_is_ser_ser t1) (s_is_ser_ser t2)
-    | tsum t1 t2 => sum_is_ser' v s (s_is_ser_ser t1) (s_is_ser_ser t2)
-    | toption t1 => option_is_ser' v s (s_is_ser_ser t1)
-    | tstring => string_is_ser v s
-    | tint => int_is_ser v s
-    | tauth => auth_is_ser v s
-    end. *)
-
   Fixpoint s_is_ser_deser (t : evi_type) (v : val) (s : string) : iProp Σ :=
     match t with
     | tprod t1 t2 => prod_is_ser' v s (s_is_ser_deser t1) (s_is_ser_deser t2)
@@ -490,388 +81,13 @@ Section authenticatable.
   #[global] Instance s_is_ser_proph_persistent t v s : Persistent (s_is_ser_proph t v s).
   Proof. revert v s. induction t => v s; simpl; apply _. Qed.
 
-  (* Fixpoint s_valid_val (t: evi_type) (v: val) : iProp Σ :=
-    match t with
-    | tprod t1 t2 => prod_valid_val' v (s_valid_val t1) (s_valid_val t2)
-    | tsum t1 t2 => sum_valid_val' v (s_valid_val t1) (s_valid_val t2)
-    | tstring => string_valid_val v
-    | tint => int_valid_val v
-    | tauth => auth_valid_val v
-    end.
-
-  #[global] Instance s_valid_val_persistent t v : Persistent (s_valid_val t v).
-  Proof. revert v. induction t => v; simpl; apply _. Qed.
-
-  Fixpoint s_deser_valid_val (dq : dfrac) (t : evi_type) (v : val) : iProp Σ :=
-    match t with
-    | tprod t1 t2 => prod_valid_val' v (s_deser_valid_val dq t1) (s_deser_valid_val dq t2)
-    | tsum t1 t2 => sum_valid_val' v (s_deser_valid_val dq t1) (s_deser_valid_val dq t2)
-    | tstring => string_valid_val v
-    | tint => int_valid_val v
-    | tauth => auth_deser_valid_val dq v
-    end.
-
-  Definition s_deser_valid_val_bef := s_deser_valid_val (DfracOwn (3/4)).
-
-  Definition s_deser_valid_val_aft := s_deser_valid_val (DfracOwn (1/2)). *)
-
-  (* Fixpoint s_deser_valid_val_tok (t : evi_type) (v : val) : iProp Σ :=
-    match t with
-    | tprod t1 t2 => prod_valid_val' v (s_deser_valid_val t1) (s_deser_valid_val t2)
-    | tsum t1 t2 => sum_valid_val' v (s_deser_valid_val t1) (s_deser_valid_val t2)
-    | tstring => string_valid_val v
-    | tint => int_valid_val v
-    | tauth => auth_deser_valid_val_tok v
-    end. *)
-
-  (* #[global] Instance s_valid_val_persistent t v: Persistent (s_valid_val t v).
-  Proof. revert v; induction t => v; simpl; apply _. Qed. *)
-
   #[global] Instance s_is_ser''_persistent t v s: Persistent (s_is_ser'' t v s).
   Proof. revert v s; induction t => v s; simpl; apply _. Qed.
 
-  (* Fixpoint susp_list (t : evi_type) (v : val) (susp_l : list loc) : iProp Σ :=
-    match t with
-    | tprod t1 t2 =>
-        ∃ v1 v2 susp_v1 susp_v2,
-          ⌜v = (v1, v2)%V ∧ susp_l = susp_v1 ++ susp_v2⌝ ∗ susp_list t1 v1 susp_v1 ∗ susp_list t2 v2 susp_v2
-    | tsum t1 t2 =>
-        ∃ v',
-          (⌜v = InjLV v'⌝ ∗ susp_list t1 v' susp_l) ∨ (⌜v = InjRV v'⌝ ∗ susp_list t2 v' susp_l) 
-    | tstring => ∃ (s: string), ⌜v = #s ∧ susp_l = []⌝
-    | tint => ∃ (i: nat), ⌜v = #i ∧ susp_l = []⌝
-    | tauth =>
-        (∃ v', ⌜v = SOMEV v'⌝ ∧
-                 ((∃ (h : string), ⌜v' = InjLV #h ∧ susp_l = []⌝) ∨ 
-                    (∃ (susp : loc), ⌜v' = InjRV #susp ∧ susp_l = [susp]⌝)))
-    end. *)
-
-  (* ((∃ b so, single_instance pid pt px pvᵥ so b) -∗ susp_in_v pt px susp) ∗ (* Parent's instance *)
-                          ((∃ aid ax avᵥ t, single_instance aid t ax avᵥ None true ∗ val_eq t ax avᵥ) -∗ (* Most recent pre-filled ancestor *)
-                             (∃ aid cx cvᵥ ct, single_instance aid ct cx cvᵥ (Some susp) false -∗ val_eq ct cx cvᵥ)) *)
-  
-  (* Lemma deser_ser_proph E t v s1 :
-    seq_tok E ∗ s_is_ser_deser t v s1 ==∗ seq_tok E ∗ ∃ s2, s_is_ser_proph t v s2.
-  Proof. Admitted. *)
-
-  (* Lemma deser_valid :
-    ∀ ct v vᵥ s ax avᵥ t px pvᵥ pt,
-      ⌜subeq_obj_bin px pvᵥ v vᵥ ⌝ -∗ □(val_eq t ax avᵥ -∗ val_eq pt px pvᵥ) -∗ s_is_ser_deser ct v s -∗ s_deser_valid_val_bef ct v.
-  Proof.
-    iIntros (??????????) "%Hsubeqbin #Heq_trans Hser".
-    pose proof (subeq_obj_bin_to_unary _ _ _ _ Hsubeqbin) as [Hsubeqx Hsubeqv].
-    iInduction ct as [| | | |] forall (v vᵥ s Hsubeqx Hsubeqv Hsubeqbin); iSimpl; iSimpl in "Hser".
-    - iDestruct "Hser" as (????) "((-> & ->) & H1 & H2)".
-      assert (H1: subeq_obj (v1, v2) v1).
-      { left. eexists (tprod ct1 ct2).
-        exists v1, v2. eauto. }
-      assert (H1': subeq_obj px v1).
-      { by apply (subeq_obj_trans px (v1, v2) v1). }
-      assert (H2: subeq_obj (v1, v2) v2).
-      { left. eexists (tprod ct1 ct2).
-        exists v1, v2. eauto. }
-      assert (H2': subeq_obj px v2).
-      { by apply (subeq_obj_trans px (v1, v2) v2). }
-      iPoseProof ("IHct1" with "[] [] [] H1") as "H1"; [done|done|admit| ].
-      iPoseProof ("IHct2" with "[] [] [] H2") as "H2"; [done|done|admit| ].
-      iExists v1, v2. by iFrame.
-    - iDestruct "Hser" as (??) "[(H & %)|(H & %)]".
-      + destruct H as [-> _]. iExists _. iLeft. iSplit; first done.
-        iPoseProof ("IHct1" with "[] [] [] H") as "H"; admit.
-      + destruct H as [-> _]. iExists _. iRight. iSplit; first done.
-        iPoseProof ("IHct2" with "[] [] [] H") as "H"; admit.
-    - iDestruct "Hser" as "%Hser". destruct Hser as (? & -> & _). iExists _. done.
-    - iDestruct "Hser" as "%Hser". destruct Hser as (? & -> & _). iExists _. done.
-    - iDestruct "Hser" as (? ->) "[(% & -> & Hser)|(%&% & -> & Hsusp & Hser)]".
-      + iExists _. iSplit; [done|].
-        iLeft. eauto.
-      + iExists _. iSplit; [done|].
-        iRight. iExists _. iSplit; [done|].
-        iDestruct (fractional_split _ (λ q, susp ↦{DfracOwn q} InjLV #pid)%I (3/4) (1/4) with "Hsusp") as "[Hsusp1 Hsusp2]".
-        { admit. }
-        iExists pid.
-        destruct Hsubeqx as [[ct Hsub]|Heq]; last first.
-        * iExists tauth, t, px, pvᵥ, ax, avᵥ. iFrame. iSplitL.
-          { iIntros "_". iExists _. iSplit; eauto. }
-          iIntros "(%ancid & _ & Hanceq)".
-          iExists vᵥ. iIntros "_".
-          iPoseProof ("Heq_trans" with "Hanceq") as "#Hpeq".
-          iPoseProof (val_eq_sub_eq with "[$Hpeq //]") as "#Heq".
-          iDestruct "Heq" as (?) "Heq".
-          destruct st.
-          { by iDestruct "Heq" as (????[? ->]) "_". }
-          { iDestruct "Heq" as (??) "[([%  %] & _)|([%  %] & Heq)]"; try done.
-            simplify_eq.
-            destruct st2.
-            { by iDestruct "Heq" as (????[? ->]) "_". }
-            { iDestruct "Heq" as (??) "[([%  %] & _)|([%  %] & Heq)]"; try done.
-              simplify_eq.
-              destruct st2_2; iSimpl in "Heq".
-              { by iDestruct "Heq" as (????[? ->]) "_". }
-              { by iDestruct "Heq" as (??) "[([%  %] & _)|([%  %] & Heq)]". }
-              { by iDestruct "Heq" as (?) "[% %]". }
-              { by iDestruct "Heq" as (?) "[% %]". }
-              { admit. } }
-            { by iDestruct "Heq" as (?) "[% %]". }
-            { by iDestruct "Heq" as (?) "[% %]". }
-            { iDestruct "Heq" as "[[% %]|(% & H)]"; try done.
-              admit. } }
-          { by iDestruct "Heq" as (?) "[% %]". }
-          { by iDestruct "Heq" as (?) "[% %]". }
-          { iFrame "#". }
-        * iExists pt, t, px, pvᵥ, ax, avᵥ. iFrame. iSplitL.
-          { iIntros "_". iApply (sub_obj_susp_in with "[$Hsusp2]"). admit. }
-          iIntros "Heq". iDestruct "Heq" as (?) "[_ Hanceq]".
-          iPoseProof ("Heq_trans" with "Hanceq") as "#Hpeq".
-          iPoseProof (val_eq_sub_eq with "[$Hpeq //]") as "#Heq".
-          iExists vᵥ. iIntros "_".
-          iDestruct "Heq" as (?) "Heq".
-          destruct st.
-          { by iDestruct "Heq" as (????[? ->]) "_". }
-          { iDestruct "Heq" as (??) "[([%  %] & _)|([%  %] & Heq)]"; try done.
-            simplify_eq.
-            destruct st2.
-            { by iDestruct "Heq" as (????[? ->]) "_". }
-            { iDestruct "Heq" as (??) "[([%  %] & _)|([%  %] & Heq)]"; try done.
-              simplify_eq.
-              destruct st2_2; iSimpl in "Heq".
-              { by iDestruct "Heq" as (????[? ->]) "_". }
-              { by iDestruct "Heq" as (??) "[([%  %] & _)|([%  %] & Heq)]". }
-              { by iDestruct "Heq" as (?) "[% %]". }
-              { by iDestruct "Heq" as (?) "[% %]". }
-              { admit. } }
-            { by iDestruct "Heq" as (?) "[% %]". }
-            { by iDestruct "Heq" as (?) "[% %]". }
-            { iDestruct "Heq" as "[[% %]|(% & H)]"; try done.
-              admit. } }
-          { by iDestruct "Heq" as (?) "[% %]". }
-          { by iDestruct "Heq" as (?) "[% %]". }
-          { iFrame "#". }
-  Admitted. *)
-      
-  (* Lemma evi_type_ser''_inj (t1 t2 : evi_type) v1 v2 s :
-    (s_is_ser'' t1 v1 s ∨ s_is_ser_proph t1 v1 s) -∗ s_is_ser'' t2 v2 s -∗ val_eq t1 v1 v2.
-  Proof.  *)
-    (* iInduction t1 as [| | | |] forall (t2 v1 v2 s).
-    - iIntros "Ht1 Ht2".
-      iDestruct "Ht1" as "[Ht1|Ht1]".
-      + iDestruct "Ht1" as (?????) "(Ht11 & Ht12)".
-        destruct H as [-> ->].
-        destruct t2 => /=; simplify_eq.
-        * iDestruct "Ht2" as (?????) "(Ht21 & Ht22)".
-          destruct H as [-> H]. simplify_eq.
-          iExists _, _, _, _. iSplit; [eauto|].
-          iPoseProof ("IHt1_2" with "[Ht12] Ht22") as "Ht32".
-          { by iLeft. }
-          iPoseProof ("IHt1_1" with "[Ht11] Ht21") as "Ht31".
-          { by iLeft. }
-          iFrame.
-        * iDestruct "Ht2" as (??) "[(Ht2&%)|(Ht2&%)]";
-            destruct H; simplify_eq.
-          { exfalso. by eapply prod_ser_inl_ser_neq. }
-          { exfalso. by eapply prod_ser_inr_ser_neq. }
-        * iDestruct "Ht2" as (?) "(%&%)".
-          iExFalso. by eapply prod_ser_string_ser_neq in H0.
-         * iDestruct "Ht2" as (?) "(%&%)".
-          iExFalso. by eapply prod_ser_int_ser_neq in H0.
-        * admit.
-      + iDestruct "Ht1" as (?????) "(Ht11 & Ht12)".
-        destruct H as [-> ->].
-        destruct t2 => /=; simplify_eq.
-        * iDestruct "Ht2" as (?????) "(Ht21 & Ht22)".
-          destruct H as [-> H]. simplify_eq.
-          iExists _, _, _, _. iSplit; [eauto|].
-          iPoseProof ("IHt1_2" with "[Ht12] Ht22") as "Ht32".
-          { by iRight. }
-          iPoseProof ("IHt1_1" with "[Ht11] Ht21") as "Ht31".
-          { by iRight. }
-          iFrame.
-        * iDestruct "Ht2" as (??) "[(Ht2&%)|(Ht2&%)]";
-            destruct H; simplify_eq.
-          { exfalso. by eapply prod_ser_inl_ser_neq. }
-          { exfalso. by eapply prod_ser_inr_ser_neq. }
-        * iDestruct "Ht2" as (?) "(%&%)".
-          iExFalso. by eapply prod_ser_string_ser_neq in H0.
-        * iDestruct "Ht2" as (?) "(%&%)".
-          iExFalso. by eapply prod_ser_int_ser_neq in H0.
-        * admit.
-    - admit.
-    - admit.
-    - admit.
-    - iIntros "Ht1 Ht2".
-      iDestruct "Ht1" as "[Ht1|Ht1]".
-      + iDestruct "Ht1" as (?->) "[Ht1|Ht1]".
-        * iDestruct "Ht1" as (?) "(-> & Ht1)".
-          destruct t2 => /=; simplify_eq.
-          -- iDestruct "Ht1" as "[(% & ->)|(% & % & (% & %) & Hser)]"; [done|].
-             simplify_eq.
-             iDestruct "Ht2" as (?????) "(Ht21 & Ht22)".
-             destruct H as [-> H].
-             simplify_eq.
-             exfalso. by eapply prod_ser_some_ser_neq.
-          -- iDestruct "Ht1" as "[(% & ->)|(% & % & (% & %) & Hser)]"; [done|].
-             simplify_eq.
-             iDestruct "Ht2" as (??) "[(Ht2&%)|(Ht2&%)]";
-               destruct H; simplify_eq.
-          -- iDestruct "Ht1" as "[(% & ->)|(% & % & (% & %) & (% & -> & ->))]"; [done|].
-             simplify_eq.
-             iDestruct "Ht2" as (?) "(%&%)". simplify_eq.
-          -- iDestruct "Ht1" as "[(% & ->)|(% & % & (% & %) & (% & -> & ->))]"; [done|].
-             simplify_eq.
-             iDestruct "Ht2" as (?) "(%&%)". simplify_eq.
-          -- iDestruct "Ht1" as "[(% & ->)|(% & % & (% & %) & (% & -> & ->))]"; [done|].
-             simplify_eq.
-             iDestruct "Ht2" as (?->) "[(% & -> & Ht2)|(%& ->& %& #Hloc & Ht2)]"; iFrame.
-             { iDestruct "Ht2" as "[(% & %)|(% & % & (% & %) & (% & -> & ->))]"; [done|].
-               simplify_eq. iRight. iExists _. iSplit; iLeft; eauto. }            
-             iRight. iExists _. iSplit.
-             { iLeft. eauto. }
-             iDestruct "Ht2" as "[(% & %)|(% & % & (% & %) & (% & % & %))]"; simplify_eq.
-             iRight. iExists _. eauto.
-        * iDestruct "Ht1" as (?->?) "(Hloc & Ht1)".
-          destruct t2 => /=; simplify_eq.
-          -- iDestruct "Ht1" as "[(% & ->)|(% & % & (% & %) & Hser)]"; [done|].
-             simplify_eq.
-             iDestruct "Ht2" as (?????) "(Ht21 & Ht22)".
-             destruct H as [-> H].
-             simplify_eq.
-             exfalso. by eapply prod_ser_some_ser_neq.
-          -- iDestruct "Ht1" as "[(% & ->)|(% & % & (% & %) & Hser)]"; [done|].
-             simplify_eq.
-             iDestruct "Ht2" as (??) "[(Ht2&%)|(Ht2&%)]";
-               destruct H; simplify_eq.
-          -- iDestruct "Ht1" as "[(% & ->)|(% & % & (% & %) & (% & -> & ->))]"; [done|].
-             simplify_eq.
-             iDestruct "Ht2" as (?) "(%&%)". simplify_eq.
-          -- iDestruct "Ht1" as "[(% & ->)|(% & % & (% & %) & (% & -> & ->))]"; [done|].
-             simplify_eq.
-             iDestruct "Ht2" as (?) "(%&%)". simplify_eq.
-          -- iDestruct "Ht1" as "[(% & ->)|(% & % & (% & %) & (% & -> & ->))]"; [done|].
-             simplify_eq.
-             iDestruct "Ht2" as (?->) "[(% & -> & Ht2)|(%& -> & %& #Hloc1 & Ht2)]"; iFrame.
-             { iDestruct "Ht2" as "[(% & %)|(% & % & (% & %) & (% & -> & ->))]"; [done|].
-               simplify_eq. iRight. iExists _. iSplit; [iRight|iLeft]; eauto. }
-             iRight. iExists _. iSplit.
-             { iRight. eauto. }
-             iRight. iExists _. iSplit; first done.
-             iDestruct "Ht2" as "[(% & %)|(% & % & (% & %) & (% & % & %))]"; by simplify_eq.
-      + iDestruct "Ht1" as (?->) "[Ht1|Ht1]".
-        * iDestruct "Ht1" as (?) "(-> & Ht1)".
-          destruct t2 => /=; simplify_eq.
-          -- iDestruct "Ht1" as "[(% & ->)|(% & % & (% & %) & Hser)]"; [done|].
-             simplify_eq.
-             iDestruct "Ht2" as (?????) "(Ht21 & Ht22)".
-             destruct H as [-> H].
-             simplify_eq.
-             exfalso. by eapply prod_ser_some_ser_neq.
-          -- iDestruct "Ht1" as "[(% & ->)|(% & % & (% & %) & Hser)]"; [done|].
-             simplify_eq.
-             iDestruct "Ht2" as (??) "[(Ht2&%)|(Ht2&%)]";
-               destruct H; simplify_eq.
-          -- iDestruct "Ht1" as "[(% & ->)|(% & % & (% & %) & (% & -> & ->))]"; [done|].
-             simplify_eq.
-             iDestruct "Ht2" as (?) "(%&%)". simplify_eq.
-          -- iDestruct "Ht1" as "[(% & ->)|(% & % & (% & %) & (% & -> & ->))]"; [done|].
-             simplify_eq.
-             iDestruct "Ht2" as (?) "(%&%)". simplify_eq.
-          -- iDestruct "Ht1" as "[(% & ->)|(% & % & (% & %) & (% & -> & ->))]"; [done|].
-             simplify_eq.
-             iDestruct "Ht2" as (?->) "[(% & -> & Ht2)|(%& ->& %& #Hloc & Ht2)]"; iFrame.
-             { iDestruct "Ht2" as "[(% & %)|(% & % & (% & %) & (% & -> & ->))]"; [done|].
-               simplify_eq. iRight. iExists _. iSplit; iLeft; eauto. }            
-             iRight. iExists _. iSplit.
-             { iLeft. eauto. }
-             iDestruct "Ht2" as "[(% & %)|(% & % & (% & %) & (% & % & %))]"; simplify_eq.
-             iRight. iExists _. eauto.
-        * iDestruct "Ht1" as (? -> ???) "(Hloc & Hproph & Ht1)".
-          destruct t2 => /=; simplify_eq.
-          -- iDestruct "Ht1" as "[(% & ->)|(% & % & (% & %) & Hser)]"; [|done].
-             simplify_eq.
-             iDestruct "Ht2" as (?????) "(Ht21 & Ht22)".
-             destruct H as [-> H].
-             exfalso. by eapply prod_ser_none_ser_neq.
-          -- iDestruct "Ht1" as "[(% & ->)|(% & % & (% & %) & Hser)]"; [|done].
-             simplify_eq.
-             iDestruct "Ht2" as (??) "[(Ht2&%)|(Ht2&%)]";
-               destruct H; simplify_eq.
-          -- iDestruct "Ht1" as "[(% & ->)|(% & % & (% & %) & (% & -> & ->))]"; [|done].
-             simplify_eq.
-             iDestruct "Ht2" as (?) "(%&%)". simplify_eq.
-          -- iDestruct "Ht1" as "[(% & ->)|(% & % & (% & %) & (% & -> & ->))]"; [|done].
-             simplify_eq.
-             iDestruct "Ht2" as (?) "(%&%)". simplify_eq.
-          -- iDestruct "Ht1" as "[(% & ->)|(% & % & (% & %) & (% & -> & ->))]"; [|done].
-             simplify_eq.
-             iDestruct "Ht2" as (?->) "[(% & -> & Ht2)|(%& -> & %& #Hloc1 & Ht2)]"; iFrame;
-               iDestruct "Ht2" as "[(% & %)|(% & % & (% & %) & (% & -> & ->))]"; done. *)
-
-  (* Lemma deser_valid_weak :
-    ∀ t v, s_deser_valid_val_aft t v ⊢ |={⊤}=> s_valid_val t v.
-  Proof.
-    iIntros (??) "Hdvalid".
-    iInduction t as [| | | |] forall (v); iSimpl; iSimpl in "Hdvalid".
-    - iDestruct "Hdvalid" as (??->) "[H1 H2]".
-      iPoseProof ("IHt1" with "H1") as "H1".
-      iPoseProof ("IHt2" with "H2") as "H2".
-      iExists v1, v2.
-      iMod "H1". iMod "H2".
-      iModIntro. iSplit; [done|iFrame].
-    - iDestruct "Hdvalid" as (?) "[[-> H]|[-> H]]".
-      + iPoseProof ("IHt1" with "H") as "H". iMod "H".
-        iModIntro. iExists _. iLeft. iSplit; [done|iExact "H"].
-      + iPoseProof ("IHt2" with "H") as "H". iMod "H".
-        iModIntro. iExists _. iRight. iSplit; [done|iExact "H"].
-    - by iModIntro.
-    - by iModIntro.
-    - iDestruct "Hdvalid" as (? ->) "[(% & ->)|(%&-> & %&%&%&%&%&%&% & Hsusp & Hsuspin & Heq)]".
-      + iExists _. iModIntro. iSplit; [done|].
-        iLeft. eauto.
-      + iExists _.
-        iMod (na_inv_alloc seqG_name _ (authValidN #susp) (valid_auth_inv susp) with "[Hsusp Hsuspin Heq]") as "Hinv".
-        { iNext. iRight. iFrame. }
-        iModIntro.
-        iSplit; [done|].
-        iRight. eauto.
-  Qed. *)
-        
   #[global] Instance : Inhabited evi_type.
   Proof. constructor. apply tstring. Qed.
 
-  (* Definition count_auth_inv (susp: loc) (c: nat) : iProp Σ :=
-     ((∃ (h : string), susp ↦□ (InjRV #h) ∗ ⌜c = 0⌝) ∨
-        (∃ (pid : nat), susp ↦ (InjLV #pid) ∗ ⌜c = 1⌝)). *)
-
-(*  Lemma count_valid t v :
-    ∀ E1 c, ∃ E2, seq_tok E1 ∗ count_is_correct t v c  ={E1,E2}=∗ seq_tok E2 ∗ s_valid_val t v.
-  Proof.
-    iIntros (?). eexists _. iIntros "(Htok & Hcount)".
-    iInduction t as [| | | |] forall (E1 v c); iSimpl; iSimpl in "Hcount".
-    - iDestruct "Hcount" as (???? -> ) "(Hcount1 & Hcount2 & %)". simplify_eq.
-      iPoseProof ("IHt1" with "Htok Hcount1") as "H1".
-      iMod "H1" as "(Htok & H1)".
-      iPoseProof ("IHt2" with "Htok Hcount2") as "H2".
-      iMod "H2" as "(Htok & H2)". iFrame.
-      iModIntro. iFrame. eauto.
-    - iDestruct "Hcount" as "[(%&->&Hcount)|(%&->&Hcount)]".
-      + iPoseProof ("IHt1" with "Htok Hcount") as "H".
-        iMod "H" as "(Htok & H)". iFrame.
-        iModIntro. iExists _. iLeft. eauto.
-      + iPoseProof ("IHt2" with "Htok Hcount") as "H".
-        iMod "H" as "(Htok & H)". iFrame.
-        iModIntro. iExists _. iRight. eauto.
-    - iFrame. by iDestruct "Hcount" as "(H&%)".
-    - iFrame. by iDestruct "Hcount" as "(H&%)".
-    - iFrame. iDestruct "Hcount" as (??) "[(%&->&->)|(%&->&Hsusp)]".
-      + iModIntro. iExists _. iSplit; [done|]. eauto.
-      + iExists _.
-        iMod (na_inv_acc with "Hsusp") as "Hinv". *)
-
-  (* Definition count_update (t : evi_type) : iProp Σ :=
-    ∀ (v : val) (susp : loc) (c pid : nat) (h : string),
-      {{{ susp ↦{#1/2} InjLV #pid ∗ susp_in_v t v susp ∗ count_is_correct t v c }}}
-        #susp <- InjR #h
-        {{{ RET #(); count_is_correct t v (c-1) ∗ susp ↦□ InjRV #h }}}. *)
-                                                 
+                                               
   Definition ser_spec_3 (ser : val) (t : evi_type) : iProp Σ :=
     ∀ (v1 : val) (s : string) E,
       ⌜↑authSet N ⊆ E⌝ -∗
@@ -879,13 +95,6 @@ Section authenticatable.
         ser v1
       {{{ o, RET $o; seq_tok E ∗ ((⌜o = Some #s⌝ ∗ s_is_ser'' t v1 s) ∨ ⌜o = None⌝) }}}.
         
-                                                 
-  (* Definition ser_spec_2 (ser : val) (t : evi_type) : iProp Σ :=
-    ∀ (v1 : val),
-      {{{ ▷ (s_valid_val t v1 ∗ seq_tok ⊤) }}}
-        ser v1
-        {{{ o, RET $o; seq_tok ⊤ ∗ if o is Some s then s_is_ser'' t v1 s else True }}}. *)
-  
   Definition ser_spec_un (A : lrel_un Σ) (ser : val) (t : evi_type) : iProp Σ :=
     ∀ (v : val) E,
       ⌜↑authSet N ⊆ E⌝ -∗
@@ -900,7 +109,6 @@ Section authenticatable.
         ser v1
       {{{ o, RET $o; seq_tok E ∗ if o is Some s then s_is_ser'' t v1 s else True }}}.
 
-  (* Pass single_instance through here, and set it in s_is_ser_deser. Or maybe do it in count. *)
   Definition deser_spec (A : lrel_un Σ) (deser : val) (t : evi_type) : iProp Σ :=
     ∀ (pid : nat),
       {{{ True }}}
@@ -916,34 +124,12 @@ Section authenticatable.
                   else True }}}
       }}}.
   
-  (* Definition deser1_spec (deser_partial : val) (t : evi_type) : iProp Σ :=
-    ∀ (s : string),
-      ({{{ True }}}
-         deser_partial #s
-      {{{ o, RET $o; if o is Some v then s_is_ser_deser t v s else True }}}). *)
-
   Definition count_spec (count : val) (t : evi_type) : iProp Σ :=
     ∀ (x : val) (s : string) (E : coPset),
       ⌜↑authSet N ⊆ E⌝ →
-      {{{ ▷ (s_is_ser_proph t x s ∗ seq_tok E) }}}
+      {{{ (s_is_ser_proph t x s ∗ seq_tok E) }}}
         count x
       {{{ (c : nat), RET #c; s_is_ser_proph t x s ∗ seq_tok E }}}.
-
-  (* Definition val_eq_rel_un (A : lrel_un Σ) : iProp Σ :=
-    ∀ (E : coPset) (v1 v2 : val) (s : string) (t1 t2 : evi_type),
-        ⌜↑authSet N ⊆ E⌝ →
-        □ (seq_tok E -∗ (s_is_ser'' t1 v1 s ∨ s_is_ser_proph t1 v1 s) -∗ 
-            s_is_ser'' t2 v2 s -∗ A v2 ={⊤}=∗ 
-              seq_tok E ∗ A v1). *)
-
-    (* ∀ (a1 a2 : val) (E : coPset),
-      ⌜↑authSet N ⊆ E⌝ →
-      □ (seq_tok E ∗ val_eq t a1 a2 ∗ A a1 ={⊤}=∗ A a2 ∗ seq_tok E). *)
-
-  (* Definition val_eq_rel (A : lrel Σ) (t: evi_type) : iProp Σ :=
-    ∀ (a1 a2 b1: val) (E : coPset),
-      ⌜↑authSet N ⊆ E⌝ →
-      □ (seq_tok E ∗ val_eq t a1 a2 ∗ A a1 b1 ={⊤}=∗ A a2 b1 ∗ seq_tok E). *)
 
   Definition val_eq_rel (A : lrel Σ) : iProp Σ :=
     ∀ (E : coPset) (v1 v2 b1 : val) (s : string) (t1 t2 : evi_type),
@@ -951,6 +137,7 @@ Section authenticatable.
       □ (seq_tok E -∗ (s_is_ser'' t1 v1 s ∨ s_is_ser_proph t1 v1 s) -∗ 
           s_is_ser'' t2 v2 s -∗ A v2 b1 ={⊤}=∗ 
             seq_tok E ∗ A v1 b1).
+
 
   Definition lrel_un_evidence' (A : lrel_un Σ) : lrel_un Σ :=
     LRelUn (λ v,
@@ -960,9 +147,6 @@ Section authenticatable.
   
   Definition lrel_bin_evidence' (A : lrel_bi Σ) : lrel Σ :=
     LRel (λ v1 v2, val_eq_rel A)%I.
-        (* ∃ (t : evi_type) (ser deser count : val),
-          ⌜v1 = (ser, deser, count)%V⌝ ∗ ser_spec A ser t ∗ ser_spec_3 ser t ∗
-            (* count_spec count t ∗ deser_spec deser t ∗ *) val_eq_rel A)%I. *)
 
   Definition lrel_bi_evidence' (A : lrel_bi Σ) : lrel_bi Σ :=
     LRelBi (lrel_un_evidence' (lrel_bi_un A))
@@ -1190,163 +374,7 @@ Section proof.
                   iSplit.
                   { interp_unfold!. iFrame "∗ #". done. }
                   rewrite interp_un_prod_unfold. interp_unfold!. iFrame "∗ #". done. }
-
-              (* iExists (tprod tA tB), _, _, _.
-              iSplit; [done|]. clear. iSplit; [|iSplit; [|iSplit; [|iSplit]]].
-              + iIntros (v1 v2 ???) "!# (Hp' & Htok) H".
-                iDestruct "Hp'" as "[Hp Hp_un]". repeat interp_unfold.
-                iDestruct "Hp" as (w1 w2 u1 u2) "(>-> & >-> & #HA & #HB)".
-                rewrite interp_un_prod_unfold. repeat interp_unfold.
-                iDestruct "Hp_un" as (??) "(>% & #Hpa_un & #Hpb_un)".
-                simplify_eq. iSimpl in "H".
-                wp_apply (prod_ser'_spec_ser (λ v1, A v1 w2) (λ v1, B v1 u2) with "[] [] [] [$Htok]") => /=; [done| | | |done].  
-                { iIntros (?) "!# Hp H". by wp_apply ("HserA" with "[//] Hp"). }
-                { iIntros (?) "!# Hp H". by wp_apply ("HserB" with "[//] Hp"). }
-                iExists _, _. iModIntro. iSplit; first done. iFrame "#".
-              (* - iIntros (v1 ?) "!# (Hp & Htok) H". iSimpl in "Hp".
-      iDestruct "Hp" as (w1 w2) "(>-> & HA & HB)".
-      wp_apply (prod_ser'_spec_ser (s_valid_val _ tA) (s_valid_val _ tB) with "[] [] [] [HA HB $Htok]") => /=; [done| | | |done].  
-      { iIntros (?) "!# Hp H". by wp_apply ("Hser2A" with "Hp"). }
-      { iIntros (?) "!# Hp H". by wp_apply ("Hser2B" with "Hp"). }
-      iNext. iFrame. eauto. *)
-              + iIntros (v ???) "!# (Hser & Htok) H".
-                iDestruct "Hser" as (????) "((>-> & >->) & HA & HB)". admit.
-                (* wp_apply (prod_ser'_spec_ser (λ v1, s_is_ser_proph N tA v1 s1) (λ v2, s_is_ser_proph N tB v2 s2) with "[] [] [] [HA HB $Htok]") => /=; [done| | | |done].
-                { iIntros (?) "!# Hser H". by wp_apply ("Hser3A" with "[//] Hser"). }
-                { iIntros (?) "!# Hser H". by wp_apply ("Hser3B" with "[//] Hser"). }
-                iNext. iFrame. eauto. *)
-              + iIntros (???) "!# Hser HΨ".  wp_pures.
-                iDestruct "Hser" as (????) "((-> & ->) & HA & HB)".
-                wp_pures. rewrite /count_spec.
-                wp_bind (countB _).
-                wp_apply ("HcountB" $! v2 with "HB").
-                iIntros (?) "HB".
-                wp_pures.
-                wp_apply ("HcountA" $! v1 with "HA").
-                iIntros (?) "HA".
-                simplify_eq. wp_pures. iModIntro.
-                iSpecialize ("HΨ" $! (c0+c)).
-                assert (#(c0 + c) = #(c0 + c)%nat).
-                { by rewrite Nat2Z.inj_add. }
-                rewrite H. iApply "HΨ".
-                by iFrame.
-              + iIntros (pid ?) "!# _ HΨ".
-                wp_pures.
-                wp_apply "HdeserB"; [done|]. iIntros "%deparB #HdeparB".
-                wp_apply "HdeserA"; [done|]. iIntros "%deparA #HdeparA".
-                rewrite /prod_deser.
-                wp_pures. iModIntro. iApply "HΨ".
-                iIntros (s ?) "!# _ HΨ".
-                wp_apply prod_deser'_sound; try auto.
-              (* iIntros ([]); last first.
-      { iIntros "_". by iApply ("HΨ" $! None). }
-      iIntros "(%&%&%&%&[-> ->] & (Hsera & (% & Hserpa)) & Hserb & (% & Hserpb))".
-      iApply ("HΨ" $! (Some _)). iFrame. eauto. *)
-              + iIntros (E v1 v2 b1 s t1 t2) "%HE !# Htok Hser1 Hser2 HA".
-                interp_unfold!.
-                iDestruct "HA" as (w1 w2 u1 u2) "(-> & -> & #HA & #HB)".
-                interp_unfold! in "HA".
-                interp_unfold! in "HB".
-                destruct t2 as [t2A t2B | t2A t2B | | |]; iSimpl in "Hser2".
-                all: try (iDestruct "Hser2" as %(? & Habs & ?); done).
-                2: { iDestruct "Hser2" as "(%w & %s' & [(_ & [%Hv _]) | (_ & [%Hv _])])"; done. }
-                2: { iDestruct "Hser2" as (?) "[%Hv _]"; done. }
-                iDestruct "Hser2" as (x1 x2 s1 s2) "[%Hpq [HS21 HS22]]".
-                destruct Hpq as [Hv Hs]. simplify_eq.
-                iDestruct "Hser1" as "[Hser1|Hser1]"; destruct t1 as [t1A t1B | t1A t1B | | |]; iSimpl in "Hser1".
-                all: try (iDestruct "Hser1" as %(? & ? & Habs); exfalso;
-                          first [exact (prod_ser_string_ser_neq _ s1 s2 Habs) |
-                                 exact (prod_ser_int_ser_neq _ s1 s2 Habs)]).
-                2: { iDestruct "Hser1" as "(%w & %s' & [(_ & [%Hv %Habs]) | (_ & [%Hv %Habs])])".
-                     - exfalso. exact (prod_ser_inl_ser_neq s' s1 s2 Habs).
-                     - exfalso. exact (prod_ser_inr_ser_neq s' s1 s2 Habs). }
-                4: { iDestruct "Hser1" as "(%w & %s' & [(_ & [%Hv %Habs]) | (_ & [%Hv %Habs])])".
-                     - exfalso. exact (prod_ser_inl_ser_neq s' s1 s2 Habs).
-                     - exfalso. exact (prod_ser_inr_ser_neq s' s1 s2 Habs). }
-                2: { iDestruct "Hser1" as (v0 ?) "[Hauth | (%susp & ? & Hauth)]".
-                     - iDestruct "Hauth" as (h ?) "Hser".
-                       iPoseProof (auth_scheme.(s_is_ser_eq) with "Hser") as "#Hstr".
-                       iDestruct "Hstr" as "[%Habs | (%s' & %Habs & _)]".
-                       + exfalso. exact (prod_ser_none_ser_neq s1 s2 Habs).
-                       + exfalso. exact (prod_ser_some_ser_neq _ s1 s2 Habs).
-                     - iDestruct "Hauth" as (h) "[_ Hser]".
-                       iPoseProof (auth_scheme.(s_is_ser_eq) with "Hser") as "#Hstr".
-                       iDestruct "Hstr" as "[%Habs | (%s' & %Habs & _)]".
-                       + exfalso. exact (prod_ser_none_ser_neq s1 s2 Habs).
-                       + exfalso. exact (prod_ser_some_ser_neq _ s1 s2 Habs). }
-                3: { iDestruct "Hser1" as (v0 ?) "[Hauth | (%susp & ? & [Hauth | Hauth])]".
-                     - iDestruct "Hauth" as (h ?) "Hser".
-                       iPoseProof (auth_scheme.(s_is_ser_eq) with "Hser") as "#Hstr".
-                       iDestruct "Hstr" as "[%Habs | (%s' & %Habs & _)]".
-                       + exfalso. exact (prod_ser_none_ser_neq s1 s2 Habs).
-                       + exfalso. exact (prod_ser_some_ser_neq _ s1 s2 Habs).
-                     - iDestruct "Hauth" as (h) "[_ Hser]".
-                       iPoseProof (auth_scheme.(s_is_ser_eq) with "Hser") as "#Hstr".
-                       iDestruct "Hstr" as "[%Habs | (%s' & %Habs & _)]".
-                       + exfalso. exact (prod_ser_none_ser_neq s1 s2 Habs).
-                       + exfalso. exact (prod_ser_some_ser_neq _ s1 s2 Habs).
-                     - iDestruct "Hauth" as (?? h) "[_ [_ Hser]]".
-                       iPoseProof (auth_scheme.(s_is_ser_eq) with "Hser") as "#Hstr".
-                       iDestruct "Hstr" as "[%Habs | (%s' & %Habs & _)]".
-                       + exfalso. exact (prod_ser_none_ser_neq s1 s2 Habs).
-                       + exfalso. exact (prod_ser_some_ser_neq _ s1 s2 Habs). }
-                * iDestruct "Hser1" as (y1 y2 s1' s2') "[%Hpq [HT1 HT2]]".
-                  destruct Hpq as [Hv Hs]. apply (inj2 prod_ser_str) in Hs as [<- <-]. subst v1.
-                  iPoseProof ("HrelA" with "[//] Htok [HT1] HS21 HA") as "> (Htok & #HA')".
-                  { by iLeft. }
-                  iPoseProof ("HrelB" with "[//] Htok [HT2] HS22 HB") as "> (Htok & #HB')".
-                  { by iLeft. }
-                  iModIntro. iFrame "Htok".
-                  iDestruct "HA'" as "[HA'b HA'u]". iDestruct "HB'" as "[HB'b HB'u]".
-                  iSplit.
-                  { interp_unfold!. iFrame "∗ #". done. }
-                  rewrite interp_un_prod_unfold. interp_unfold!. iFrame "∗ #". done.
-                * iDestruct "Hser1" as (y1 y2 s1' s2') "[%Hpq [HT1 HT2]]".
-                  destruct Hpq as [Hv Hs]. apply (inj2 prod_ser_str) in Hs as [<- <-]. subst v1.
-                  iPoseProof ("HrelA" with "[//] Htok [HT1] HS21 HA") as "> (Htok & #HA')".
-                  { by iRight. }
-                  iPoseProof ("HrelB" with "[//] Htok [HT2] HS22 HB") as "> (Htok & #HB')".
-                  { by iRight. }
-                  iModIntro. iFrame "Htok".
-                  iDestruct "HA'" as "[HA'b HA'u]". iDestruct "HB'" as "[HB'b HB'u]".
-                  iSplit.
-                  { interp_unfold!. iFrame "∗ #". done. }
-                  rewrite interp_un_prod_unfold. interp_unfold!. iFrame "∗ #". done. } *)
-                  (* iModIntro. iFrame "Htok". interp_unfold!. iFrame "∗ #". done. } *)
-                (* iIntros (??????) "!# Htok Hser1 Hser2 HA". interp_unfold.
-                iDestruct "HA" as (w1 w2 u1 u2) "(-> & -> & #HA & #HB)".
-                interp_unfold! in "HA".
-                interp_unfold! in "HB".
-                iDestruct "Hser1" as "[Hser1|Hser1]".
-                * iDestruct "Hser1" as (????[??]) "[Hser11 Hser12]".
-                  iDestruct "Hser2" as (????[??]) "[Hser21 Hser22]".
-                  simplify_eq.
-                  iPoseProof ("HrelA" with "[//] Htok [Hser11] Hser21 HA") as "> (Htok & #HA')".
-                  { by iLeft. }
-                  iPoseProof ("HrelB" with "[//] Htok [Hser12] Hser22 HB") as "> (Htok & #HB')".
-                  { by iLeft. }
-                  interp_unfold!. iFrame "∗ #". done.
-                * iDestruct "Hser1" as (????[??]) "[Hser11 Hser12]".
-                  iDestruct "Hser2" as (????[??]) "[Hser21 Hser22]".
-                  simplify_eq.
-                  iPoseProof ("HrelA" with "[//] Htok [Hser11] Hser21 HA") as "> (Htok & #HA')".
-                  { by iRight. }
-                  iPoseProof ("HrelB" with "[//] Htok [Hser12] Hser22 HB") as "> (Htok & #HB')".
-                  { by iRight. }
-                  interp_unfold!. iFrame "∗ #". done. } *)
-
-                (* iSimpl in "Heq".
-                iDestruct "Heq" as (???? H1) "(HeqA & HeqB)".
-                destruct H1. simplify_eq.
-                interp_unfold! in "HA".
-                interp_unfold! in "HB".
-                iPoseProof ("HrelA" with "[//] [$HeqA HA $Htok]") as "> (HArel & Htok)"; first iExact "HA".
-                iPoseProof ("HrelB" with "[//] [$HeqB HB $Htok]") as "> (HBrel & $)"; first iExact "HB".
-                do 4 iExists _. iModIntro. do 2 (iSplit; [eauto|]).
-                interp_unfold. interp_unfold.
-                iFrame. } *)
-            { iApply (refines_un_Auth_pair with "HA HB"). }
-          }
+            { iApply (refines_un_Auth_pair with "HA HB"). } }
           { iPoseProof "HA" as (tA_un serA_un deserA_un countA_un ?) "(#HserA_un & #Hser3A_un & #HcountA_un & #HdeserA_un)".
             rewrite interp_un_arr_unfold.
             iIntros (?) "!# #HB".
@@ -1356,8 +384,7 @@ Section proof.
             wp_pures.
             rewrite /prod_ser'' /prod_count.
             wp_pures. iFrame. iModIntro.
-            iApply (refines_un_Auth_pair with "HA HB"). }
-        }
+            iApply (refines_un_Auth_pair with "HA HB"). } }
         { rewrite interp_un_arr_unfold.
           iIntros (?) "!# #HA".
           interp_unfold! in "HA".
@@ -1373,8 +400,7 @@ Section proof.
           wp_pures.
           rewrite /prod_ser'' /prod_count.
           wp_pures. iFrame. iModIntro.
-          iApply (refines_un_Auth_pair with "HA HB"). }
-      }
+          iApply (refines_un_Auth_pair with "HA HB"). } }
       { rewrite interp_un_forall_unfold.
         iIntros (B ??) "!# Htok".
         wp_pures.
@@ -1422,21 +448,6 @@ Section proof.
       iApply (refines_un_Auth_pair with "HA HB").
   Qed.
       
-            
-    (* - iIntros (??????) "!# (Hsusp & Hin & Hc) HΦ".
-      iSimpl in "Hin Hc".
-      iDestruct "Hin" as (??) "[% [HinA|HinB]]";
-        iDestruct "Hc" as (????) "((% & %) & [HcA HcB])";
-        simplify_eq.
-      + iPoseProof (count_gt0 with "[$HinA $HcA]") as (?) "[HinA HcA]".
-        wp_apply ("HcupdA" with "[$Hsusp $HinA $HcA]").
-        iIntros "[Hc Hsusp]". iApply "HΦ". iFrame.
-        iPureIntro. split; [done|lia].
-      + iPoseProof (count_gt0 with "[$HinB $HcB]") as (?) "[HinB HcB]".
-        wp_apply ("HcupdB" with "[$Hsusp $HinB $HcB]").
-        iIntros "[Hc Hsusp]". iApply "HΦ". iFrame.
-        iPureIntro. split; [done|lia]. *)
-  
   Lemma refines_Auth_sum Θ (Δ : ctxO Σ Θ) :
     ⊢ ⟦ ∀: ⋆; ⋆, var2 var1 → var2 var0 → var2 (var1 + var0) ⟧
       (ext Δ (lrel_evidence N)) v_Auth_sum i_Auth_sum.
@@ -1502,38 +513,14 @@ Section proof.
         iIntros (??) "(Hi & Htok)".
         interp_unfold! in "H".
         iDestruct "H" as "[Hrel H]".
-        iPoseProof "H" as "(%t & %ser & %deser & %count & -> & #Hser & #Hser3 & #Hcount & #Hdeser)".
+        iPoseProof "H" as "(%t & %ser & %deser & %count & -> & H')".
         i_pures. wp_pures.
         iFrame. iModIntro.
         iSplit; interp_unfold!.
-        * admit. 
-          (* iExists t, _, _, _. iSplit; [done|].
-          clear. iSplit; [|iSplit]; [| |iSplit; [|iSplit]].
-          -- iIntros (v1 v2 ?? Ψ) "!# (#[Hs Hs_un] & Htok) HΨ".
-             wp_pures.
-             rewrite interp_rec_star_bin_unfold.
-             rewrite interp_rec_star_un_unfold.
-             rewrite interp_unseal /=.
-             wp_apply ("Hser" with "[//] [$Htok]"); [by iFrame "#"|done].
-          (* - iIntros (v1 Ψ) "!# (Hs & Htok) HΨ".
-      wp_pures.
-      wp_apply ("Hser2" with "[Hs Htok]"); [by iFrame|done]. *)
-          -- iIntros (v1 ?? Ψ) "!# (Hs & Htok) HΨ".
-             wp_pures.
-             by wp_apply ("Hser3" with "[$Hs $Htok]").
-          -- iIntros (???) "!# Hp HΨ". wp_pures.
-             by iApply ("Hcount" with "Hp").
-          -- iIntros (pid Ψ) "!# _ HΨ". wp_pures.
-             iApply "HΨ". iModIntro.
-             iIntros (s ?) "!# _ HΨ". wp_pures.
-             wp_apply "Hdeser"; [done|].
-             iIntros (depar) "HΨ1".
-             iApply "HΨ1"; [done|].
-             iModIntro.
-             iIntros ([]) "H"; last first.
-             { by iApply "HΨ". }
-             by iApply "HΨ".
-          -- admit. *)
+        * iIntros (????????) "!# Htok Hser Hser' #Hmu". 
+          rewrite interp_rec_star_unfold.
+          rewrite interp_unseal /=.
+          admit.
         * iApply (refines_un_Auth_mu with "H").
       + rewrite interp_un_arr_unfold.
         iIntros (?) "!# #H Htok".
@@ -1558,15 +545,7 @@ Section proof.
       interp_unfold!.
       iApply (refines_un_Auth_mu with "H").
   Admitted.
-
-  (* Remove suspended case from lrel_auth? It would also make serialization always pass *)
-  (*  Definition auth_inv (susp : loc) (s1 : string) :=
-    ((hashed s1 ∗ susp ↦□ InjRV #(hash s1) ∗ auth_valid_val_2 susp) ∨
-       auth_valid_val_3 susp (DfracOwn (3/4)))%I. *)
-
-  (* Definition auth_inv (s1 : string) (susp : loc) : iProp Σ :=
-    ∃ (s : string), ⌜s = some_ser_str (string_ser_str (hash s1))⌝ ∗
-      (hashed s1 ∗ auth_is_ser_2 s susp ∨ auth_is_ser_3_proph s susp). *)
+  
 
   Definition auth_some (A : lrel_bi Σ) (v1 v2 : val) : iProp Σ :=
     (∃ (a1 : val) (t : evi_type) (s1 : string),
@@ -1809,12 +788,24 @@ Section proof.
             simplify_eq.
           + assert (h = h0) as ->; first admit.
             by iFrame "# ∗".
-          + assert (h = h0) as ->; first admit.
-            iMod (na_inv_alloc seqG_name _ (authN N susp) (auth_inv _ susp) with "[Hser1 Hsusp1]") as "#Hinv".
-            { iModIntro. iLeft. iFrame "# ∗". admit. }
-            iModIntro. iFrame "∗ #".
-            iSplit; iLeft; iExists _; iSplit; try done; eauto.
-            admit.
+          + iAssert (⌜h = h0⌝)%I as %->.
+            { iDestruct "Hser1" as %H1. iDestruct "Hser2" as %H2. iPureIntro. naive_solver. }
+            iDestruct "HAb" as "[(%w & % & auth_ab)|%]"; simplify_eq.
+            iDestruct "auth_ab" as "(%ab & %tb & %sb & #hashsb & #Hser_ab & #HA_rel & [% | (%& %& % & % & #Hinv_ab)])"; simplify_eq.
+            iMod (na_inv_acc with "Hinv_ab Htok") as "(Hinv1 & Htok & Hclose)"; [solve_ndisj|solve_ndisj|].
+            iDestruct "Hinv1" as ">[(%s1' & % & #hashss1 & (% & #Hsusp' & #Hser')) | (%& %& %& Hsusp' & _ & _)]"; last first.
+            { iExFalso. iDestruct (pointsto_agree with "Hsusp' Hsusp1") as %?. done. }
+            iDestruct (pointsto_agree with "Hsusp' Hsusp1") as %Heqh. simplify_eq.
+            iMod ("Hclose" with "[$Htok]") as "Htok".
+            { iNext. iLeft. iExists s1'. iSplit; [iPureIntro; congruence|]. iSplit; [iFrame "#"|].
+              iExists h0. iFrame "#". }
+            iModIntro. iFrame "Htok".
+            iSplit.
+            * iAssert (⌜h0 = hash sb⌝)%I as %->.
+              { iDestruct "Hser'" as %H'. iPureIntro. naive_solver. }
+              iLeft. iExists (InjLV #(hash sb)). iSplit; [done|].
+              iExists ab, tb, sb. iFrame "#". iLeft. done.
+            * iLeft. iExists (InjLV #h0). iSplit; [done|]. iLeft. iExists h0. done.
           + iFrame "# ∗".
             iModIntro. iSplit; iLeft; iExists _; iSplit; try eauto.
             iDestruct "HAb" as "[(%&%& (%&%&%& #hashs & #Hser & #HA & HAb))|%]"; simplify_eq.
@@ -1832,440 +823,6 @@ Section proof.
               iModIntro. iSplit; iLeft; iExists _; iSplit; try done; [|iRight; eauto].
               eauto.
             * iPoseProof (pointsto_agree with "Hsusp1 Hsusp") as "%". done. }
-        
-        (* iExists tauth, _, _, _.
-        iSplit; [done|]. clear. iSplit; [|iSplit]; [| |iSplit; [|iSplit]].
-        - iIntros (?????) "!# (#[Hauth _] & Htok) H".
-          rewrite /auth_ser_v. wp_pure.
-          iDestruct "Hauth" as "[(% & -> & Hauth)|->]"; wp_pures; last first.
-          { iApply ("H" $! None). by iFrame. }
-          iDestruct "Hauth" as "(%&%&%&Hser&HA&[(Hhash&%)|(%&%&Hinv)])";
-            simplify_eq; wp_pures.
-          + wp_apply s_ser_spec'.
-            { iRight. eauto. }
-            iIntros (o) "#Ho". destruct o; last first.
-            { iApply ("H"  $! None). by iFrame. }
-            iApply ("H" $! (Some _)). iFrame.
-            iExists _. iSplit; [done|].
-            iLeft. iExists _. eauto.
-          + wp_bind (!_)%E.
-            iMod (na_inv_acc with "Hinv Htok") as "(Hinv1 & Htok & Hclose)"; [solve_ndisj|solve_ndisj|].
-            iDestruct "Hinv1" as (?) "(>% & [(#hashs1& %& #Hsusp & #Hser1)|(%& %& %& Hsusp & Hproph & #Hser1)])".
-            * (* 
-              ∃ (pid: nat) (p : proph_id) (h : string),
-      ⌜v = InjRV #susp⌝ ∗ susp ↦ InjLV (#pid, #p) ∗ proph_susp p h ∗
-        s_is_ser (g:=gwp_upto_bad) auth_scheme (SOMEV #h) s.
-            iMod ("Hclose" with "[Htok]") as "Htok".
-              { iFrame. iNext. iLeft. iFrame "∗ #". }
-              wp_pures.
-              iMod ("Hclose" with "[Htok]") as "Htok".
-              { iFrame. iNext. iLeft. iFrame "∗ #". }
-              wp_apply s_ser_spec'.
-              { iRight. eauto. }
-              iIntros (o) "#Ho". destruct o; last first.
-              { by iApply ("H" $! None). }
-              iApply ("H" $! (Some _)).
-              iFrame.
-              iExists _. iSplit; [done|].
-              iRight. iExists _, _.
-              iSplit; [done|]. iFrame "#". *)
-              wp_load.
-              iMod ("Hclose" with "[Hser HA Hsusp Htok Hser1]") as "Htok".
-              { iFrame. iNext. iExists _. iSplit; first done. iLeft. by iFrame "∗ #". }
-              wp_pures.
-              wp_apply s_ser_spec'.
-              { iRight. eauto. }
-              iIntros (o) "#Ho". destruct o; last first.
-              { iApply ("H" $! None). iFrame. }
-              iApply ("H" $! (Some _)). iFrame.
-              iExists _. iSplit; [done|].
-              iRight. iExists _. iSplit; first done.
-              iExists _. eauto.
-            * wp_load.
-              iMod ("Hclose" with "[Hsusp Hproph Hser1 $Htok]") as "Htok".
-              { iNext. iExists _. iSplit; first done. iRight. by iFrame. }
-              wp_pures.
-              iApply ("H" $! None). by iFrame.
-        (* - iIntros (??) "!# (#Hauth & Htok) H".
-          rewrite /auth_ser_v. wp_pure. iSimpl in "Hauth".
-          iDestruct "Hauth" as "(% & -> & [(% & ->)|(%&%&Hinv)])".
-          + wp_pures. wp_apply s_ser_spec'.
-            { iRight. eauto. }
-            iIntros (o) "#Ho". destruct o; last first.
-            { iApply ("H"  $! None). by iFrame. }
-            iApply ("H" $! (Some _)). iFrame.
-            iExists _. iSplit; [done|].
-            iLeft. iExists _. eauto.
-          + simplify_eq. wp_pures. wp_bind (!_)%E.
-            iMod (na_inv_acc with "Hinv Htok") as "([(%&#Hsusp)|(%&Hsusp)] & Htok & Hclose)"; [done|done| |]; wp_load.
-            * iMod ("Hclose" with "[$Htok]") as "Htok".
-              { iLeft. iFrame "#∗". }
-              wp_pures.
-              wp_apply s_ser_spec'.
-              { iRight. eauto. }
-              iIntros (o) "#Ho". destruct o; last first.
-              { iApply ("H" $! None). by iFrame. }
-              iApply ("H" $! (Some _)). iFrame.
-              iExists _. iSplit; [done|].
-              iRight. iExists _, _.
-              eauto.
-            * iMod ("Hclose" with "[Hsusp $Htok]") as "Htok".
-              { iRight. eauto. }
-              wp_pures.
-              iApply ("H" $! None). by iFrame. *)
-
-        - iIntros (????) "!# (Hser & Htok) HΦ".
-          rewrite /auth_ser_v. wp_pure. iSimpl in "Hser".
-          iDestruct "Hser" as (?->) "[(% & -> & Hser)|(% & ->& Hser)]".
-          + wp_pures. wp_apply s_ser_spec'.
-            { iRight. eauto. }
-            iIntros (o) "#Ho". destruct o; last first.
-            { iApply ("HΦ"  $! None). iFrame. by iRight. }
-            iApply ("HΦ" $! (Some _)). iFrame.
-            iPoseProof (s_is_ser_inj with "Hser Ho") as "->".
-            iLeft. iSplit; first done.
-            simpl. iExists _. iSplit; [done|].
-            iLeft. iExists _. eauto.
-          + simplify_eq. wp_pures. wp_bind (!_)%E.
-            iDestruct "Hser" as "[(%& #Hsusp & Hser1)|(%& %& %& Hsusp & Hproph & Hser1)]".
-            * wp_load.
-              iDestruct "Hser1" as "#Hser1".
-              wp_pures.
-              wp_apply s_ser_spec'.
-              { iRight. eauto. }
-              iIntros (o) "#Ho". destruct o; last first.
-              { iApply ("HΦ" $! None). iFrame. by iRight. }
-              iApply ("HΦ" $! (Some _)). iFrame. iLeft.
-              iPoseProof (s_is_ser_inj with "Hser1 Ho") as "->".
-              iSplit; first done. simpl.
-              iExists _. iSplit; [done|].
-              iRight. iExists _. iSplit; first done.
-              iExists _. eauto.
-            * wp_load. wp_pures.
-              iApply ("HΦ" $! None). iFrame. eauto.
-            
-        - iIntros (???) "!# Hser H".
-          rewrite /auth_count. wp_pures.
-          iDestruct "Hser" as (?->) "[(%& ->& Hser)|(%& ->& Hser)]"; simplify_eq; wp_pures.
-          { iApply ("H" $! 0%nat). iFrame. iModIntro. iExists _.  
-            iSplit; first done. by iLeft. }
-          iDestruct "Hser" as "[(%& #Hsusp & Hser1)|(%& %& %& Hsusp & Hproph & Hser1)]"; wp_load; wp_pures.
-          { iApply ("H" $! 0%nat). iFrame. iModIntro. iExists _.  
-            iSplit; first done. iRight. iExists _. iSplit; first done. 
-            iLeft. by iFrame "∗ #". }
-
-          iApply ("H" $! (1%nat)). iModIntro. iExists _. iSplit; first done.
-          iRight. iExists _. iSplit; first done. iRight. iFrame.
-
-            (* iAssert (susp ↦{#1/2} InjLV #pid ∗ susp ↦{#1/4} InjLV #pid)%I with "[Hsusp]" as "[Hsusp1 Hsusp2]"; [admit|].
-            iSplitR "Hin Heq Hsusp1".
-            { iExists _. iSplit; [done|]. iRight. iExists susp.
-              iSplit; [done|]. iRight. iExists _. iSplit; [|done]. iFrame. }
-            iExists _. iSplit; [done|]. iRight. iExists susp.
-            iSplit; [done|]. iFrame. *)
-          
-          (* iDestruct "Hauth" as "(% & -> & [(% & ->)|(%&%&#Hinv)])"; simplify_eq; wp_pures.
-          { iApply "H". iExists 0. iModIntro. iSplit; [done|].
-            iRight. iExists _. eauto. }
-          wp_bind (!_)%E.
-          iInv "Hinv" as "[(%&#Hsusp)|(%&Hsusp)]" "Hclose"; wp_load.
-          + iMod ("Hclose" with "[]") as "_".
-            { iLeft. eauto. }
-            iModIntro. wp_pures.
-            iApply "H". iExists 0. iModIntro.
-            iSplit; [iPureIntro; f_equal|].
-            iRight. iExists _. iRight.
-            iExists _. iSplit; [done|].
-            iLeft. eauto.
-          + iMod ("Hclose" with "[Hsusp]") as "_".
-            { iRight. eauto. }
-            iModIntro. wp_pures.
-            iApply "H". iExists 1. iModIntro.
-            iSplit; [iPureIntro; f_equal|].
-            iRight. iExists _. iRight. iExists susp.
-            iSplit; [done|]. by iRight. *)
-            
-              
-        - iIntros (??) "!# _ H".
-          rewrite /auth_deser_v. wp_pures.
-          iModIntro. iApply "H".
-          iIntros (s?) "!# _ H".
-          wp_pures. wp_apply s_deser_sound; [done|].
-          iIntros ([] ?); wp_pures; last (by iApply ("H" $! None)).
-          destruct H as [(->&H)|(?&?&(->&H)&?)]; wp_pures.
-          * wp_apply (typed_proph_wp_new_proph1 StringTypedProph); first done.
-            iIntros (??) "Hproph".
-            wp_alloc susp as "Hsusp".
-            (* iMod (own_alloc parent_agree pid tauth NONEV). *)
-            (*          iMod(inv_alloc (authSerN #susp) _ (auth_inv A susp) with "[Hsusp]") as "#Hinv".
-              { iModIntro. iRight. eauto. } *)
-            wp_pures.
-            iApply ("H" $! (Some _)).
-            (* iAssert (susp ↦{#1/4} InjLV (#pid, #p) ∗ susp ↦{#3/4} InjLV (#pid, #p))%I with "[Hsusp]" as "[Hsusp1 Hsusp2]"; [admit|].
-            pose (s' := some_ser_str (string_ser_str v)).
-            iMod (na_inv_alloc seqG_name ⊤ (authSerN N #susp)
-                    (auth_ser_inv (InjRV #susp) s' susp) with "[Hsusp1 Hproph]") as "Hinv".
-            { iNext. iRight. iFrame. iSplit; first done.
-              iRight. iExists _, _. iSplit; first done. eauto. } *)
-            iModIntro.
-            iExists _. iSplit; [done|].
-            (*          { simpl. iExists _. iSplit; [done|].
-                iRight. rewrite /auth_is_ser_3.
-                iExists _, _. iSplit; [done|].
-                iInv "Hinv" as "[(%&%&%&%&Hser&HA&Hhash&#Hsusp)|(%&Hsusp)]" "Hclose".
-                iInv 
-                eauto. } *)
-            iRight. iExists _. iSplit; [done|].
-            iFrame. iSimpl. iLeft. done. 
-          * iModIntro. iApply ("H" $! (Some _)).
-            iExists _. iSplit; [done|].
-            iLeft. rewrite /auth_is_ser_1.
-            destruct! H0. simplify_eq.          
-            iExists _. iSplit; [done|].
-            iRight. iExists _, _.
-            eauto.
-        - iIntros (????????) "!# Htok Hser1 Hser2 [HAb HAu]".
-          destruct t1 as [| | | |]. 1,2,3,4 : admit.
-          destruct t2 as [| | | |]. 1,2,3,4 : admit.
-          iDestruct "Hser1" as "[Hser1|Hser1]".
-          + iDestruct "Hser1" as (??) "[(%&%&Hser1)|(%&%&(%&Hsusp2&Hser1))]";
-              iDestruct "Hser2" as (??) "[(%&%&Hser2)|(%&%&(%&Hsusp1&Hser2))]";
-              simplify_eq.
-            * assert (h = h0) as ->; first admit.
-              by iFrame.
-            * assert (h = h0) as ->; first admit.
-              assert (h0 = (hash s)) as ->; first admit.
-              iAssert (hashed s) as "hashs"; first admit.
-              iModIntro. iFrame. 
-              iSplit; iLeft; iExists _; iSplit; try done;
-                iExists _; iFrame "#"; admit.
-            * assert (h = h0) as ->; first admit.
-              assert (h0 = (hash s)) as ->; first admit.
-              iAssert (hashed s) as "hashs"; first admit.
-              iMod (na_inv_alloc seqG_name _ (authN N #susp) (auth_inv s susp) with "[Hser1 Hsusp2]") as "#Hinv".
-              { iModIntro. iExists _. iSplit; first done. iFrame "# ∗".
-                iLeft. iFrame "∗". iRight. admit. }
-              iModIntro. iFrame.
-              iSplit; iLeft; iExists _; iSplit; try done;
-                iExists _; iFrame "#"; admit.
-            * assert (h = h0) as ->; first admit.
-              assert (h0 = (hash s)) as ->; first admit.
-              iAssert (hashed s) as "hashs"; first admit.
-              iMod (na_inv_alloc seqG_name _ (authN N #susp) (auth_inv s susp) with "[Hser1 Hsusp2]") as "#Hinv".
-              { iModIntro. iExists _. iSplit; first done. iFrame "# ∗".
-                iLeft. iFrame "∗". iRight. admit. }
-              iModIntro. iFrame.
-              iSplit; iLeft; iExists _; iSplit; try done;
-                iExists _; iFrame "#"; admit.
-          + iDestruct "Hser1" as (??) "[(%&%&Hser1)|(%&%&[(%&Hsusp2&Hser1)|(%&%&%&Hsusp2&Hproph&Hser1)])]";
-              iDestruct "Hser2" as (??) "[(%&%&Hser2)|(%&%&(%&Hsusp1&Hser2))]";
-              simplify_eq.
-            * assert (h = h0) as ->; first admit.
-              by iFrame.
-            * assert (h = h0) as ->; first admit.
-              assert (h0 = (hash s)) as ->; first admit.
-              iAssert (hashed s) as "hashs"; first admit.
-              iModIntro. iFrame. 
-              iSplit; iLeft; iExists _; iSplit; try done;
-                iExists _; iFrame "#"; admit.
-            * assert (h = h0) as ->; first admit.
-              assert (h0 = (hash s)) as ->; first admit.
-              iAssert (hashed s) as "hashs"; first admit.
-              iMod (na_inv_alloc seqG_name _ (authN N #susp) (auth_inv s susp) with "[Hser1 Hsusp2]") as "#Hinv".
-              { iModIntro. iExists _. iSplit; first done. iFrame "# ∗".
-                iLeft. iFrame "∗". iRight. admit. }
-              iModIntro. iFrame.
-              iSplit; iLeft; iExists _; iSplit; try done;
-                iExists _; iFrame "#"; admit.
-            * assert (h = h0) as ->; first admit.
-              assert (h0 = (hash s)) as ->; first admit.
-              iAssert (hashed s) as "hashs"; first admit.
-              iMod (na_inv_alloc seqG_name _ (authN N #susp) (auth_inv s susp) with "[Hser1 Hsusp2]") as "#Hinv".
-              { iModIntro. iExists _. iSplit; first done. iFrame "# ∗".
-                iLeft. iFrame "∗". iRight. admit. }
-              iModIntro. iFrame.
-              iSplit; iLeft; iExists _; iSplit; try done;
-                iExists _; iFrame "#"; admit.
-            * assert (h = h0) as ->; first admit.
-              assert (h0 = (hash s)) as ->; first admit.
-              iMod (na_inv_alloc seqG_name _ (authN N #susp) (auth_inv s susp) with "[Hser1 Hsusp2 Hproph]") as "#Hinv".
-              { iModIntro. iExists _. iSplit; first done. iFrame "# ∗".
-                iRight. iFrame. admit. }
-              iModIntro. iFrame.
-              iSplit; iLeft; iExists _; iSplit; try done;
-                iExists _; iFrame "# ∗"; admit.
-            * assert (h = h0) as ->; first admit.
-              assert (h0 = (hash s)) as ->; first admit.
-              iMod (na_inv_alloc seqG_name _ (authN N #susp) (auth_inv s susp) with "[Hser1 Hsusp2 Hproph]") as "#Hinv".
-              { iModIntro. iExists _. iSplit; first done. iFrame "# ∗".
-                iRight. iFrame. admit. }
-              iModIntro. iFrame.
-              iSplit; iLeft; iExists _; iSplit; try done;
-                iExists _; iFrame "# ∗"; admit. }
-          (* iIntros (??????) "!# Htok Hser1 #Hser2 Hauth".
-          iDestruct "Hauth" as "[(% & -> & Hauth)|->]"; last first.
-          { iDestruct "Hser2" as (??) "Hser2". simplify_eq. }
-          iDestruct "Hauth" as "(%&%&%&#Hser&#HA&[(#Hhash&%)|(%&%&#Hinv)])"; simplify_eq.
-          + iDestruct "Hser1" as "[Hser1|Hser1]".
-            * iDestruct "Hser1" as (??) "[(%&%&Hser1)|(%&%&(%&Hsusp2&Hser1))]";
-                iDestruct "Hser2" as (??) "[(%&%&Hser2)|(%&%&(%&Hsusp1&Hser2))]";
-                simplify_eq; iFrame; iLeft; iExists _.
-              -- iFrame "#". iModIntro. iSplit; first done. iLeft.
-                 iDestruct "Hser1" as "[[% %]|(%&%&[% %]&Hser1)]"; simplify_eq.
-                 iDestruct "Hser1" as "(% & % & %)".
-                 iDestruct "Hser2" as "[[% %]|(%&%&[% %]&Hser2)]"; simplify_eq.
-                 iDestruct "Hser2" as "(% & % & %)". by simplify_eq.
-              -- instantiate (1 := (InjRV #susp)).
-                 iMod (na_inv_alloc seqG_name _ (authN N #susp) (auth_inv s1 susp) with "[Hser1 Hsusp2]") as "Hinv".
-                 { iModIntro. iExists _. iSplit; first done. iLeft. iFrame "∗ #".
-                   iRight. iExists _, _. iSplit; first done.
-                   iExists _. iSplit; first done. 
-                   iDestruct "Hser1" as "[[% %]|(%&%&[% %]&Hser1)]"; simplify_eq.
-                   iDestruct "Hser1" as "(% & % & %)".
-                   iDestruct "Hser2" as "[[% %]|(%&%&[% %]&Hser2)]"; simplify_eq.
-                   iDestruct "Hser2" as "(% & % & %)". by simplify_eq. }
-                 iModIntro. iSplit; first done.
-                 iFrame "#". iRight. by iFrame.
-            * iSimpl in "Hser1".
-              iDestruct "Hser1" as (??) "[(%&%&Hser1)|(%&%&Hser1)]";
-                iDestruct "Hser2" as (??) "[(%&%&Hser2)|(%&%&(%&Hsusp1&Hser2))]";
-                simplify_eq; iFrame; iLeft; iExists _.
-              -- iFrame "#". iModIntro. iSplit; first done. iLeft.
-                 iDestruct "Hser1" as "[[% %]|(%&%&[% %]&Hser1)]"; simplify_eq.
-                 iDestruct "Hser1" as "(% & % & %)".
-                 iDestruct "Hser2" as "[[% %]|(%&%&[% %]&Hser2)]"; simplify_eq.
-                 iDestruct "Hser2" as "(% & % & %)". by simplify_eq.
-              -- instantiate (1 := (InjRV #susp)).
-                 iMod (na_inv_alloc seqG_name _ (authN N #susp) (auth_inv s1 susp) with "[Hser1]") as "Hinv".
-                 { iModIntro. iExists _. iSplit; first done. iFrame "∗ #".
-                   iDestruct "Hser2" as "[[% %]|(%&%&[% %]&Hser2)]"; simplify_eq.
-                   iDestruct "Hser2" as "(% & % & %)". by simplify_eq. }
-                  iModIntro. iSplit; first done. iFrame "#". iRight.
-                  by iFrame.
-          
-          + iDestruct "Hser1" as "[Hser1|Hser1]".
-            * iMod (na_inv_acc with "Hinv Htok") as "(Hinv1 & Htok & Hclose)"; [solve_ndisj|solve_ndisj|].
-              iDestruct "Hser1" as (??) "[(%&%&Hser1)|(%&%&(%&#Hsusp2&Hser1))]";
-                iDestruct "Hinv1" as (?) "(>% & [(>#hashs1& %& >#Hsusp & >#Hser1')|(%& %& %& >Hsusp & Hproph & >#Hser1')])";
-                iDestruct "Hser2" as (??) "[(%&%&Hser2)|(%&%&(%&Hsusp1&Hser2))]";
-                simplify_eq.
-              -- iMod ("Hclose" with "[$Htok]") as "$".
-                 { iNext; iExists _. iSplit; first done. iLeft; iFrame "#". }
-                 iPoseProof (pointsto_agree with "Hsusp1 Hsusp") as "%"; simplify_eq.
-                 iModIntro. iLeft. iExists _. iSplit; first done.
-                 iDestruct "Hser1" as "[[% %]|(%&%&[% %]&Hser1)]"; simplify_eq.
-                 iDestruct "Hser1" as "(% & % & %)". simplify_eq.
-                 iDestruct "Hser2" as "[[% %]|(%&%&[% %]&Hser2)]"; simplify_eq.
-                 iDestruct "Hser2" as "(% & % & %)".
-                 iDestruct "Hser1'" as "[[% %]|(%&%&[% %]&Hser1')]"; simplify_eq.
-                 iDestruct "Hser1'" as "(% & % & %)". simplify_eq.
-                 iFrame "#". by iLeft.
-              -- iPoseProof (pointsto_agree with "Hsusp1 Hsusp") as "%"; simplify_eq.
-              -- iPoseProof (pointsto_agree with "Hsusp1 Hsusp") as "%"; simplify_eq.
-                 iDestruct "Hser1" as "[[% %]|(%&%&[% %]&Hser1)]"; simplify_eq.
-                 iDestruct "Hser1" as "(% & % & %)". simplify_eq.
-                 iDestruct "Hser2" as "[[% %]|(%&%&[% %]&Hser2)]"; simplify_eq.
-                 iDestruct "Hser2" as "(% & % & %)".
-                 iDestruct "Hser1'" as "[[% %]|(%&%&[% %]&Hser1')]"; simplify_eq.
-                 iDestruct "Hser1'" as "(% & % & %)". simplify_eq.
-                 iMod (na_inv_alloc seqG_name _ (authN N #susp0) (auth_inv s1 susp0) with "[]") as "#Hinv1".
-                 { iModIntro. iExists _. iSplit; first done. iFrame "∗ #".
-                   iLeft. iRight. do 2 iExists _. iSplit; first done. eauto. }
-                 iMod ("Hclose" with "[$Htok]") as "$".
-                 { iNext; iExists _. iSplit; first done. iLeft; iFrame "#".
-                   iRight. do 2 iExists _. iSplit; first done. eauto. }
-                 iModIntro. iLeft. iExists _. iSplit; first done.
-                 do 3 iExists _. iFrame "#". by iRight.
-              -- iPoseProof (pointsto_agree with "Hsusp1 Hsusp") as "%"; simplify_eq.
-            * iMod (na_inv_acc with "Hinv Htok") as "(Hinv1 & Htok & Hclose)"; [solve_ndisj|solve_ndisj|].
-              iDestruct "Hser1" as (??) "[(%&%&Hser1)|(%&%&Hser1)]";
-                iDestruct "Hinv1" as (?) "(>% & [(>#hashs1& %& >#Hsusp & >#Hser1')|(%& %& %& >Hsusp & Hproph & >#Hser1')])";
-                iDestruct "Hser2" as (??) "[(%&%&Hser2)|(%&%&(%&Hsusp1&Hser2))]";
-                simplify_eq.
-              -- iMod ("Hclose" with "[$Htok]") as "$".
-                 { iNext; iExists _. iSplit; first done. iLeft; iFrame "#". }
-                 iPoseProof (pointsto_agree with "Hsusp1 Hsusp") as "%"; simplify_eq.
-                 iModIntro. iLeft. iExists _. iSplit; first done.
-                 iDestruct "Hser1" as "[[% %]|(%&%&[% %]&Hser1)]"; simplify_eq.
-                 iDestruct "Hser1" as "(% & % & %)". simplify_eq.
-                 iDestruct "Hser2" as "[[% %]|(%&%&[% %]&Hser2)]"; simplify_eq.
-                 iDestruct "Hser2" as "(% & % & %)".
-                 iDestruct "Hser1'" as "[[% %]|(%&%&[% %]&Hser1')]"; simplify_eq.
-                 iDestruct "Hser1'" as "(% & % & %)". simplify_eq.
-                 iFrame "#". by iLeft.
-              -- iPoseProof (pointsto_agree with "Hsusp1 Hsusp") as "%"; simplify_eq.
-              -- iPoseProof (pointsto_agree with "Hsusp1 Hsusp") as "%"; simplify_eq.
-                 iDestruct "Hser1" as "[(% & #Hsusp2 & Hser1)|(%&%&%& Hsusp2 & Hproph & Hser1)]";
-                 iDestruct "Hser2" as "[[% %]|(%&%&[% %]&Hser2)]"; simplify_eq;
-                 iDestruct "Hser2" as "(% & % & %)";
-                 iDestruct "Hser1'" as "[[% %]|(%&%&[% %]&Hser1')]"; simplify_eq;
-                 iDestruct "Hser1'" as "(% & % & %)"; simplify_eq;
-                 iDestruct "Hser1" as "[[% %]|(%&%&[% %]&Hser1)]"; simplify_eq;
-                 iDestruct "Hser1" as "(% & % & %)"; simplify_eq.
-                 ++ iMod (na_inv_alloc seqG_name _ (authN N #susp0) (auth_inv s1 susp0) with "[]") as "#Hinv1".
-                    { iModIntro. iExists _. iSplit; first done. iFrame "∗ #".
-                      iLeft. iRight. do 2 iExists _. iSplit; first done. eauto. }
-                    iMod ("Hclose" with "[$Htok]") as "$".
-                    { iNext; iExists _. iSplit; first done. iLeft; iFrame "#".
-                      iRight. do 2 iExists _. iSplit; first done. eauto. }
-                    iModIntro. iLeft. iExists _. iSplit; first done.
-                    do 3 iExists _. iFrame "#". by iRight.
-                 ++ admit.
-              -- admit. } *)
-                 
-        
-          (* iIntros (?????) "!# (Htok & Heq & Hauth)".
-          iDestruct "Hauth" as "[(% & -> & Hauth)|->]"; iSimpl in "Heq"; last first.
-          { iDestruct "Heq" as "[(% & %)|(% & ([%|(% & % & H)]&Heq))]"; simplify_eq.
-            iFrame. by iRight. }
-
-          iDestruct "Heq" as "[(% & %)|(% & Heq)]"; simplify_eq.
-          iDestruct "Hauth" as "(%&%&%&#Hser&#HA&[(#Hhash&%)|(%&%&#Hinv)])"; simplify_eq.
-          + iDestruct "Heq" as "([%|(% & % & H)] & [%|(% & % & #Hsusp)])";
-              simplify_eq; iFrame; iLeft; iExists _.
-            * iModIntro. iSplit; [done|]. do 3 iExists _. iFrame "∗ #". iLeft. eauto.
-            * iMod (na_inv_alloc seqG_name _ (authN N #susp) (auth_inv s1 susp) with "[Hhash]") as "Hinv".
-              { iModIntro. iExists _. iSplit; first done. iLeft. iFrame "∗ #".
-                iRight. iExists _, _. iSplit; first done.
-                iExists _. done. }
-                (* { iModIntro. iLeft. iFrame "∗ #". do 3 iExists _.
-                iIntros "HancIn". iDestruct "HancIn" as (?) "[_ Heq]".
-                iExists a1. iIntros "_". iFrame. } *)
-              iModIntro. iSplit; [done|]. do 3 iExists _. iFrame "∗ #". iRight.
-              iExists _. iSplit; [done|]. by iFrame.
-          + iMod (na_inv_acc with "Hinv Htok") as "(Hinv1 & Htok & Hclose)"; [solve_ndisj|solve_ndisj|].
-            iDestruct "Heq" as "([%|(% & % & #Hsusp1)] & [%|(% & % & #Hsusp2)])"; simplify_eq;
-              (* simplify_eq; iDestruct "Hinv1" as "[(>#Hsusp & Hval)|(%pid&%&%&%&%&%&% & Hsusp & Hin & Heq)]". *)
-              iDestruct "Hinv1" as (?) "(>% & [(>#hashs1& %& >#Hsusp & >#Hser1)|(%& %& %& >Hsusp & Hproph & >#Hser1)])";
-              iPoseProof (pointsto_agree with "Hsusp Hsusp1") as "%"; try done.
-            (* 2, 4: iMod (timeless (susp0 ↦{DfracOwn (3/4)} InjLV #pid) with "Hsusp") as "Hsusp";
-            iPoseProof (pointsto_agree with "Hsusp1 Hsusp") as "%"; done.
-            all: (iMod ("Hclose" with "[$Htok Hval]") as "Htok").
-            1, 3: iNext; iLeft; iFrame "∗ #".
-            all: iMod (timeless with "Hsusp") as "Hsusp_";
-              iPoseProof (pointsto_agree with "Hsusp1 Hsusp_") as "%";
-              simplify_eq; iFrame.
-            * iModIntro. iLeft. iExists _. iSplit; first done.
-              iFrame "#". by iLeft.
-            * iMod (na_inv_alloc seqG_name _ (authN N #susp1) (auth_inv susp1 s1) with "[]") as "#Hinv2".
-              { iLeft. iFrame "∗ #". iNext. do 3 iExists _.
-                iIntros "HancIn". iDestruct "HancIn" as (?) "[_ Heq]".
-                iExists a1. iIntros "_". iFrame. }
-              iModIntro. iLeft. iExists _. iSplit; first done.
-              do 3 iExists _. iFrame "#". by iRight. *)
-            * iMod ("Hclose" with "[$Htok]") as "$".
-              { iNext; iExists _. iSplit; first done. iLeft; iFrame "#". }
-              iModIntro. iLeft. iExists _. iSplit; first done.
-              iFrame "# ∗".
-              iDestruct "Hser1" as "[(%&%)|(%&%&(%&%)&Hser1)]"; simplify_eq.
-              iDestruct "Hser1" as "(%&%&%)". simplify_eq. by iLeft.
-            * iMod ("Hclose" with "[$Htok]") as "$".
-              { iNext; iExists _. iSplit; first done. iLeft. iFrame "∗ #". }
-              simplify_eq.
-              iMod (na_inv_alloc seqG_name _ (authN N #susp1) (auth_inv s1 susp1) with "[]") as "#Hinv2".
-              { by iFrame "# % ∗". }
-              iModIntro. iLeft. iExists _. iSplit; first done.
-              iFrame "#". by iRight. } *) *)
       { iApply refines_un_Auth_auth. } }
     { rewrite interp_un_forall_unfold.
       iIntros (A ?) "!# _ Htok"; rewrite -!/interp.
@@ -2274,20 +831,6 @@ Section proof.
       iModIntro. iFrame.
       rewrite /auth_ctx. interp_unfold!.
       iApply refines_un_Auth_auth. }
-
-            
-
-  (*        - iIntros (??????) "!# (Hsusp & Hin & Hcount) HΦ".
-          iDestruct "Hin" as (?[??]) "[(% & Hsusp1)|Hf]"; try done.
-          iDestruct "Hcount" as (??) "[[% [% %]]|(% & % & [(% & Hsusp2 & %)|(%& Hsusp2 & %)])]"; simplify_eq.
-          + iPoseProof (pointsto_agree with "Hsusp2 Hsusp1") as "%". done.
-          + iCombine "Hsusp2 Hsusp1 Hsusp" as "H".
-            iAssert (susp0 ↦ InjLV #pid1)%I with "[H]" as "H"; [admit|].
-            wp_store. iApply "HΦ".
-            iAssert (susp0 ↦□ InjRV #h)%I with "[H]" as "#H1"; [admit|].
-            iFrame "#". iModIntro. iExists _. iSplit; [done|].
-            iRight. iSplit; [done|].
-            iLeft. done. *)
   Admitted.
 
   Lemma refines_un_auth_auth Θ (Δ : ctxO Σ Θ) (R : kindO Σ (⋆ ⇒ ⋆) ) (A : kindO Σ ⋆) :
